theories/check2.v
@@ -1,0 +1,4074 @@
+From mathcomp Require Import all_ssreflect.
+From det Require Import finmap ctx lang.
+From det Require Import tree tree_prop.
+From elpi.apps Require Import derive derive.std.
+From HB Require Import structures.
+From det Require Import tree_valid_cut.
+
+
+  Lemma catf_refl {K:choiceType} {T:Type} (A:{fmap K -> T}):
+    A + A = A.
+  Proof. by apply/fmapP => k; rewrite fnd_cat if_same. Qed.
+
+
+Lemma all2_cat_rev {T1 T2} (P : T1 -> T2 -> bool) A B C D:
+  size A = size C -> size B = size D ->
+  all2 P (catrev A B) (catrev C D) = all2 P A C && all2 P B D.
+Proof.
+  elim: A C B D => [|x xs IH] [|y ys]//= B D [H1] H2.
+  rewrite IH//=; last by rewrite H2.
+  rewrite (andbC _ (all2 _ xs _)) andbA//.
+Qed.
+
+Lemma all2_rev {T1 T2} (P : T1 -> T2 -> bool) A B:
+  size A = size B -> all2 P (rev A) (rev B) = all2 P A B.
+Proof. move=> H; by rewrite /rev all2_cat_rev//= andbT. Qed.
+
+Set Implicit Arguments.
+Unset Strict Implicit.
+Import Prenex Implicits.
+
+Lemma tm2RC_kp {t1 k} : 
+  tm2RC t1 = Some (RCallable_Kp k) -> t1 = Tm_Kp k.
+Proof.
+  case: t1 k => //=.
+  - move=> k1 k2 []; congruence.
+  - move=> h b k; case X: tm2RC => //.
+Qed.
+
+Lemma deref_kp {s1 t k}:
+  tm2RC (deref s1 t) = Some (RCallable_Kp k) ->
+    (t = Tm_Kp k) \/ (exists v, t = Tm_V v /\ lookup v s1 = Some (Tm_Kp k)).
+Proof.
+  case: t k => //=.
+  - move=> k1 k2 []; left; congruence.
+  - move=> v k; case x: (lookup _ _) => [t1|]//=.
+    move=>/tm2RC_kp?; subst.
+    right; by eexists.
+  - move=> h b k; case X: tm2RC => //.
+Qed.
+
+Lemma expand_CB_is_ko {u s A B}:
+  (* we have a superficial cut *)
+  step u s A = CutBrothers B -> is_ko B = false.
+Proof.
+  elim: A s B => //=.
+  - move=> _ []//.
+  - move=> A HA s B HB s1 C.
+    case: ifP => //=dA; case: step => //.
+  - move=> A HA B0 _ B HB s C.
+    case E: step => //=[A'|A'].
+      move=> [?]; subst => /=.
+      apply: HA E.
+    have [? sA] := expand_solved_same _ E; subst A'.
+    case X: step => //=[B'][<-]{C}/=.
+    rewrite -success_cut in sA.
+    by apply: success_is_ko.
+Qed.
+
+Definition full_sP {K:countType} {V:eqType} (s: ctx K V) := forall k, lookup k s <> None.
+
+Definition sigV := (ctx V S).
+
+Definition is_sigV (x : sigV) := unit.
+Lemma is_sigV_inhab : forall x, is_sigV x. Proof. exact (fun x => tt). Qed.
+Definition sigV_eqb (x y : sigV) := x == y.
+Lemma sigV_eqb_correct : forall x, eqb_correct_on sigV_eqb x. Proof. by move=>??/eqP. Qed.
+Lemma sigV_eqb_refl : forall x, eqb_refl_on sigV_eqb x. Proof. by move=>?; exact: eqxx. Qed.
+Elpi derive.eqbOK.register_axiomx sigV is_sigV is_sigV_inhab sigV_eqb sigV_eqb_correct sigV_eqb_refl.
+HB.instance Definition _ : hasDecEq sigV := Equality.copy sigV _.
+
+Section min_max.
+    Definition maxD (d1 d2 : D) :=
+    match d1 with
+    | Pred => Pred
+    | _ => d2
+    end.
+
+  Definition minD (d1 d2 : D) :=
+    match d1 with
+    | Func => Func
+    | Pred => d2
+    end.
+
+  Lemma maxD_refl {r}: maxD r r = r.
+  Proof. case: r => //. Qed.
+
+  Lemma maxD_comm {l r}: maxD l r = maxD r l.
+  Proof. case: l; case: r => //. Qed.
+
+  Lemma minD_refl {r}: minD r r = r.
+  Proof. case: r => //. Qed.
+
+  Lemma minD_comm {l r}: minD l r = minD r l.
+  Proof. case: l; case: r => //. Qed.
+
+  Lemma maxD_assoc {x y z}: maxD x (maxD y z) = maxD (maxD x y) z.
+  Proof. case: x => //=; case: y => //=; case: z => //. Qed.
+
+  Lemma minD_assoc {x y z}: minD x (minD y z) = minD (minD x y) z.
+  Proof. case: x => //=; case: y => //=; case: z => //. Qed.
+
+  Definition negD x := match x with Pred => Func | Func => Pred end.
+
+  Fixpoint min_aux minD maxD s1 s2 : S :=
+    let is_min : bool := minD Pred Func == Func in
+    match s1, s2 with
+    | b Exp, b Exp => b Exp
+    | b(d D1), b(d D2) => b (d (minD D1 D2))
+    | arr i l1 r1, arr i l2 r2 => arr i (min_aux maxD minD l1 l2) (min_aux minD maxD r1 r2)
+    | arr o l1 r1, arr o l2 r2 => arr o (min_aux minD maxD l1 l2) (min_aux minD maxD r1 r2)
+  
+    | b (d X), arr _ _ _ | b (d X), b Exp => 
+        if is_min then if X == Func then s1 else s2 else if X == Pred then s1 else s2
+    | arr _ _ _, b (d X) | b Exp, b (d X) => 
+        if is_min then if X == Pred then s1 else s2 else if X == Func then s1 else s2
+
+    | b Exp, arr _ _ _ | arr o _ _, arr i _ _ =>  if is_min then s1 else s2
+    | arr _ _ _, b Exp | arr i _ _, arr o _ _ => if ~~is_min then s1 else s2
+    end.
+
+  Definition min := min_aux minD maxD.
+  Definition max := min_aux maxD minD.
+
+  Lemma min_refl {A}: min A A = A
+  with max_refl {A}: max A A = A.
+  Proof.
+    all: rewrite/min/max in min_refl max_refl *.
+    - by case d1: A => [[|[]]|[] bl br] //=; congr (arr _ _ _).
+    - by case d1: A => [[|[]]|[] bl br] //=; congr (arr _ _ _).
+  Qed.
+
+  Lemma min_comm {A B}: min A B = min B A
+  with max_comm {A B}: max A B = max B A.
+  Proof.
+    all: rewrite/min/max in min_comm max_comm *.
+    - by case d1: A => [[|[]]|[] bl br]; case d2: B => [[|[]]|[] cl cr] //=; congr(arr _ _ _).
+    - by case d1: A => [[|[]]|[] bl br]; case d2: B => [[|[]]|[] cl cr] //=; congr(arr _ _ _).
+  Qed.
+
+  Lemma min_assoc {A B C}: min A (min B C) = min (min A B) C
+  with max_assoc {A B C}: max A (max B C) = max (max A B) C.
+  Proof.
+    all: rewrite/max/min in min_assoc max_assoc *.
+    - case d1: A => [[|[]]|[] bl br]; case d2: B => [[|[]]|[] cl cr];
+      case d3: C => [[|[]]|[] dl dr]//=; f_equal; auto.
+    - case d1: A => [[|[]]|[] bl br]; case d2: B => [[|[]]|[] cl cr];
+      case d3: C => [[|[]]|[] dl dr]//=; f_equal; auto.
+  Qed.
+
+  Lemma min_assorb {A B}: min A (max A B) = A
+  with max_assorb {A B}: max A (min A B) = A.
+  Proof.
+    all: rewrite/max/min in min_assorb max_assorb *.
+    - case d1: A => [[|[]]|[] bl br]; case d2: B => [[|[]]|[] cl cr]//=; f_equal; auto; try by [apply min_refl | apply: max_refl].
+    - case d1: A => [[|[]]|[] bl br]; case d2: B => [[|[]]|[] cl cr]//=; f_equal; auto; try by [apply min_refl | apply: max_refl].
+  Qed.
+
+  Definition incl A B := (min A B == A).
+  Definition not_incl A B := max A B == A.
+
+  Lemma incl_refl {r}: incl r r.
+  Proof. rewrite/incl min_refl//. Qed.
+  
+  Lemma incl_trans {A B C}: incl A B -> incl B C -> incl A C.
+  Proof.
+    rewrite/incl.
+    move=> /eqP<-/eqP<-.
+    rewrite -!min_assoc min_refl//.
+  Qed.
+
+  Lemma min_incl {S1 S2 S3}: min S1 S2 = S3 -> (incl S3 S1).
+  Proof. move=> <-; rewrite /incl min_comm min_assoc min_refl//. Qed.
+
+  Lemma incl_min {S1 S2}: (incl S1 S2) -> min S1 S2 = S1.
+  Proof. rewrite/incl => /eqP//. Qed.
+
+  Lemma not_incl_incl {A B}: not_incl A B = incl B A.
+  Proof. 
+    rewrite/not_incl/incl; do 2 case:eqP => //=.
+      move=> + H; rewrite-H.
+      rewrite max_comm min_assorb//.
+    move=> <-; rewrite min_comm max_assorb//.
+  Qed.
+
+  Lemma max2_incl {A B C D}:
+    max A B = C -> not_incl D A -> not_incl D B -> not_incl D C.
+  Proof.
+    rewrite/not_incl.
+    move=> <- /eqP <- /eqP<-.
+    rewrite -2!max_assoc (@max_comm B) -max_assoc max_refl.
+    rewrite (@max_assoc A) max_refl -max_assoc//.
+  Qed.
+
+  Lemma min2_incl {A B C D}:
+    min A B = C -> incl D A -> incl D B -> incl D C.
+  Proof.
+    rewrite/incl.
+    move=> <- /eqP <- /eqP<-.
+    rewrite -2!min_assoc (@min_comm B) -min_assoc min_refl.
+    rewrite (@min_assoc A) min_refl -min_assoc//.
+  Qed.
+
+  Lemma max2_incl1 {A B C D}:
+    max A B = C -> not_incl A D -> not_incl B D -> not_incl C D.
+  Proof.
+    rewrite/not_incl.
+    move=> <- /eqP <- /eqP<-.
+    rewrite -!max_assoc max_refl//.
+  Qed.
+
+  Lemma min2_incl1 {A B C D}:
+    min A B = C -> incl A D -> incl B D -> incl C D.
+  Proof.
+    rewrite/incl.
+    move=> <- /eqP <- /eqP<-.
+    rewrite -!min_assoc min_refl//.
+  Qed.
+
+  Lemma incl_inv {A B}: incl A B -> A = B \/ (incl B A) = false.
+  Proof.
+    rewrite/incl => /eqP<-.
+    rewrite (@min_comm B) -min_assoc min_refl.
+    case:eqP; auto.
+  Qed.
+
+  Lemma not_incl_inv {A B}: not_incl A B -> A = B \/  (not_incl B A) = false.
+  Proof.
+    rewrite/not_incl => /eqP<-.
+    rewrite (@max_comm B) -max_assoc max_refl.
+    case:eqP; auto.
+  Qed.
+
+  Fixpoint strong s :=
+    match s with
+    | b Exp => b Exp
+    | b(d _) => b(d Func)
+    | arr i l r => arr i (weak l) (strong r)
+    | arr o l r => arr o (strong l) (strong r)
+    end
+  with weak s :=
+    match s with
+    | b Exp => b Exp
+    | b(d _) => b(d Pred) 
+    | arr i l r => arr i (strong l) (weak r)
+    | arr o l r => arr o (weak l) (weak r)
+    end.
+
+  Section test.
+    Definition SMap := 
+      (arr i (arr i (b Exp) (arr o (b Exp) (b(d Func)))) (arr i (b Exp) (arr o (b Exp) (b(d Func))))).
+    Definition WMap := 
+      (arr i (arr i (b Exp) (arr o (b Exp) (b(d Func)))) (arr i (b Exp) (arr o (b Exp) (b(d Pred))))).
+    Goal incl SMap WMap. Proof. move=>//=. Qed.
+    Goal  (incl WMap SMap) = false. Proof. move=>//=. Qed.
+    Goal (weak SMap) == WMap. Proof. move=> //=. Qed.
+  End test.
+
+  Lemma min_strong {A}: min A (strong A) = (strong A)
+  with max_weak {A}: max A (weak A) = (weak A).
+  Proof.
+    all: rewrite/min/max in min_strong max_weak *.
+    - case: A => /=[[|[]]|[]s1 s2]//; rewrite ?min_strong ?max_weak//=.
+    - case: A => /=[[|[]]|[]s1 s2]//; rewrite ?min_strong ?max_weak//=.
+  Qed.
+
+  Lemma min_weak {A}: min A (weak A) = A
+  with max_strong {A}: max A (strong A) = A.
+  Proof.
+    all: rewrite/min/max in min_weak max_strong *.
+    - case: A => /=[[|[]]|[]s1 s2]//; rewrite /=?min_weak ?max_strong//=.
+    - case: A => /=[[|[]]|[]s1 s2]//; rewrite /=?min_weak ?max_strong//=.
+  Qed.
+
+  Lemma func_is_min {A}: incl (b (d Func)) A.
+  Proof. rewrite/incl/=; case: A => //=[[]]//. Qed.
+
+  Lemma pred_is_max {A}: incl A (b (d Pred)).
+  Proof. rewrite/incl/=; case: A => //=[[|[]]|[]]//. Qed.
+
+  Lemma weak_incl {A}: incl A (weak A).
+  Proof. apply/eqP; apply: min_weak. Qed.
+
+  Lemma max_predR {A}: max A (b (d Pred)) = (b (d Pred)).
+  Proof. rewrite max_comm/max/=; case: A => [[]|]//. Qed.
+  
+  Lemma max_predL {A}: max (b (d Pred)) A = (b (d Pred)).
+  Proof. case: A => [[|[]]|[]]//. Qed.
+
+  Lemma max_funcR {A}: max A (b (d Func)) = A.
+  Proof. rewrite max_comm/max/=; case: A => [[]|]//. Qed.
+  
+  Lemma max_funcL {A}: max (b (d Func)) A = A.
+  Proof. case: A => [[|[]]|[]]//. Qed.
+
+  Lemma min_funcR {A}: min A (b (d Func)) = (b (d Func)).
+  Proof. rewrite min_comm/min/=; case: A => [[]|]//. Qed.
+
+  Lemma min_funcL {A}: min (b (d Func)) A = (b (d Func)).
+  Proof. case: A => [[|[]]|[]]//. Qed.
+
+  Lemma strong_incl {A}: incl (strong A) A.
+  Proof. apply: min_incl min_strong. Qed.
+
+  Lemma weak2 {A}: weak (weak A) = weak A
+  with strong2 {A}: strong (strong A) = strong A.
+  Proof. all: case: A => -[]//=??; rewrite?weak2?strong2//. Qed.
+
+  Lemma weak_strong {A B}: weak A = weak B -> strong A = strong B
+  with strong_weak {A B}: strong A = strong B -> weak A = weak B.
+  Proof.
+    - case: A => [[|[]]|[] l1 r1]; case: B => [[]|[]l2 r2]//= [H1 H2]; f_equal; auto.
+    - case: A => [[|[]]|[] l1 r1]; case: B => [[]|[]l2 r2]//= [H1 H2]; f_equal; auto.
+  Qed.
+
+  Lemma min_arr s t s' t' m : min (arr m s' t') (arr m s t)  = arr m (if m == i then max s' s else min s' s) (min t' t). by case: m. Qed.
+  Lemma max_arr s t s' t' m : max (arr m s' t') (arr m s t)  = arr m (if m == i then min s' s else max s' s) (max t' t). by case: m. Qed.
+
+  Lemma incl_arr s t s' t' m :
+    incl (arr m s' t') (arr m s t) = (if m == i then incl s s' else incl s' s) && incl t' t.
+  Proof.
+    rewrite /incl min_arr; case: m => /=; symmetry; (repeat case: eqP); try by [|congruence].
+    - by move=> + E F; rewrite E -F min_comm max_assorb.
+    - by move=> [] <- ??; rewrite max_comm min_assorb.
+  Qed.
+
+  Lemma min_weakr s t : min (min s t) (weak t) = min s t
+  with max_strongr s t : max (max s t) (strong t) = max s t.
+  Proof.
+    all: rewrite/min/max in min_weakr max_strongr *.
+    - case: s => [[|[]]|[] f1 a1]; case: t => [[|[]]|[] f2 a2]//=; f_equal; auto;
+      try by [apply max_strong|apply: min_weak].
+    - case: s => [[|[]]|[] f1 a1]; case: t => [[|[]]|[] f2 a2]//=; f_equal; auto;
+      try by [apply max_strong|apply: min_weak].
+  Qed.
+  
+  Lemma incl_weakr s t : incl s t -> incl s (weak t).
+  Proof. move=> /eqP <-; apply/eqP/min_weakr. Qed.
+
+  Lemma min_abb a b: min (min a b) b = min a b.
+  Proof. rewrite -min_assoc min_refl//. Qed.
+
+  Lemma max_abb a b: max (max a b) b = max a b.
+  Proof. rewrite -max_assoc max_refl//. Qed.
+
+  Lemma inclL_max A B C: incl A C -> incl B C -> incl (max A B) C
+  with inclR_min A B C: incl C A -> incl C B -> incl C (min A B).
+  Proof.
+      case: A => [[|[]]|[] f a]; case: B => [[|[]]|[] f1 a1]; 
+      case: C => [[|[]]|[] f2 a2]//=; rewrite ?pred_is_max//=?max_arr/=?incl_arr//=; cycle 1;
+      [|move=> /andP[H1 H2] /andP[H3 H4]; apply/andP; split; auto..];
+      rewrite/incl/min/=//.
+    move=> /eqP<-/eqP<-; apply/eqP.
+    rewrite -!min_assoc.
+    by rewrite (@min_assoc A B) min_refl.
+  Qed.
+
+  Lemma incl2_max A B C D: incl A C -> incl B D -> incl (max A B) (max C D)
+  with incl2_min A B C D: incl A C -> incl B D -> incl (min A B) (min C D).
+  Proof.
+    move=> H1 H2; apply: inclL_max.
+    - move: H1; rewrite /incl => /eqP <-.
+      rewrite -min_assoc min_assorb//.
+    - move: H2; rewrite /incl => /eqP <-.
+      rewrite -min_assoc max_comm min_assorb//.
+    move=> H1 H2; apply: inclR_min.
+    - move: H1; rewrite /incl => /eqP <-.
+      rewrite min_comm min_assoc (@min_comm C) -(@min_assoc A C C) min_refl//.
+    - move: H2; rewrite /incl => /eqP <-.
+      by rewrite -!min_assoc min_refl.
+  Qed.
+  
+  Lemma inclL_min A B C: incl A C -> incl (min A B) C
+  with inclR_max A B C: incl A C -> incl A (max B C).
+  Proof.
+      move=>/eqP<-; apply/eqP.
+      rewrite min_comm min_assoc.
+      by rewrite (@min_comm A) min_assoc min_refl.
+    case: A => [[|[]]|[] f a]; case: C => [[|[]]|[] f2 a2]//=;
+    rewrite ?max_predR ?pred_is_max ?func_is_min//=;
+    case: B => [[|[]]|[] f3 a3]/=;
+    rewrite ?max_arr/=?max_predL?max_funcL ?pred_is_max?incl_arr//=; cycle 2.
+    - by move=> /andP[]/inclR_max->/inclR_max->.
+    - by rewrite min_comm; move=> /andP[/inclL_min->/inclR_max->]//.
+    - rewrite/max/={3}/incl/=/min/=//.
+  Qed.
+
+  Lemma eq_incl x y : (incl x y && incl y x) = (x == y).
+  Proof.
+    apply/andP/eqP => [[]|-> //]; rewrite?incl_refl//.
+    by move=> /eqP<-/eqP<-; rewrite min_assoc min_refl (@min_comm x) min_assoc min_refl.
+  Qed.
+
+  Lemma min_strong2 {A B}: strong (min (strong A) (strong B)) = (min (strong A) (strong B))
+  with max_weak2 {A B}: weak (max (weak A) (weak B)) = (max (weak A) (weak B)).
+  Proof.
+    all: rewrite/min/max in min_strong2 max_weak2 *.
+    - case: A => /=[[|[]]|[]s1 s2]//; case: B => /=[[|[]]|[]s3 s4]//=; rewrite ?strong2//; f_equal; auto.
+    - case: A => /=[[|[]]|[]s1 s2]//; case: B => /=[[|[]]|[]s3 s4]//=; rewrite ?strong2//?weak2; f_equal; auto.
+  Qed.
+
+
+End min_max.
+Hint Resolve incl_refl : core.
+Hint Resolve minD_refl : core.
+
+Section compat_type.
+  Fixpoint compat_type x y :=
+    match x, y with
+    | b Exp, b Exp => true
+    | b (d _), b (d _) => true
+    | arr i a xb, arr i a' b' => compat_type a a' && compat_type xb b'
+    | arr o a xb, arr o a' b' => compat_type a a' && compat_type xb b'
+    | _, _ => false
+    end.
+
+  Lemma compat_type_refl x: compat_type x x.
+  Proof. elim: x => [[|[]]//|[]//= _ -> _ ->]//. Qed.
+
+  Lemma compat_type_trans2 a b c: 
+    compat_type a b -> compat_type a c = compat_type b c.
+  Proof.
+    elim: a b c => [[|[]] [[|[]]|]//|];
+    move=> []/=f IHf a IHa [[|[]]//|[]f1 a1]//[[|[]]//|[]]//=;
+    move=> f2 a2 /andP[/IHf {}IHf /IHa {}IHa]; f_equal; auto.
+  Qed.
+
+  Lemma compat_type_trans : transitive compat_type.
+  Proof. move=> B A C /compat_type_trans2 ->//. Qed.
+
+  Lemma compat_type_comm x y: compat_type x y = compat_type y x.
+  Proof. by elim: x y => [[|[]][[|[]]|[]]//|] [] f Hf a Ha [[|[]]|[] f1 a1]//=; f_equal. Qed.
+
+  Lemma compat_type_comm1 x y: compat_type x y -> compat_type y x.
+  Proof. by rewrite compat_type_comm. Qed.
+
+  Lemma compat_type_weakL x y: 
+    (compat_type (weak x) y = compat_type x y)
+  with compat_type_strongL x y: 
+    (compat_type (strong x) y = compat_type x y).
+  Proof.
+    by case: x => [[|[]]|[] f a]/=; case: y => [[|[]]|[] f1 a1]//=; f_equal; auto.
+    by case: x => [[|[]]|[] f a]/=; case: y => [[|[]]|[] f1 a1]//=; f_equal; auto.
+  Qed.
+
+  Lemma compat_type_weak x y: 
+    (compat_type (weak x) y = compat_type x y) * (compat_type y (weak x) = compat_type y x).
+  Proof. rewrite (compat_type_comm _ (weak _)) (compat_type_comm y) compat_type_weakL//. Qed.
+
+  Lemma compat_type_min A B C D:
+    compat_type A B -> compat_type B C -> compat_type C D -> compat_type (min A C) (min B D)
+  with compat_type_max A B C D:
+    compat_type A B -> compat_type B C -> compat_type C D -> compat_type (max A C) (max B D).
+  Proof.
+    all: rewrite/max/min in compat_type_min compat_type_max *.
+    - by case Z: B => [[|[]]|[] f a]; case Y: C => [[|[]]|[] f1 a1]//=;
+      case W: A => [[|[]]|[] f2 a2]; case K: D => [[|[]]|[] f3 a3] //=;
+      move=> /andP[H1 H2] /andP[H3 H4] /andP[H5 H6]; apply/andP; auto.
+    - by case Z: B => [[|[]]|[] f a]; case Y: C => [[|[]]|[] f1 a1]//=;
+      case W: A => [[|[]]|[] f2 a2]; case K: D => [[|[]]|[] f3 a3] //=;
+      move=> /andP[H1 H2] /andP[H3 H4] /andP[H5 H6]; apply/andP; auto.
+  Qed.
+
+  (* Lemma compat_type_min1 A B C D:
+    compat_type A C -> compat_type B D -> compat_type (min A B) (min C D)
+  with compat_type_max1 A B C D:
+    compat_type A C -> compat_type B D -> compat_type (max A B) (max C D).
+  Proof.
+    all: rewrite/max/min in compat_type_min1 compat_type_max1 *.
+    - case Z: B => [[|[]]|[] f a]; case Y: C => [[|[]]|[] f1 a1]//;
+      case W: A => [[|[]]|[] f2 a2]; case K: D => [[|[]]|[] f3 a3] //.
+      move=> /andP[H1 H2] /andP[H3 H4] /andP[H5 H6]; apply/andP; auto.
+    - by case Z: B => [[|[]]|[] f a]; case Y: C => [[|[]]|[] f1 a1]//=;
+      case W: A => [[|[]]|[] f2 a2]; case K: D => [[|[]]|[] f3 a3] //=;
+      move=> /andP[H1 H2] /andP[H3 H4] /andP[H5 H6]; apply/andP; auto.
+  Qed. *)
+  
+  Hint Resolve compat_type_refl : core.
+
+  Lemma compat_type_minR A B: compat_type A B -> compat_type A (min A B).
+  Proof. rewrite -{2}(@min_refl A); apply: compat_type_min => //. Qed.
+
+  Lemma compat_type_minL A B: compat_type A B -> compat_type (min A B) A.
+  Proof. rewrite (compat_type_comm _ A); apply compat_type_minR. Qed.
+
+  Lemma compat_type_maxR A B: compat_type A B -> compat_type A (max A B).
+  Proof. rewrite -{2}(@max_refl A); apply: compat_type_max => //. Qed.
+
+  Lemma compat_type_maxL A B: compat_type A B -> compat_type (max A B) A.
+  Proof. rewrite (compat_type_comm _ A); apply compat_type_maxR. Qed.
+
+  Lemma incl_weak2 s t : incl s t -> incl (weak s) (weak t)
+  with not_incl_strong s t : not_incl s t -> not_incl (strong s) (strong t).
+  Proof.
+    case: s => [[|[]]|[] f1 a1]; case: t => [[|[]]|[] f2 a2]//=; 
+    rewrite?pred_is_max//?incl_arr/=.
+    (*IMPOSSIBLE*)
+  Abort.
+
+  Lemma comp_weak s t : compat_type s t -> (weak s) = (weak t)
+  with comp_strong s t : compat_type s t -> (strong s) = (strong t).
+  Proof.
+    by case: s => [[|[]]|[] f1 a1]; case: t => [[|[]]|[] f2 a2]//= => /andP[+/comp_weak ->];
+      [move=> /comp_strong|move=> /comp_weak] => ->.
+    by case: s => [[|[]]|[] f1 a1]; case: t => [[|[]]|[] f2 a2]//= => /andP[+/comp_strong ->];
+      [move=> /comp_weak|move=> /comp_strong] => ->.
+  Qed.
+
+  Lemma compat_type_incl_weak  {A B}: compat_type A B -> incl A (weak B)
+  with compat_type_incl_strong {A B}: compat_type B A -> max B  (strong A) == B.
+  Proof.
+    all: rewrite/incl/min/max in compat_type_incl_weak compat_type_incl_strong *.
+    - case: A => /=[[|[]]|[]s1 s2]//;
+      case: B => /=[[|[]]|[]s3 s4]// => /andP[C1 C2]; apply/eqP; f_equal; apply/eqP; auto.
+    - case: A => /=[[|[]]|[]s1 s2]//;
+      case: B => /=[[|[]]|[]s3 s4]// => /andP[C1 C2]; apply/eqP; f_equal; apply/eqP; auto.
+  Qed.
+
+  Lemma compat_type_weak_eq  {A B}: compat_type A B -> weak A = (weak B)
+  with compat_type_strong_eq {A B}: compat_type A B -> strong A = strong B.
+  Proof.
+    all: rewrite/incl/min/max in compat_type_weak_eq compat_type_strong_eq *.
+    - case: A => /=[[|[]]|[]s1 s2]//;
+      case: B => /=[[|[]]|[]s3 s4]// => /andP[C1 C2]; f_equal; auto.
+    - case: A => /=[[|[]]|[]s1 s2]//;
+      case: B => /=[[|[]]|[]s3 s4]// => /andP[C1 C2]; f_equal; auto.
+  Qed.
+
+
+End compat_type.
+Hint Resolve compat_type_refl : core.
+
+
+Section checker.
+
+  Fixpoint get_sig_hd (sig:S) :=
+    match sig with
+    | b V => V
+    | arr _ _ s => get_sig_hd s
+    end.
+
+  Definition is_det_sig (sig:S) : bool :=
+    get_sig_hd sig == (d Func).
+
+  Definition get_tm_hd_sig (sP : sigT) (sV : sigV) (tm: Tm) : option S :=
+    match get_tm_hd tm with
+    | inl K => Some (b Exp)
+    | inr (inl K) => lookup K sP
+    | inr (inr K) => lookup K sV
+    end.
+
+  Definition get_callable_hd_sig (sP: sigT) sV (t: Callable) : option S :=
+    get_tm_hd_sig sP sV (Callable2Tm t).
+
+  Definition any_pos := (b (d Pred), true).
+  Definition any_neg := (b (d Func), true).
+
+  Fixpoint get_last (s: S) : option (S * mode * S) :=
+    match s with
+    | arr m l r => 
+      if get_last r is Some (l1, m1, r1) then (Some (arr m l l1, m1, r1))
+      else (Some (l, m, r))
+    | _ => None
+    end.
+
+  Definition odflt1 {T} (ab : T * bool) x := match x with (Some x, b1) => (x,b1) | (None,_) => ab end.
+
+  (* takes a tm and returns its signature + if it is well-called
+     the tm has no signature if its head is a variable with no assignment in sV *)
+  Fixpoint check_tm (sP:sigT) (sV:sigV) (tm : Tm)  : S * bool :=
+    match tm with
+    | Tm_Kd k => (b Exp, true)
+    | Tm_Kp k => odflt1 (b(d Pred),false) (lookup k sP, true)
+    | Tm_V v =>  odflt1 (b(d Pred),false) (lookup v sV, true)
+    | Tm_Comb l r => 
+        (* before we check the LHS and then we go right *)
+        let (sl, b1) := check_tm sP sV l  in
+        (* if the type of l is not an arrow, we return anyT *)
+        if sl is arr m tl tr then
+          if m == i then
+            let (cr, br) := check_tm sP sV r in
+            if incl cr tl && b1 && br then (tr, true)
+            else (weak tr, false)
+          else (tr, b1)
+        else (b(d Pred),false)
+    end.
+
+  Definition flex_head T := if get_tm_hd T is inr (inr _) then true else false.
+    
+    (* takes a tm and a signature and updates variable signatures
+     updates are performed only on variables in input positions *)
+  Fixpoint assume_tm (sP:sigT) (sV:sigV) (tm : Tm) (s : seq (mode * S)): sigV :=
+    match tm, s with
+    | _, [::] => sV
+    | (Tm_Kd _ | Tm_Kp _), _ => sV 
+    | Tm_V _, (o, _) :: _ => sV 
+    | Tm_V v, (i, s) :: _ =>
+        match sV.[? v] with
+        | None => sV
+        | Some oldv =>
+          if compat_type oldv s then add v (min s oldv) sV else sV
+        end
+    | (Tm_Comb L R), (m, s) :: sx =>
+      (* we ignore flex_head terms *)
+      if flex_head L then sV
+      else
+        if m == i then
+          (* before we assume in the LHS and then we go right  *)
+          let sV' := assume_tm sP sV L sx in
+          assume_tm sP sV' R (sigtm_rev R s)
+      else assume_tm sP sV L sx
+    end.
+
+  (* assumes the output tm and then it goes on inputs *)
+  Definition assume_call (sP:sigT) (sV:sigV) (c : Callable) (s : S): sigV :=
+    let tm := (Callable2Tm c) in
+    assume_tm sP sV tm (sigtm_rev tm s).
+
+  (* verifies variables in outputs positions *)
+  Fixpoint check_hd (sP:sigT) (sV:sigV) (tm:Tm) (s : seq (mode * S)) : bool :=
+    match tm, s with
+    | _, [::] => true
+
+    (* SKIP INPUT *)
+    | (Tm_Kp _ | Tm_Kd _ | Tm_V _), (i, _) :: _ => true
+    | Tm_Comb l r, (i, tr) :: xs => check_hd sP sV l xs
+
+    (* TEST OUTPUT *)
+    | Tm_Kd _, (o, s) :: _ => incl (b Exp) s
+    | Tm_Kp k, (o, s) :: _ => if lookup k sP is Some x then incl x s else false 
+    | Tm_V v, (o, s) :: _ =>  if lookup v sV is Some x then incl x s else false
+    | Tm_Comb l r, (o, tr) :: xs =>
+        (* getting the type of r and if it is well_called *)
+        let: (tr', b1) := check_tm sP sV r in
+        check_hd sP sV l xs && b1 && (incl tr' tr)
+    end.
+
+  (* checks inputs and assumes outputs of a callable *)
+  Definition check_callable sP sV (c: Callable) d : D * sigV :=
+    match check_tm sP sV (Callable2Tm c) with
+    | ((b Exp | arr _ _ _), _) => (Pred, sV)
+    | (b(d x), b1) =>
+      if b1 then 
+        if get_callable_hd_sig sP sV c is Some s then
+         (maxD x d, (assume_call sP sV c s))
+        else (Pred, sV)
+      else (Pred, sV)
+    end.
+
+  Definition check_atom sP sV (a: A) (s:D) : D * sigV :=
+    match a with
+    | ACut => (Func, sV)
+    | ACall t => check_callable sP sV t s
+    end. 
+
+  (* takes a list of atoms and returns if they typecheck, their determinacy, the updated sigV *)
+  Fixpoint check_atoms sP sV l s :=
+    match l with
+    | [::] => (s, sV)
+    | x :: xs => 
+      let: (s', sV') := check_atom sP sV x s in
+      check_atoms sP sV' xs s'
+    end.
+
+  Definition RCallable_sig (sP: sigT) (t:RCallable) :=
+    get_tm_hd_sig sP [fmap] (Callable2Tm(RCallable2Callable t)).
+
+  Definition empty_ctx : sigV := [fmap].
+  
+  Definition check_rule sP sV head prems :=
+    match RCallable_sig sP head with
+    | None => false
+    | Some hd_sig => 
+        let is_det_head := is_det_sig hd_sig in
+        let tm_head := (Callable2Tm (RCallable2Callable head)) in
+        let ass_hd := assume_tm sP sV tm_head (sigtm_rev tm_head hd_sig) in
+        let: (b1, sV'') := check_atoms sP ass_hd prems Func in
+        (* we reject functional rules with non-deterministic body *)
+        if is_det_head && (b1 == Pred) then false
+        else check_hd sP sV'' tm_head (sigtm_rev tm_head hd_sig)
+    end.
+
+  Definition check_rules sP sV rules :=
+    all (fun x => check_rule sP sV x.(head) x.(premises)) rules.
+
+  Definition check_program sP tE := 
+    forall pr, check_rules sP tE (rules pr).
+End checker.
+
+Lemma check_callable_pred {sP sV c d1 d2 s}:
+  check_callable sP sV c d1 = (d2, s) ->
+    maxD d2 d1 = d2.
+Proof.
+  rewrite/check_callable.
+  case: check_tm => //= -[]; last by move=> _ _ _ _ [<-].
+  move=> [|d [|[<-]]] //; first by move=> _ [<-].
+  case gc: get_callable_hd_sig => [S|][<-]//.
+  rewrite -maxD_assoc maxD_refl//.
+Qed.
+
+Lemma get_tm_hd_callable t:
+  exists R, get_tm_hd (Callable2Tm t) = inr R.
+Proof. elim: t => //=-[]; repeat eexists. Qed.
+
+Global Ltac foo := match goal with H1 : Datatypes.is_true (?x \in domf ?A), H2 : Datatypes.is_true (?x \notin domf ?A) |- _ => by rewrite H1 in H2 end.
+Section merge.
+
+  Open Scope fset_scope.
+
+  Lemma valPE {K : choiceType} V x (H : {fmap K -> V}) (xH : x \in domf H) : [` (valP [`xH]) ] = [` xH].
+  Proof.
+    by move: (valP _); rewrite [val _]/= => xH'; rewrite (bool_irrelevance xH' xH).
+  Qed.
+
+  Lemma fnd_in {T : choiceType} V (f : {fmap T -> V}) (k : T) (kA : k \in domf f) :
+    f.[kA] = odflt f.[kA] f.[? k].
+  Proof. by rewrite in_fnd. Qed.
+
+  Lemma fun_if_Some (T : eqType) p (d : T) : (if p is Some x then Some x else Some d) = Some (if p is Some x then x else d).
+  Proof. by case: p. Qed.
+
+  Lemma in_fst (T:choiceType) (f g : {fset T}) (x : f `&` g) : val x \in f.
+  Proof. by case: x => /= x; rewrite in_fsetE; case/andP. Defined.
+  Lemma in_snd (T:choiceType) (f g : {fset T}) (x : f `&` g) : val x \in g.
+  Proof. by case: x => /= x; rewrite in_fsetE; case/andP. Defined.
+  Lemma fst_snd_in (T:choiceType) (F G : {fset T}) x (xF : x \in F) (xG : x \in G) : x \in F `&` G.
+  Proof. by rewrite in_fsetE xF xG. Qed.
+
+  Lemma fstE (T:choiceType) (F G : {fset T}) x (xF : x \in F) (xG : x \in G) : in_fst (Sub x (fst_snd_in xF xG)) = xF.
+  Proof. by apply: bool_irrelevance. Qed.
+  Lemma sndE (T:choiceType) (F G : {fset T}) x (xF : x \in F) (xG : x \in G) : in_snd (Sub x (fst_snd_in xF xG)) = xG.
+  Proof. by apply: bool_irrelevance. Qed.
+
+  Lemma domfU2 x {A B : sigV} : x \in domf A `|` domf B -> (x \in domf A) + (x \in domf B).
+  Proof. rewrite in_fsetU; case: (x \in domf A); [left|right] => //. Qed.
+
+  Inductive merge_dom_spec {T : choiceType} k (A B : {fset T}) : bool -> bool -> Type :=
+  | InBoth : forall ka : k \in A, all_equal_to ka -> forall kb : k \in B, all_equal_to kb -> merge_dom_spec true true
+  | InLeft : forall ka : k \in A, all_equal_to ka -> k \notin B -> merge_dom_spec true false
+  | InRight : k \notin A -> forall kb : k \in B, all_equal_to kb -> merge_dom_spec false true.
+  
+  Lemma fsetUP {T : choiceType} {x} {A B : {fset T}} :
+    (x \in A) + (x \in B) -> merge_dom_spec x A B (x \in A) (x \in B).
+  Proof.
+    case E: (x \in A); case F: (x \in B) => // AB.
+    by apply: InBoth (E) _ (F) _ => ?; apply: bool_irrelevance.
+    by apply: InLeft (E) _ _; rewrite ?F // => ?; apply: bool_irrelevance.
+    by apply: InRight _ (F) _; rewrite ?E // => ?; apply: bool_irrelevance.
+    by case: AB.
+  Qed.
+
+  Inductive fsetI_spec {T : choiceType} k (A B : {fset T}) : bool -> bool -> Type :=
+  | Both: forall ka : k \in A, all_equal_to ka -> forall kb : k \in B, all_equal_to kb -> fsetI_spec true true.
+
+  Lemma fsetILR  {T : choiceType} {x} {A B : {fset T}} :
+    x \in A -> x \in B -> fsetI_spec x A B (x \in A) (x \in B).
+  Proof. by move=> E F; rewrite E F; apply: Both (E) _ (F) _ => ?; apply: bool_irrelevance. Qed.
+
+  Definition merge_sig (f g: sigV) : sigV :=
+   [fmap k : domf f `|` domf g =>
+          match fsetUP (domfU2 (valP k)) with
+            | InBoth kf _ kg _ => max f.[kf] g.[kg]
+            | InLeft kf _ _    => weak f.[kf]
+            | InRight _ kg _   => weak g.[kg]
+          end].
+
+  Lemma merge_sig_domf A B: domf (merge_sig A B) = domf A `|` domf B.
+  Proof. apply/fsetP => //=. Qed.
+  
+
+  Lemma merge_sigL k f g :
+      k \in domf f -> k \notin domf g ->
+      (merge_sig f g).[? k] = omap weak f.[? k].
+  Proof.
+    move=> /[dup] kf kf_ nkg.
+    have H : k \in domf (merge_sig f g) by rewrite in_fsetE kf.
+    rewrite /merge_sig (in_fnd H) (in_fnd kf) /= ffunE.
+    by case: fsetUP => [//|/=? -> ?|//] in kf_ nkg *.
+  Qed.
+
+  Lemma merge_sigR k f g :
+      k \notin domf f -> k \in domf g ->
+      (merge_sig f g).[? k] = omap weak g.[? k].
+  Proof.
+    move=> nkf /[dup] kg_ kg.
+    have H : k \in domf (merge_sig f g).
+      by rewrite in_fsetE kg orbC.
+    rewrite /merge_sig (in_fnd H) (in_fnd kg) /= ffunE.
+    by case: fsetUP => [//|//|/= ?? ->] in nkf kg_ *.
+  Qed.
+
+  Lemma merge_sigLR k f g :
+      forall kf :k \in domf f, forall kg : k \in domf g,
+      (merge_sig f g).[? k] = Some (max f.[kf] g.[kg]).
+  Proof.
+    move=> /[dup] kf_ kf /[dup] kg_ kg.
+    have H : k \in domf (merge_sig f g) by rewrite in_fsetE kf kg.
+    rewrite /merge_sig (in_fnd H) /= ffunE.
+    case: fsetUP => [/=kf' -> kg' -> |//|//] in kf_ kg_ *.
+    by case: max.
+  Qed.
+
+  Lemma merge_sig_None k f g :
+      forall kf :k \notin domf f, forall kg : k \notin domf g,
+      (merge_sig f g).[? k] = None.
+  Proof.
+    move=> /[dup] kf_ kf /[dup] kg_ kg.
+    have H : k \notin domf (merge_sig f g).
+      by rewrite in_fsetE (negPf kf) (negPf kg).
+    by rewrite not_fnd//.
+  Qed.
+ 
+  Lemma merge_refl {A}: merge_sig A A = A.
+  Proof. 
+    apply/fmapP=> k; case: fndP => /[dup] kAA_ kAA; case: fndP => kA //.
+      congr (Some _); rewrite /merge_sig ffunE.
+      case: fsetUP => /= [_ -> {}kA ->|//|]; first by rewrite max_refl.
+        by move=> ? _; rewrite kA.
+      by rewrite {1}kA.
+    - by move: kAA_ kA; rewrite /= in_fsetE=> /orP[->|->].
+    by move: kAA; rewrite /= in_fsetE kA.
+  Qed.
+
+  Lemma merge_comm {A B}: merge_sig A B = merge_sig B A.
+  Proof.
+    rewrite /merge_sig.
+    apply/fmapP=> k.
+    case: fndP => /= [/[dup] kAB_ kAB|nkAB].
+      have kBA : k \in domf B `|` domf A by rewrite fsetUC.
+      rewrite in_fnd /= !ffunE /=; congr (Some _).
+      case: fsetUP => [kA UkA kB UkB|kA UkA nkB|nkA kB UkB];
+      case: fsetUP => [kB' _ kA' _|kB' _ nkA'|nkB' kA' _]; rewrite ?UkA ?UkB; try by [foo|].
+      by exact max_comm.
+    have nkBA : k \notin domf B `|` domf A by rewrite fsetUC.
+    by rewrite not_fnd.
+  Qed.
+
+End merge.
+
+Definition sigma2ctx (sP:sigT) sV (s: Sigma) : sigV :=
+  [fmap k : domf s =>
+    let (S, b1) := check_tm sP sV s.[valP k] in
+      if b1 then S else weak S].
+
+Lemma sigma2ctx_empty sP sV:
+  sigma2ctx sP sV empty = empty_ctx.
+Proof.
+  apply/ fmapP => /=v.
+  repeat case: fndP => //.
+Qed.
+
+Fixpoint get_ctxS sP te (s:sigV) A :=
+  match A with
+  | CutS | CallS _ _ | Bot | OK | Dead => s
+  | Or A s1 B => if is_dead A then get_ctxS sP te (sigma2ctx sP te s1) B else get_ctxS sP te s A
+  | And A _ B => if success A then get_ctxS sP te (get_ctxS sP te s A) B else (get_ctxS sP te s A)
+  end.
+
+Definition all_compat_type f g :=
+  [forall k : domf f `|` domf g, 
+    match fsetUP (domfU2 (valP k)) with
+      | InBoth kf _ kg _ => compat_type f.[kf] g.[kg]
+      | InLeft kf _ _    => true
+      | InRight _ kg _   => true
+    end 
+  ].
+
+Definition weak_all (s:sigV) : sigV := [fmap x : domf s => weak s.[valP x]].
+
+Definition all_weak (sV:sigV):= [forall k : domf sV, sV.[valP k] == weak (sV.[valP k]) ].
+
+(* a free alternative can be reached without encountering a cutr following SLD 
+
+  "((A, !, A') ; B) , C" is OK since B is not free
+  "((A, A') ; B) , !, C" is OK because any alt from first conjunct dies
+  "((A, A') ; B) , C" is OK if B is dead already (cutr by predecessor of A for example)
+
+*)
+
+(* I need te since in the OR branch I translate the substitution s
+   for the state B. In substitution, some variables that are in
+   the full tree may not be mapped, te is essentially the
+   typing environment, whereas sVD.2 is the substitution
+   updated by the det_checker. *)
+Fixpoint tc_tree_aux (sP:sigT) A (te:sigV) (sVD1:(D * sigV)): (D * sigV) :=
+  let (d0, sV1) := sVD1 in
+  match A with
+  | CutS => (Func, te + sV1)
+  | Bot | Dead => (Func, te + sV1)
+  | CallS _ a => 
+    let (dCall, sV') := (check_callable sP (te + sV1) a d0) in  (maxD d0 dCall, sV')
+  | OK => (d0, te + sV1)
+  | And A B0 B =>
+    if is_ko A then (Func, te + sV1)
+    else 
+    if is_ko B0 then
+      if success A then
+        tc_tree_aux sP B te (d0, te + get_ctxS sP te sV1 A)
+      else (d0, te + sV1)
+    else
+    (* we prepend B0 to the continuation *)
+    (* TODO: in case of success in A, we should remove the success from the
+       execution of k1
+       For example in the state:
+       - `(OK \/ ALT) /\_RESET B`, RESET should not be run with OK
+       A way of doing so count be: I pass (FULL, sV) instead of SVD,
+       where full is such that: merge_sig FULL A = merge_sig A FULL = A
+       NOTE: if the return is FULL, then it would mean that the state after the succes is_ko
+       For example: 
+       - `(A \/ KO) /\_RESET B`, RESET will never be run since KO is_ko
+         The previous state may be generated from `(! \/ ANY) /\_RESET B` *)
+    let: (D, T) := tc_tree_aux sP A te sVD1 in
+    let: (D, T) := tc_tree_aux sP B0 te (D, T) in
+    (* if A is a success then we need to consider B, otherwise (in a valid state), B = B0 *)
+    if success A then
+      let: (DB, TB) := tc_tree_aux sP B te (d0, get_ctxS sP te sV1 A) in
+      (maxD DB D, merge_sig T TB)
+    else (D, T)
+  | Or A s B =>
+      (* We launch A with the signature received in entry, but B
+         should take into account the substitution s *)
+      (* let max_ko X := (maxD d0 X.1, X.2) in *)
+      let max_ko x := x in
+      (* TODO: in all cases we should consider:
+         if there is a cut in A or B, they do not lower the determinacy
+         received in entry (i.e. d0), but the continuation can.
+         For example, we can have:
+         - (A \/ !) and k = OK: in this case if d0 is pred, it stays pred
+         - (A \/ B) and k = !: in this case for any d0, the result will be func *)
+      if is_ko A && is_ko B then (Func, te + sV1)
+      else if is_ko A then max_ko (tc_tree_aux sP B te (d0, sigma2ctx sP te s))
+      else if is_ko B then max_ko (tc_tree_aux sP A te sVD1)
+      else  
+        let dA  := tc_tree_aux sP A te sVD1 in
+        let dB := tc_tree_aux sP B te (d0, sigma2ctx sP te s) in
+        let func :=
+          if has_cut A then maxD d0 (maxD dA.1 dB.1)
+          else Pred in
+        (func, merge_sig dA.2 dB.2)
+  end.
+
+Definition all_vars_subset {K:choiceType} {V: Type} (sV: {fmap K -> V}) (vars:{fset K}) :=
+  [forall x : vars, val x \in sV ].
+
+Definition closed_inT (sV: sigV) t := all_vars_subset sV (vars_tree t).
+
+Definition compat_subst (sP:sigT) (N:sigV) (s:Sigma) :=
+  all_vars_subset N (vars_sigma s) &&
+  [forall x: domf s, if N.[?val x] is Some T then (compat_type (check_tm sP N s.[valP x]).1 T) else false].
+
+Fixpoint compat_sig_subst sP N T :=
+  let rec := compat_sig_subst sP N in
+  match T with
+  | Or A s B => [&& compat_subst sP N s, rec A & rec B]
+  | And A B0 B => [&& rec A, rec B0 & rec B]
+  | Bot | OK | Dead | CutS | CallS _ _ => true
+  end.
+
+Definition tc sP ty T :=
+  [&& all_weak ty,              (*all sig in ty are weak*)
+    closed_inT ty T &           (*all variables in the tree are in ty*)
+    compat_sig_subst sP ty T  (*all variables in OR are mapped and compatible with the sig in ty*)
+  ].
+
+Definition compat_sig (N O:sigV) :=
+  [forall x: domf O, compat_type O.[valP x] (odflt O.[valP x] N.[?val x])].
+
+Definition tcE (tyO:sigV) (tyN:sigV) := 
+  { X | tyN = (X + tyO) }.
+
+Lemma tcEP tyO tyN: 
+  tcE tyO tyN ->
+  compat_sig tyO tyN /\ (domf tyO `<=` domf tyN).
+Proof.
+  move=> [X->]; split.
+    apply/forallP => -[k kP]; rewrite valPE [val _]/=.
+    by rewrite fnd_in lookup_cat; case: (fndP tyO k) => //.
+  by rewrite domf_cat fsubsetUr.
+Qed.
+
+Section orP.
+
+  Lemma closed_inT_orP ctx A s B: 
+    reflect [/\ closed_inT ctx A & closed_inT ctx B]
+        (closed_inT ctx (Or A s B)).
+  Proof.
+    case C: (closed_inT _ (Or _ _ _)); constructor; move: C; last (move=> /negP; apply: contra_not);
+    rewrite/closed_inT.
+      move=> /forallP/= H; split;apply/forallP => /= -[/=] k kP;
+      (have kP': k \in vars_tree A `|` vars_tree B by rewrite !in_fsetU kP//= !orbT);
+      by have:= H (Sub k kP').
+    move=> [HA HB].
+    apply/forallP => -[k]/=; rewrite !in_fsetU => /orP[]H.
+    apply: forallP HA (Sub k H).
+    apply: forallP HB (Sub k H).
+  Qed.
+
+  Lemma compat_sig_subst_orP sP N A s B:
+    compat_sig_subst sP N (Or A s B) <-> [/\ compat_sig_subst sP N A, compat_sig_subst sP N B & compat_subst sP N s].
+  Proof.
+    split; first by move=> /and3P[].
+    by move=> [*]; apply/and3P.
+  Qed.
+
+  Lemma tc_orP sP N A s B:
+    tc sP N (Or A s B) <-> [/\ tc sP N A, tc sP N B & compat_subst sP N s].
+  Proof.
+    rewrite/tc; split.
+      by move=> /and3P[->]/=/closed_inT_orP[->->]/compat_sig_subst_orP[->->->].
+    move=> [/and3P[->]]/= cA csA /andP[cB csB] cs.
+    apply/andP;split.
+      by apply/closed_inT_orP.
+    by apply/compat_sig_subst_orP.
+  Qed.
+
+  (* Lemma tcE_orP sP N O A s B:
+    gtee sP N O (Or A s B) <-> [/\ gtee sP N O A, gtee sP N O B & compat_subst sP N s].
+  Proof.
+    rewrite/gtee; split.
+      by move=> /and3P[/tc_orP[->->->]]/=->->.
+    move=> [/andP[H1 ->] /andP[H4 _] H5].
+    by rewrite andbT; apply/tc_orP.
+  Qed. *)
+End orP.
+
+Section andP.
+
+  Lemma closed_inT_andP ctx A B0 B: reflect [/\ closed_inT ctx A, closed_inT ctx B0 & closed_inT ctx B] (closed_inT ctx (And A B0 B)) .
+  Proof.
+    case C: (closed_inT _ (And _ _ _)); constructor; move: C; last (move=> /negP; apply: contra_not);
+    rewrite/closed_inT.
+      move=> /forallP/= H; split;apply/forallP => /= -[/=] k kP;
+      (have kP': k \in vars_tree A `|` vars_tree B0 `|` vars_tree B by repeat ((apply/finmap.fsetUP; auto); left));
+      by have:= H (Sub k kP').
+    move=> [/forallP/= HA /forallP/= HB0 /forallP/= HB].
+    apply/forallP => /= -[/=k]; move=>/finmap.fsetUP[/finmap.fsetUP[]|] H.
+    apply: HA (Sub k H).
+    apply: HB0 (Sub k H).
+    apply: HB (Sub k H).
+  Qed.
+
+  Lemma compat_sig_subst_andP sP N A B0 B:
+    compat_sig_subst sP N (And A B0 B) <-> [/\ compat_sig_subst sP N A, compat_sig_subst sP N B0 & compat_sig_subst sP N B].
+  Proof.
+    split; first by move=> /and3P[].
+    by move=> [*]; apply/and3P.
+  Qed.
+
+  Lemma tc_andP sP N A B0 B:
+    tc sP N (And A B0 B) <-> [/\ tc sP N A, tc sP N B0 & tc sP N B].
+  Proof.
+    rewrite/tc; split.
+      by move=> /and3P[->]/closed_inT_andP[->->->]/compat_sig_subst_andP[->->->].
+    move=> [/andP[-> /andP[cA csa]] /=/andP[cB0 csB0] /andP[cB csB]].
+    apply/andP;split.
+      by apply/closed_inT_andP.
+    by apply/compat_sig_subst_andP.
+  Qed.
+
+  (* Lemma gtee_andP sP N O A B0 B:
+    gtee sP N O (And A B0 B) <-> [/\ gtee sP N O A, gtee sP N O B0 & gtee sP N O B].
+  Proof.
+    rewrite/gtee; split.
+      by move=> /andP[/tc_andP[->->]]->.
+    move=> [/andP[H1 ->] /andP[H3 H4] /andP[H5 H6]].
+    by rewrite andbT; apply/tc_andP.
+  Qed. *)
+End andP.
+
+Definition good_assignment sP tE SV vk :=
+  let (S, b1) := check_tm sP tE vk in
+  let SS := if b1 then S else weak S in
+  compat_type SS SV && incl SS SV.
+
+Lemma incl_good_assignment sP te s s' v :
+  incl s s' ->
+  compat_type s s' ->
+  good_assignment sP te s v ->
+  good_assignment sP te s' v.
+move=> i c; rewrite /good_assignment; case E: check_tm => [sk []]; rewrite ?valPE/=.
+  move=> /andP[comp_sk isk]; rewrite (compat_type_trans comp_sk)  //.
+  by rewrite (incl_trans isk) // in2_more_precise.
+ move=> /andP[comp_sk isk]; rewrite (compat_type_trans comp_sk)  //.
+  by rewrite (incl_trans isk) // in2_more_precise.
+Qed.
+
+Definition sigP (sP:sigT) ty (s: Sigma) (sV: sigV) :=
+  (* (domf s `<=` domf sV) && *)
+  [forall k : domf sV,
+    let SV := sV.[valP k] in
+    if s.[?val k] is Some vk then good_assignment sP ty SV vk
+    else SV == weak SV].
+
+Lemma sigma2ctx_domf sP s B: domf (sigma2ctx sP B s) = domf s.
+Proof. move=> //. Qed.
+
+Definition closed_in (sV: sigV) t := all_vars_subset sV (vars_tm t).
+
+Lemma all_vars_subset_point {K: choiceType} {V : Type} O v:
+  @all_vars_subset K V O [fset v] = (v \in domf O).
+Proof.
+  rewrite/all_vars_subset/=; apply/forallP => /=.
+  case:ifP.
+    move=> H -[k kV]/=.
+    by move: kV; rewrite in_fset1 => /eqP->.
+  move=>/negP; apply: contra_not.
+  by move=> /(_ (Sub v(fset11 v)))//.
+Qed.
+
+Lemma all_vars_OR {K: choiceType} {V : Type} (O: {fmap K -> V}) f a: all_vars_subset O (f `|` a) =
+  all_vars_subset O f && all_vars_subset O a.
+Proof.
+  apply/forallP => /=; case:ifP => [|/negP].
+    move=> /andP[H1 H2][k /[dup] /finmap.fsetUP [kfa|kfa] kfa_]/=.
+      by have := forallP H1 (Sub k kfa).
+    by have := forallP H2 (Sub k kfa).
+  apply: contra_not.
+  move=> H; apply/andP; split; apply/forallP => -[k kP]/=;
+  (have kU: k \in f `|` a by apply/finmap.fsetUP; auto);
+  apply: H (Sub k kU).
+Qed.
+
+Lemma change_only_in_tm_ck_tm_ {sP T O1 O2}:
+  closed_in O1 T ->
+  check_tm sP (O2+O1) T = check_tm sP O1 T.
+Proof.
+  move=> tmp; symmetry; move: tmp.
+  rewrite/closed_in.
+  elim: T => //.
+    move=> v; rewrite all_vars_subset_point [check_tm _ _ _]/= => vO1.
+    by rewrite in_fnd /check_tm lookup_cat vO1 /= in_fnd.
+  move=> f Hf a Ha.
+  rewrite [all_vars_subset _ _]/= all_vars_OR => /andP[/Hf {}Hf /Ha{}Ha].
+  rewrite/=Hf Ha//.
+Qed.
+
+Lemma vars_tm_vars_sigma (x: V) (k:V) (s:Sigma) (kP : k \in domf s):
+  x \in vars_tm s.[kP] -> x \in vars_sigma s.
+Proof.
+  move=> H; rewrite /vars_sigma in_fsetU.
+  apply/orP; right; rewrite/codom_vars.
+Admitted.
+
+Lemma all_vars_subset_closed_in R s k (kP: k \in domf s):
+  all_vars_subset R (vars_sigma s) -> closed_in R s.[kP].
+Proof.
+  move=> /forallP/= H.
+  apply/forallP => -[x xP]/=.
+  apply: H (Sub x _).
+  apply: vars_tm_vars_sigma xP.
+Qed.
+
+Lemma sigma2ctx_cat sP X R s:
+  compat_subst sP R s ->
+  (sigma2ctx sP (X + R) s) = (sigma2ctx sP R s).
+Proof.
+  move=> /andP [H _].
+  apply/fmapP => k.
+  case: fndP => k1; case: fndP => k2//; last first.
+    by rewrite sigma2ctx_domf k2 in k1.
+    by rewrite sigma2ctx_domf k1 in k2.
+  rewrite !ffunE/= !valPE.
+  rewrite (bool_irrelevance k1 k2).
+  rewrite change_only_in_tm_ck_tm_//.
+  by apply: all_vars_subset_closed_in.
+Qed.
+
+Lemma all_weakKR_compat K R:
+  all_weak K -> all_weak R -> domf R `<=` domf K ->
+  compat_sig R K ->
+  exists X, K = X + R /\ all_weak X.
+Proof.
+  move=> wK wR dRK cKR.
+  exists K; split; auto.
+  apply/fmapP => k.
+  rewrite lookup_cat; case: (fndP R k) => //= kR.
+  have kK := fsubsetP dRK k kR.
+  rewrite in_fnd.
+  have /eqP:= forallP wR (Sub k kR); rewrite valPE => ->.
+  have /eqP:= forallP wK (Sub k kK); rewrite valPE => ->.
+  have:= forallP cKR (Sub k kK); rewrite valPE in_fnd/=.
+  by move=> /compat_type_weak_eq->.
+Qed.
+
+(* Lemma tcE_cat sP N O A B:
+  tc sP O A ->
+  tc sP N B -> 
+  tcE O N ->
+  exists X, N = X + O /\ all_weak X.
+Proof.
+  move=> /and3P[wO _ _] /and3P[wN _ _] [X?]; subst.
+  repeat eexists.
+  apply/forallP => -[k kX]; rewrite valPE.
+  have kXO : k \in domf (X + O) by rewrite domf_cat in_fsetU kX.
+  have:= forallP wN (Sub k kXO); rewrite valPE.
+  rewrite fnd_in lookup_cat.
+  rewrite in_fnd.
+  case: fndP => kO//=.
+
+
+  Search forallP cat.
+  by apply: all_weakKR_compat.
+Qed. *)
+
+Lemma sigma2ctx_cat1 sP O N A B s X:
+  tc sP O A -> tc sP N B ->
+  compat_subst sP O s ->
+  (sigma2ctx sP (X + O) s) = (sigma2ctx sP O s).
+Proof.
+  move=> tA tB C; subst.
+  rewrite sigma2ctx_cat//.
+Qed.
+
+Lemma sigma2ctx_in_s sP tE k s:
+  k \in domf (sigma2ctx sP tE s) -> k \in domf s.
+Proof. by []. Qed.
+
+Lemma sigP_id sP tE s: sigP sP tE s (sigma2ctx sP tE s).
+Proof.
+  apply/forallP => -[k ks]; rewrite valPE ffunE valPE [val _]/=.
+  have kS := sigma2ctx_in_s ks.
+  rewrite in_fnd.
+  rewrite/good_assignment.
+  rewrite (bool_irrelevance kS ks).
+  case: check_tm => a b.
+  by rewrite compat_type_refl incl_refl.
+Qed.
+
+Lemma is_ko_tc_tree_aux {sP A R d}:
+  is_ko A -> tc_tree_aux sP A R d = (Func, R + d.2).
+Proof.
+  elim: A d=> //=; only 1, 2: by case.
+  - by move=> A HA s B HB [D SV] ->//.
+  - by move=> A HA B0 HB0 B HB [D SV] ->.
+Qed.
+
+Lemma is_dead_tc_tree_aux {sP A R d}:
+  tc_tree_aux sP (dead A) R d = (Func, R + d.2).
+Proof.
+  apply: is_ko_tc_tree_aux.
+  apply: is_dead_is_ko is_dead_dead.
+Qed.
+
+Lemma cutr_tc_tree_aux {sP R A d}:
+  tc_tree_aux sP (cutr A) R d = (Func, R + d.2).
+Proof. apply: is_ko_tc_tree_aux is_ko_cutr. Qed.
+
+Lemma get_ctxS_cutl sP tE A s: success A -> get_ctxS sP tE s (cutl A) = get_ctxS sP tE s A.
+Proof.
+  elim: A s => //=.
+    by move=> A HA smid B HB s; case:ifP => [dA sB|dA sA]/=; rewrite ?is_dead_cutl dA; auto.
+  move=> A HA B0 _ B HB s /andP[sA sB].
+  rewrite sA/= success_cut sA.
+  rewrite HB//= HA//.
+Qed.
+
+Lemma get_ctxS_cat sP te R s A:
+  R + get_ctxS sP te (R + s) A = R + get_ctxS sP te s A.
+Proof.
+  elim: A R s => //=; only 1, 2, 3, 4, 5: by move=> *; rewrite catfA catf_refl.
+    by move=> A HA s B HB R s1; rewrite !(fun_if (fun x => R + x)) HA//.
+  move=> A HA B0 HB0 B HB R s; rewrite !(fun_if (fun x => R + x)) HA//.
+  by rewrite -HB HA HB//.
+Qed.
+
+Lemma get_ctxS_cat1 sP te X A:
+  get_ctxS sP te X A = X \/
+    forall X Y, get_ctxS sP te X A = get_ctxS sP te Y A.
+Proof.
+  elim: A X => //=; auto; first by move=> *; case:ifP; auto.
+  move=> A HA B0 HB0 B HB X.
+  case:ifP => sA; last by auto.
+  case: (HB (get_ctxS sP te X A)); last by auto.
+  move=>H; rewrite H.
+  case: (HA X); auto => H1.
+  right => ??; f_equal; auto.
+Qed.
+
+Lemma get_ctxS_cat2 sP te X Y A:
+  (get_ctxS sP te X A = X /\ get_ctxS sP te Y A = Y) \/
+    forall X Y, get_ctxS sP te X A = get_ctxS sP te Y A.
+Proof.
+  elim: A X Y => //=; auto; first by move=> *; case:ifP; auto.
+  move=> A HA B0 HB0 B HB X Y.
+  case:ifP => sA; last by auto.
+  case: (HB (get_ctxS sP te X A) (get_ctxS sP te Y A)); last by auto.
+  move=> [H1 H2]; rewrite H1 H2.
+  case: (HA X Y); auto => H3.
+  right => ??; f_equal; auto.
+Qed.
+
+Definition complete_sig (pref old:sigV) := all_weak pref && (domf pref `&` domf old == fset0).
+
+Lemma tc_cat_comm R K:
+  complete_sig R K -> R + K = K + R.
+Proof.
+  move=> /andP[_ /eqP /fsetP H].
+  apply/fmapP => x; rewrite 2!lookup_cat.
+  (do 2 case: fndP) => //=kK kR.
+  move: (H x).
+  by rewrite in_fsetI kK kR in_fset0.
+Qed.
+
+Lemma catf_refl1 (A s: sigV):
+  (s + A + A) = (s + A).
+Proof. by rewrite -catfA catf_refl. Qed.
+
+Lemma tc_tree_aux_catRx sP A d R K s:
+  complete_sig R K ->
+  tc_tree_aux sP A (R + K) (d, R + s) =
+  tc_tree_aux sP A (R + K) (d, s).
+Proof.
+  elim: A d R s => /=;
+   only 1,2,3,5: by move=> D R s H; rewrite !catfA (tc_cat_comm H) catf_refl1.
+   - by move=> _ c d R s H; rewrite catfA (tc_cat_comm H) catf_refl1.
+   - move=> A HA sm B HB d R s H.
+    rewrite catfA (tc_cat_comm H) catf_refl1 -(tc_cat_comm H) HA//.
+  move=> A HA B0 HB0 B HB d R s H.
+  rewrite catfA (tc_cat_comm H) catf_refl1 -(tc_cat_comm H) HA//.
+  have [] := get_ctxS_cat2 sP (R + K) (R + s) s A.
+    move=> [->->].
+    rewrite (tc_cat_comm H) catfA catf_refl1 -(tc_cat_comm H).
+    repeat case:ifP => //.
+    by rewrite HB//.
+  by move=> /(_ (R+s) s)->.
+Qed.
+
+Lemma tc_tree_aux_catR sP A d R s:
+  tc_tree_aux sP A R (d, R + s) =
+  tc_tree_aux sP A R (d, s).
+Proof.
+  elim: A d R s => //=; only 1, 2, 3, 4, 5: by move=> *; rewrite catfA catf_refl.
+    move=> A HA s B HB d R s0; by rewrite catfA catf_refl HA => //=.
+  move=> A HA B0 HB0 B HB d R s.
+  rewrite -HA -HB !catfA !catf_refl.
+  rewrite get_ctxS_cat.
+  (repeat case: ifP => //) => kB0 kA.
+  by rewrite -HB get_ctxS_cat HB.
+Qed.
+
+Lemma get_ctxS_tcE sP PF O B X C:
+  let N := PF + O in
+  tc sP O B -> tc sP N C ->
+  (get_ctxS sP N X B) = (get_ctxS sP O X B).
+Proof.
+  move=> /= tA tB.
+  elim: B tA tB X => //=.
+    move=> A HA s B HB /tc_orP[tOA tOB tOs] tC X.
+    case:ifP => //=dA; last by auto.
+    rewrite (sigma2ctx_cat1 _ tOA tC tOs); auto.
+  move=> A HA B0 HB0 B HB /tc_andP[tOA tOB0 tOB] tC X.
+  case: ifP => sA; auto.
+  by rewrite HA//=; auto.
+Qed.
+
+Lemma get_ctx_sigma2_ctx sP te s A:
+  get_ctxS sP te (sigma2ctx sP te s) A = sigma2ctx sP te (get_substS s A).
+Proof.
+  elim: A s => //=.
+    move=> A HA smid B HB s; case: ifP => //.
+  move=> A HA B0 HB0 B HB s; case: ifP => //sA; rewrite HA//.
+Qed.
+
+Lemma sigP_success sP tE s O A:
+  sigP sP tE s O ->
+  sigP sP tE (get_substS s A) (get_ctxS sP tE O A).
+Proof.
+  elim: A s O => //=.
+    move=> A HA sB B HB s O H.
+    case:ifP => dA.
+      by rewrite get_ctx_sigma2_ctx; apply: sigP_id.
+    by apply: HA.
+  move=> A HA B0 HB0 B HB s O H.
+  by case:ifP => sA; auto.
+Qed.
+
+Lemma closed_in_var O v : closed_in O (Tm_V v) = (v \in domf O).
+Proof. apply: all_vars_subset_point. Qed.
+
+Lemma closed_in_comb O f a: closed_in O (Tm_Comb f a) = closed_in O f && closed_in O a.
+Proof. apply: all_vars_OR. Qed.
+
+Lemma closed_in_set O a k v:
+  closed_in O a -> closed_in O.[k <- v] a.
+Proof.
+  rewrite/closed_in => /forallP/= H; apply/forallP => -[/=k1 v1].
+  have /= := H (Sub k1 v1).
+  by move=> H1; apply/fset1UP; auto.
+Qed.
+
+Lemma closed_in_assume_tm sP f a xs O:
+  closed_in O a -> closed_in (assume_tm sP O f xs) a.
+Proof.
+  elim: f a xs O => //=[_ _ []//|_ _ []//|v t [|[[] S] _]//|].
+    move=> O cO; case: fndP => //=vO; case: ifP => // _.
+    by rewrite closed_in_set.
+  move=> f Hf a Ha t [|[[] S] xs]//= O CO; case:ifP => //=fh; auto.
+Qed.
+
+Lemma assume_term_cat O1 O2 sP T s :
+  closed_in O1 T ->
+  assume_tm sP (O2 + O1) T s = O2 + assume_tm sP O1 T s.
+Proof.
+  elim: T O1 O2 s => [???[]|???[]|v O1 O2 [|[[] s] xs]|] //.
+    rewrite /assume_tm lookup_cat closed_in_var => CI.
+    rewrite CI (in_fnd CI) /=.
+    by case: ifP => //; rewrite catf_setr.
+  move=> f Hf a Ha O1 O2 [|[m s] xs] //=; rewrite closed_in_comb =>  /andP[cF cA].
+  rewrite Hf // Ha ?closed_in_assume_tm //.
+  by repeat case: ifP => //.
+Qed.
+
+Lemma get_tm_hd_in T v : get_tm_hd T = inr (inr v) -> v \in vars_tm T.
+  elim: T => //=.
+    by move=> ? [->]; rewrite in_fset1.
+  by move=> f Hf ?? /= /Hf; rewrite in_fsetU => ->.
+Qed.
+
+Lemma check_callable_cat {sP T O1 O2 d0 d1 d2 N1 N2}:
+  closed_in O1 (Callable2Tm T) ->
+  check_callable sP O1 T d0 = (d1, N1) ->
+  check_callable sP (O2+O1) T d0 = (d2, N2) ->
+  ((d1 = d2) * (N2 = O2+N1)).
+Proof.
+  rewrite/check_callable => C.
+  rewrite change_only_in_tm_ck_tm_ //.
+  case: check_tm => -[[|d]|[] ? ?] [|]; only 1,2,4-8: by move=> [<- <-] [<- <-].
+  rewrite /get_callable_hd_sig/get_tm_hd_sig.
+  have [[k|v] H] := get_tm_hd_callable T; rewrite H.
+    have [kP|nkP] := fndP; move=> [<- <-] [<- <-]; split => //.
+    by rewrite [assume_call _ _ _ _]assume_term_cat.
+  have vP := forallP C (Sub v (get_tm_hd_in H)).
+  rewrite in_fnd /= lookup_cat vP /= in_fnd.
+  move=> [<- <-] [<- <-]; split => //.
+  by rewrite [assume_call _ _ _ _]assume_term_cat.
+Qed.
+
+Lemma closed_in_sub A B t : domf A `<=` domf B -> closed_in A t -> closed_in B t.
+  rewrite/closed_in.
+  move=> dA /forallP/= H; apply/forallP => /= x; have {}H := H x.
+  by apply: fsubsetP H.
+Qed.
+
+Lemma closed_in_cat R X c: closed_in R c -> closed_in (R + X) c.
+Proof. by apply: closed_in_sub; rewrite domf_cat fsubsetUl. Qed.
+
+Ltac mv_sbst_catfA := move=> [??][??]; subst; try rewrite catfA.
+
+
+Lemma merge_sig_cat O A B :
+  domf A = domf B ->
+  merge_sig (O + A) (O + B) = O + merge_sig A B.
+Proof.
+  move=> H.
+  apply/fmapP => k.
+  have [kO|/negPf nkO] := (boolP (k \in domf O)).
+    have kOA: k \in domf (O + A) by rewrite mem_catf kO.
+    have kOB: k \in domf (O + B) by rewrite mem_catf kO.
+    have kOAB: k \in domf (O + merge_sig A B) by rewrite mem_catf kO.
+    rewrite merge_sigLR in_fnd.
+    have [kA|nkA] := (boolP (k \in domf A)).
+    - have kB: k \in domf B by rewrite -H.
+      have kAB: k \in domf (merge_sig A B) by rewrite merge_sig_domf in_fsetU kA.
+      by rewrite !getf_catr (fnd_in kAB) merge_sigLR//=.
+    have nkB: k \notin domf B by rewrite -H.
+    have kAB: k \notin domf (merge_sig A B) by rewrite merge_sig_domf in_fsetU (negPf nkA).
+    by rewrite !getf_catl// max_refl.
+  have [kA|/negPf nkA] := (boolP (k \in domf A)).
+    have kB: k \in domf B by rewrite -H.
+    have kAB: k \in domf (merge_sig A B) by rewrite merge_sig_domf in_fsetU kA.
+    have kOA: k \in domf (O + A) by rewrite mem_catf kA orbT.
+    have kOB: k \in domf (O + B) by rewrite mem_catf kB orbT.
+    have kOAB: k \in domf (O + merge_sig A B) by rewrite mem_catf kAB orbT.
+    rewrite merge_sigLR in_fnd.
+    rewrite !getf_catr (fnd_in kAB) merge_sigLR//.
+  have nkB: k \in domf B = false by rewrite -H.
+  have kOAB: k \notin domf (merge_sig (O + A) (O + B)) by rewrite merge_sig_domf !domf_cat !in_fsetU nkA nkB nkO.
+  have kOAB': k \notin domf (O + merge_sig A B) by rewrite !domf_cat !in_fsetU nkO nkA nkB.
+  by rewrite !not_fnd//.
+Qed.
+
+Lemma merge_sig_cat1 O A B :
+  all_weak O ->
+  compat_sig A O ->
+  compat_sig B O ->
+  merge_sig (O + A) (O + B) = O + merge_sig A B.
+Proof.
+  move=> wO cAO cBO.
+  apply/fmapP => k.
+  have [kO|/negPf nkO] := (boolP (k \in domf O)); last first.
+    case: (fndP A k) => kA.
+      have kAB : k \in domf (merge_sig A B) by rewrite merge_sig_domf in_fsetU kA.
+      have kOAOB : k \in domf (merge_sig (O + A) (O + B)).
+        by rewrite merge_sig_domf !domf_cat !in_fsetU kA !orbT.
+      rewrite lookup_cat kAB.
+      case: (fndP B k) => kB.
+        rewrite merge_sigLR; only 1, 2: by rewrite domf_cat in_fsetU (kA, kB) orbT.
+        move=> kOA kOB.
+        rewrite fnd_in lookup_cat kA (in_fnd kA).
+        rewrite (fnd_in kOB) lookup_cat kB (in_fnd kB).
+        by rewrite merge_sigLR//=.
+      rewrite !merge_sigL//; only 2, 3: by rewrite domf_cat in_fsetU nkO//.
+      by rewrite lookup_cat kA//.
+    case: (fndP B k) => kB.
+      rewrite lookup_cat .
+      have kAB : k \in domf (merge_sig A B) by rewrite merge_sig_domf in_fsetU kB orbT.
+      rewrite kAB.
+      rewrite !merge_sigR//; only 2, 3: by rewrite domf_cat in_fsetU nkO//.
+      by rewrite lookup_cat kB/=.
+    rewrite merge_sig_None//; only 2, 3: by rewrite domf_cat in_fsetU nkO//.
+    rewrite lookup_cat merge_sig_None//.
+    by rewrite not_fnd// ?if_same//nkO.
+  rewrite !in_fnd; only 1,2: by rewrite !(domf_cat, merge_sig_domf) !in_fsetU kO.
+  move=> kOAB kOAOB.
+  rewrite fnd_in merge_sigLR; only 1,2: by rewrite domf_cat in_fsetU kO.
+  move=> kOA kOB.
+  have := forallP wO (Sub k kO); rewrite valPE => /eqP H.
+  rewrite (fnd_in kOAB) lookup_cat.
+  rewrite (fnd_in kOA) (fnd_in kOB) !lookup_cat in_fnd.
+  case: (fndP A k) => kA.
+    have kAB: k \in domf (merge_sig A B) by rewrite merge_sig_domf in_fsetU kA.
+    rewrite kAB.
+    case: (fndP B k) => kB; first by rewrite merge_sigLR//.
+    rewrite merge_sigL// !in_fnd/=.
+    have := forallP cAO (Sub k kO); rewrite valPE/= in_fnd/= => {}cAO.
+    rewrite H.
+    move: (cAO) => /comp_weak ->.
+    rewrite max_weak//.
+  case: (fndP B k) => kB.
+    rewrite merge_sigR// in_fnd.
+    have kAB: k \in domf (merge_sig A B) by rewrite merge_sig_domf in_fsetU kB orbT.
+    rewrite kAB/=.
+    have := forallP cBO (Sub k kO); rewrite valPE/= in_fnd/= => {}cBO.
+    rewrite H.
+    move: (cBO) => /comp_weak ->.
+    rewrite max_comm max_weak//.
+  have kAB: k \notin domf (merge_sig A B) by rewrite merge_sig_domf in_fsetU (negPf kA) (negPf kB).
+  by rewrite merge_sig_None// kAB/= max_refl.
+Qed.
+
+Lemma compat_subst_sub sP tyO s:
+  compat_subst sP tyO s ->
+  domf (sigma2ctx sP tyO s) `<=` domf tyO.
+Proof.
+  move=>/andP[/forallP/= H1 /forallP/= H2].
+  apply/fsubsetP => k kS.
+  have ks : k \in vars_sigma s by rewrite/vars_sigma in_fsetU kS.
+  by have:= H1 (Sub k ks) => /=.
+Qed.
+
+Lemma compat_subst_compat_sig sP tyO s:
+  compat_subst sP tyO s ->
+  compat_sig (sigma2ctx sP tyO s) tyO.
+Proof.
+  move=>/andP[/forallP/= H1 /forallP/= H2].
+  apply/forallP => -[k kO]; rewrite valPE [val _]/=.
+  case: fndP => // kO'; rewrite ffunE/=valPE.
+  case C: check_tm => [S B].
+  suffices : compat_type tyO.[kO] S.
+    by destruct B => //; rewrite compat_type_weak//.
+  have:= H2 (Sub k kO'); rewrite valPE/= in_fnd C/=.
+  by rewrite compat_type_comm.
+Qed.
+
+(* Lemma merge_sig_cat_help sP X tyO B RR DB' sB:
+  complete_sig X tyO ->
+  tc sP (X + tyO) B ->
+  tc_tree_aux sP B (X + tyO) RR = (DB', X + SB) ->
+  tc_tree_aux sP B tyO RR = (DB', SB) ->
+  merge_sig (X + SA) (X + SB) = X + merge_sig SA SB
+. *)
+
+Lemma tc_cat_weakL X ty : complete_sig X ty -> all_weak X.
+Proof. by move=> /andP[]. Qed.
+
+Lemma compat_sig_catL_id A K:
+  compat_sig A K -> compat_sig (K + A) K.
+Proof.
+  move=> /forallP H; apply/forallP=>-[k kP].
+  rewrite valPE lookup_cat/= in_fnd.
+  case: fndP => //= kA.
+  have:= H (Sub k kP); rewrite valPE/= in_fnd//.
+Qed.
+
+Lemma fsubset_catL_id s0 (tyO:sigV):
+  domf s0 `<=` domf tyO -> domf (tyO + s0) `<=` domf tyO .
+Proof. by rewrite domf_cat fsubUset fsubset_refl. Qed.
+
+Lemma compat_sig_merge_sig sA sB tyO:
+  compat_sig sA tyO -> compat_sig sB tyO ->
+  compat_sig (merge_sig sA sB) tyO.
+Proof.
+  move=> cAO cBO.
+  apply/forallP => -[k kO]; rewrite valPE [val _]/=.
+  case: (fndP sA k) => kA; case: (fndP sB k) => kB.
+  - have := forallP cAO (Sub k kO); rewrite valPE [val _]/= in_fnd [odflt _ _]/= => cOA.
+    have := forallP cBO (Sub k kO); rewrite valPE [val _]/= in_fnd [odflt _ _]/= => cOB.
+    rewrite merge_sigLR//= -(@max_refl tyO.[kO]).
+    by apply: compat_type_max => //; apply: compat_type_comm1.
+  - have := forallP cAO (Sub k kO); rewrite valPE [val _]/= in_fnd [odflt _ _]/= => cOA.
+    rewrite merge_sigL// in_fnd/= compat_type_weak//.
+  - have := forallP cBO (Sub k kO); rewrite valPE [val _]/= in_fnd [odflt _ _]/= => cOB.
+    rewrite merge_sigR// in_fnd/= compat_type_weak//.
+  - rewrite merge_sig_None//.
+Qed.
+
+Lemma compat_subst_get_substS sP tyO s A:
+  compat_subst sP tyO s -> tc sP tyO A ->
+  compat_subst sP tyO (get_substS s A).
+Proof. by elim: A s => //=[???????/tc_orP[]|????????/tc_andP[]]*; case:ifP; auto. Qed.
+
+Lemma get_substS_domf sP tyO s A: 
+  domf s `<=` domf tyO ->
+  compat_subst sP tyO s -> tc sP tyO A ->
+  domf (get_substS s A) `<=` domf tyO.
+Proof.
+  elim: A s => //=.
+    move=> A HA sm B HB s H CS /tc_orP[tA tB ts].
+    have:= compat_subst_sub ts.
+    by case: ifP; auto.
+  move=> A HA B0 HB0 B HB s H CS /tc_andP[tA tB0 tB].
+  case:ifP => _; last by auto.
+  apply: HB; auto.
+  by apply: compat_subst_get_substS.
+Qed.
+
+Lemma compat_subst_domf sP tyO sm:
+  compat_subst sP tyO sm -> domf sm `<=` domf tyO.
+Proof.
+  rewrite /compat_subst/all_vars_subset/vars_sigma.
+  move=>/andP[/forallP H _].
+  apply/fsubsetP => x xs.
+  have xx : x \in (domf sm `|` codom_vars sm) by rewrite in_fsetU xs.
+  by have:= H (Sub x xx).
+Qed.
+
+Lemma get_ctxS_domf sP tyO s A: 
+  tc sP tyO A -> domf s `<=` domf tyO ->
+  domf (get_ctxS sP tyO s A) `<=` domf tyO.
+Proof.
+  elim: A s => //=.
+    move=> A HA sm B HB s /tc_orP[tA tB ts] H.
+    case: ifP => _; last by auto.
+    rewrite get_ctx_sigma2_ctx sigma2ctx_domf.
+    apply: get_substS_domf tB; auto.
+    apply: compat_subst_domf ts.
+  move=> A HA B0 HB0 B HB s /tc_andP[tA tB0 tB] d.
+  by case: ifP => _; auto.
+Qed.
+
+Lemma domf_set_in {K: countType} {V: eqType} (k:K) (v:V) O:
+  k \in domf O -> domf O.[k <- v] = domf O.
+Proof.
+  move=> H.
+  apply/fsetP => [x].
+  rewrite in_fset1U.
+  case: eqP => //?; subst.
+  by rewrite H orbT.
+Qed.
+
+Lemma closed_in_tmE O f a:
+  closed_in O (Tm_Comb f a) = closed_in O f && closed_in O a.
+Proof.
+  apply/forallP; case:ifP => /=.
+    move=> /andP[cf ca] -[x]/=.
+    rewrite in_fsetU => /orP[]H.
+      apply: forallP cf (Sub x H).
+    apply: forallP ca (Sub x H).
+  apply: contraFnot => H.
+  apply/andP; split; apply/forallP => -[x xP]/=;
+  (have xfA: x \in vars_tm f `|` vars_tm a by rewrite in_fsetU xP?orbT);
+  apply: H (Sub x xfA).
+Qed.
+
+Lemma closed_in_tmP O f a:
+  closed_in O (Tm_Comb f a) <-> closed_in O f /\ closed_in O a.
+Proof.
+  rewrite closed_in_tmE; split.
+    by move=> /andP.
+  by move=> [->->].
+Qed.
+
+Lemma assume_call_domf sP O T S:
+  closed_in O T ->
+  domf (assume_tm sP O T S) = domf O.
+Proof.
+  elim: T O S => //=; only 1, 2: by move=> ?? [].
+    move=> v O [|[[] S] _]// /[!closed_in_var] vO.
+    rewrite in_fnd//=; case: ifP => // _.
+    rewrite domf_set_in//.
+  move=> f Hf a Ha O [|[m s] xs]///closed_in_tmP[cf ca].
+  case:ifP => //=fh; case: m => /=; last by auto.
+  rewrite Ha; auto.
+  by apply: closed_in_assume_tm.
+Qed.
+
+Lemma check_callable_domf {O N T sP d0 dA}:
+  closed_in O (Callable2Tm T) ->
+  check_callable sP O T d0 = (dA, N) -> domf N = domf O.
+Proof.
+  move=> H.
+  rewrite/check_callable.
+  case CT: check_tm => [[[|D]|] B]//; only 1,3: congruence.
+  destruct B; last by congruence.
+  case X: get_callable_hd_sig => [S|]; last by congruence.
+  move=> [_ <-].
+  by apply: assume_call_domf.
+Qed.
+
+(* Lemma check_callable_domf {O N T sP d0 dA}:
+  closed_in O (Callable2Tm T) ->
+  check_callable sP O T d0 = (dA, N) -> 
+  compat_sig N O.
+Proof.
+
+  move=> H.
+  rewrite/check_callable.
+  case CT: check_tm => [[[|D]|] B]//; only 1,3: congruence.
+  destruct B; last by congruence.
+  case X: get_callable_hd_sig => [S|]; last by congruence.
+  move=> [_ <-].
+  by apply: assume_call_domf.
+Qed. *)
+
+Lemma tc_tree_aux_sub sP tyO B d0 s0 d1 s1:
+  domf s0 `<=` domf tyO -> tc sP tyO B ->
+  tc_tree_aux sP B tyO (d0, s0) = (d1, s1) ->
+    domf s1 `<=` domf tyO.
+Proof.
+  elim: B d0 s0 d1 s1 => //=;
+  only 1, 2, 3, 5: by move=> d0 s0 d1 s1 H1 H2 [??]; subst; rewrite fsubset_catL_id// compat_sig_catL_id//.
+  - move=> p c d0 s0 d1 s1 H1 H2; case C: check_callable => [d2 s2][??]; subst.
+    rewrite (check_callable_domf _ C).
+      by rewrite fsubset_catL_id.
+    apply: closed_in_cat.
+    by move/and3P: H2 => [].
+  - move=> A HA s B HB d0 s0 d1 s1 H1 /tc_orP[tOA tOB tOs].
+    case kA: is_ko => /=.
+      case kB: is_ko => /=.
+        by move=> [_ <-]; rewrite fsubset_catL_id//.
+      apply: HB (compat_subst_sub tOs) tOB.
+    case kB: is_ko => /=; first by apply: HA.
+    case tA: tc_tree_aux => [dA sA].
+    case tB: tc_tree_aux => [dB sB].
+    have {}HA := HA _ _ _ _ H1 tOA tA.
+    have {}HB := HB _ _ _ _ (compat_subst_sub tOs) tOB tB.
+    by move=> [_ <-]; rewrite merge_sig_domf fsubUset HA HB.
+  - move=> A HA B0 HB0 B HB d0 s0 d1 s1 H /tc_andP[tOA tOB0 tOB].
+    case: ifP => kA; first by move=> [_<-]; rewrite fsubset_catL_id//.
+    case: ifP => kB0.
+      case:ifP => sA.
+        apply: HB tOB; rewrite fsubset_catL_id//.
+        by apply: get_ctxS_domf.
+      by move=> [_<-]; rewrite fsubset_catL_id//.
+    case tA: tc_tree_aux => [dA sA].
+    case tB0: tc_tree_aux => [dB0 sB0].
+    case tB: tc_tree_aux => [dB sB].
+    have {}HA := HA _ _ _ _ H tOA tA.
+    have {}HB := HB _ _ _ _ (get_ctxS_domf tOA H) tOB tB.
+    have {}HB0 := HB0 _ _ _ _ HA tOB0 tB0.
+    case: ifP => SA [??]; subst; last by [].
+    by rewrite merge_sig_domf fsubUset HB HB0.
+Qed.
+
+Lemma compat_sig_get_ctxS sP tyO s0 A:
+  compat_sig s0 tyO -> 
+  tc sP tyO A ->
+  compat_sig (get_ctxS sP tyO s0 A) tyO.
+Proof.
+  elim: A s0 => //.
+    move=> A HA sm B HB s C /tc_orP[tOA tOB tOs]/=.
+    rewrite get_ctx_sigma2_ctx.
+    case:ifP; last by auto.
+    rewrite compat_subst_compat_sig//.
+    rewrite compat_subst_get_substS//.
+  move=> A HA B0 HB0 B HB s H /tc_andP[tA tB0 tB]/=.
+  case: ifP; auto => sA.
+Qed.
+
+Lemma complete_sig_comm s1 tyO:
+  all_weak tyO ->
+  complete_sig s1 tyO -> complete_sig tyO s1.
+Proof.
+  move=> H1 /andP[H2/eqP H3].
+  rewrite /complete_sig H1/=-H3.
+  by rewrite fsetIC.
+Qed.
+
+Lemma compat_sig_comm A B:
+  compat_sig A B = compat_sig B A.
+Proof.
+  apply/forallP => /=; case: ifP.
+    move=> cBA [k kB]; rewrite valPE/=.
+    case: fndP => // kA.
+    have:= forallP cBA (Sub k kA).
+    by rewrite valPE in_fnd/= compat_type_comm.
+  apply: contraFnot => H.
+  apply/forallP => -[k kA]; rewrite valPE/=.
+  case: fndP => //=kB.
+  by have:= H (Sub k kB); rewrite valPE/= in_fnd compat_type_comm.
+Qed.
+
+Lemma tc_tree_aux_compat_sig sP tyO B d0 s0 d1 s1:
+  compat_sig s0 tyO -> tc sP tyO B ->
+  tc_tree_aux sP B tyO (d0, s0) = (d1, s1) ->
+    compat_sig s1 tyO.
+Proof.
+  elim: B d0 s0 d1 s1 => //=;
+  only 1, 2, 3, 5: by move=> d0 s0 d1 s1 H1 H2 [??]; subst; rewrite compat_sig_catL_id//.
+  - move=> p c d0 s0 d1 s1 H1 H2; case C: check_callable => [d2 s2][??]; subst.
+    case C1 : (check_callable sP tyO c d0) => [d3 s3].
+    (* rewrite tc_cat_comm// in C; last first.  *)
+    admit.
+  - move=> A HA s B HB d0 s0 d1 s1 H1 /tc_orP[tOA tOB tOs].
+    case kA: is_ko => /=.
+      case kB: is_ko => /=.
+        by move=> [_ <-]; rewrite compat_sig_catL_id//.
+      apply: HB (compat_subst_compat_sig tOs) tOB.
+    case kB: is_ko => /=; first by apply: HA.
+    case tA: tc_tree_aux => [dA sA].
+    case tB: tc_tree_aux => [dB sB].
+    have {}HA := HA _ _ _ _ H1 tOA tA.
+    have {}HB := HB _ _ _ _ (compat_subst_compat_sig tOs) tOB tB.
+    move=> [_ <-]; rewrite compat_sig_merge_sig//.
+  - move=> A HA B0 HB0 B HB d0 s0 d1 s1 H1 /tc_andP[tOA tOB0 tOB].
+    case:ifP => kA.
+      by move=> [_<-]; rewrite compat_sig_catL_id//.
+    rewrite tc_tree_aux_catR.
+    case tB: tc_tree_aux => [dB sB].
+    case tA: tc_tree_aux => [dA sA].
+    case tB0: tc_tree_aux => [dB0 sB0].
+    have {}HA := HA _ _ _ _ H1 tOA tA.
+    have {}HB := HB _ _ _ _ (compat_sig_get_ctxS H1 tOA) tOB tB.
+    have {}HB0 := HB0 _ _ _ _ HA tOB0 tB0.
+    case: ifP => kB0; case: ifP => SA [_ <-]; auto.
+      by rewrite compat_sig_catL_id//.
+    by rewrite compat_sig_merge_sig//.
+Admitted.
+
+Lemma tc_tree_aux_cat sP A tyO X d0 s0 d1 d2 N1 N2:
+  complete_sig X tyO ->
+  let tyN := X + tyO in
+  tc sP tyO A -> tc sP tyN A ->
+  domf s0 `<=` domf tyO ->
+  compat_sig s0 tyO ->
+  valid_tree A ->
+  tc_tree_aux sP A tyO (d0,s0) = (d1, N1) ->
+  tc_tree_aux sP A tyN (d0,s0) = (d2, N2) ->
+  ((d1 = d2) * (N2 = X + N1)).
+Proof.
+  move=> /=CM.
+  elim: A d0 s0 d1 d2 N1 N2; 
+    only 1,2,3,5: by move=> > ?????/=; mv_sbst_catfA.
+  - move=> p c d0 s0 d1 d2 N1 N2 tO tN DR CS _ /=.
+    case c1: check_callable => [D1 S1].
+    case c2: check_callable => [D2 S2].
+    mv_sbst_catfA; rewrite -catfA in c2.
+    suffices C : closed_in (tyO + s0) (Callable2Tm c).
+      by rewrite !(check_callable_cat C c1 c2).
+    by move/and3P: tO => [???]; apply/closed_in_cat.
+  - move=> A HA s B HB d0 s0 d1 d2 N1 N2 ++ DR CS.
+    move=> /tc_orP[tOA tOB tOs] /tc_orP[tNA tNB tNs]/=.
+    rewrite (sigma2ctx_cat1 _ tOA tNA tOs).
+    case kA: is_ko => /=.
+      case kB: is_ko; first by move=> _; mv_sbst_catfA.
+      move=> H; apply: HB; auto.
+        rewrite compat_subst_sub//=.
+        rewrite compat_subst_compat_sig//.
+      by move: H; case:ifP => // _ /andP[_ /bbOr_valid].
+    rewrite (contraFF is_dead_is_ko kA) => /andP[vA bB].
+    case kB: is_ko => /=; first by eauto.
+    case tA: tc_tree_aux => [DA SA].
+    case tB: tc_tree_aux => [DB SB].
+    case tA': tc_tree_aux => [DA' SA'].
+    case tB': tc_tree_aux => [DB' SB']/=.
+    have [??] := HA _ _ _ _ _ _ tOA tNA DR CS vA tA tA'.
+    have [??] := HB _ _ _ _ _ _ tOB tNB (compat_subst_sub tOs) (compat_subst_compat_sig tOs) (bbOr_valid bB) tB tB'.
+    subst. 
+    suffices sax : compat_sig SA X.
+    suffices sbx: compat_sig SB X.
+    by case:ifP => cA; mv_sbst_catfA; (split; first by []); apply:merge_sig_cat1 (andP CM).1 _ _.
+      have CSB := tc_tree_aux_compat_sig (compat_subst_compat_sig tOs) tOB tB.
+      have DBO := tc_tree_aux_sub (compat_subst_sub tOs) tOB tB.
+      admit.
+    have CSA := tc_tree_aux_compat_sig CS tOA tA.
+    have DAO := tc_tree_aux_sub DR tOA tA.
+    admit.
+  - move=> A HA B0 HB0 B HB d0 s0 d1 d2 N1 N2 ++ DR CS.
+    move=> /tc_andP[tOA tOB0 tOB] /tc_andP[tNA tNB0 tNB] /=/and4P[vA].
+    rewrite (get_ctxS_tcE _ tOA tNA) !tc_tree_aux_catR/=.
+    case:ifP => /=[sA vB bB ckB|sA /eqP-> + _].
+      rewrite success_is_ko//=.
+      case:ifP => kB0.
+        apply: HB; auto.
+          apply: get_ctxS_domf; auto.
+        apply: compat_sig_get_ctxS; auto.
+      case tA: (tc_tree_aux _ A) => [DA SA].
+      case tB0: (tc_tree_aux _ B0) => [DB0 SB0].
+      case tB: (tc_tree_aux _ B) => [DB SB].
+      case tA': (tc_tree_aux _ A) => [DA' SA'].
+      case tB0': (tc_tree_aux _ B0) => [DB0' SB0'].
+      case tB': (tc_tree_aux _ B) => [DB' SB'].
+      mv_sbst_catfA.
+      have {HA} [??] := HA _ _ _ _ _ _ tOA tNA DR CS vA tA tA'.
+      have {HB }  := HB _ _ _ _ _ _ tOB tNB _ _ vB tB tB'.
+      move=> [||??]; subst.
+        apply: get_ctxS_domf; auto.
+        apply: compat_sig_get_ctxS; auto.
+      rewrite tc_tree_aux_catRx// in tB0'.
+      have := HB0 _ _ _ _ _ _ tOB0 tNB0 _ _ (bbAnd_valid bB) tB0 tB0'.
+      move=> [||??]; subst.
+        by apply: tc_tree_aux_sub tA; auto.
+        by apply: tc_tree_aux_compat_sig tA; auto.
+      subst; split; first by [].
+      apply: merge_sig_cat1; admit.
+    case kA: is_ko => /=; first by move=> _; mv_sbst_catfA.
+    case kB: is_ko => /=; first by move=> _; mv_sbst_catfA.
+    case tA: (tc_tree_aux _ A) => [DA SA].
+    case tB: (tc_tree_aux _ B) => [DB SB].
+    case tA': (tc_tree_aux _ A) => [DA' SA'].
+    case tB': (tc_tree_aux _ B) => [DB' SB'].
+    move=> vB [??][??]; subst.
+    have [??] := HA _ _ _ _ _ _ tOA tNA DR CS vA tA tA'.
+    have {}vB: valid_tree B by move: vB; case:ifP => [_ /bbAnd_valid|_ /base_and_valid].
+    subst.
+    rewrite tc_tree_aux_catRx// in tB'.
+    have := HB _ _ _ _ _ _ tOB tNB _ _ vB tB tB'.
+    move=> [||??/[subst]]//.
+      by apply: tc_tree_aux_sub tA; auto.
+    by apply: tc_tree_aux_compat_sig tA; auto.
+Admitted.
+
+Lemma tc_tree_aux_cat1 sP A tyO X d0 s0 d1 d2 N1 N2:
+  complete_sig X tyO ->
+  let tyN := X + tyO in
+  tc sP tyO A -> tc sP tyN A ->
+  domf s0 `<=` domf tyO ->
+  compat_sig s0 tyO ->
+  valid_tree A ->
+  tc_tree_aux sP A tyO (d0,s0) = (d1, N1) ->
+  tc_tree_aux sP A tyN (d0,s0) = (d2, N2) ->
+  ((d2 = d1)).
+Proof.
+  move=>/= H1 H2 H3 H4 H5 H6 H7 H8.
+  by rewrite (tc_tree_aux_cat H1 H2 H3 H4 H5 H6 H7 H8).
+Qed.
+
+Definition incl_sig (N O:sigV) :=
+  [forall x: domf O, incl (odflt O.[valP x] N.[?val x]) O.[valP x]].
+
+Lemma compat_sig_refl O: compat_sig O O.
+Proof. by apply/forallP => -[k v]; rewrite valPE in_fnd//. Qed.
+
+(* tells if big is more precise then smal; *)
+(* e.g. big has more mapping then small, and/or the mappings have less holes *)
+Definition more_precise (new old: sigV) : bool :=
+  [&& (domf old `<=` domf new), compat_sig new old & incl_sig new old].
+
+Lemma tc_tree_aux_step u sP tyO X A r s1 O N1 N2 d:
+  complete_sig X tyO ->
+  let tyN := X + tyO in
+
+  valid_tree A ->
+  step u s1 A = r ->
+
+  forall (tcO : tc sP tyO A)
+         (tcN : tc sP tyN (get_tree r)),
+  domf O `<=` domf tyO ->
+  compat_sig O tyO ->
+
+  sigP sP tyO s1 O ->
+
+  tc_tree_aux sP A tyO (Func, O) = (Func, N1) ->
+  tc_tree_aux sP (get_tree r) tyN (Func, O) = (d, N2) ->
+  ((d = Func)).
+Proof.
+  move=> CM/=.
+  elim: A r s1 O N1 N2 d;
+  only 1, 2, 3, 5: by move=> r s1 O N1 N2 d t <-/=; congruence.
+  - move=> p c r s1 O N1 N2 d _ <-/= tcO tcN DR CS sO.
+    case C: check_callable => [D S][??] H; subst.
+    admit.
+  - move=> A HA s B HB r s1 O N1 N2 d/= + <-{r} /tc_orP[tOA tOB tOs]+DR CS H.
+    case: (boolP (is_dead _)) => [dA vB|dA /andP[vA bB]].
+      rewrite get_tree_Or/= is_dead_is_ko//= => /tc_orP[tNA + tNs].
+      case: ifP => kB; first by rewrite is_ko_step//=kB; congruence.
+      case tB: tc_tree_aux => [DB SB] tNB [??]; subst.
+      rewrite sigma2ctx_cat//=.
+      case tB': tc_tree_aux => [DB' SB'].
+      have ? := HB _ _ _ _ _ _ vB erefl tOB tNB (compat_subst_sub tOs) (compat_subst_compat_sig tOs) (sigP_id _ _ _) tB tB'; subst.
+      by case:ifP => k [??]; subst; auto.
+    case kA: is_ko; first (rewrite is_ko_step//=kA/=; case: ifP; first congruence).
+      move=> kB /tc_orP[tNA tNB tNs].
+      rewrite (sigma2ctx_cat1 _ tOA tNA)//.
+      apply: tc_tree_aux_cat1; auto.
+        by apply/compat_subst_sub.
+        by apply/compat_subst_compat_sig.
+      by apply/bbOr_valid.
+    case: ifP => kB.
+      by case eA: step => [A'|A'|A'|A']/=; rewrite !(is_ko_cutr,kB, andbT);
+      (case kA': is_ko; [by congruence | ]) => /tc_orP[tNA tNB tNs];
+      apply: HA eA _ _ _ _ _; auto.
+    case: ifP => cutA; last by [].
+    case tA: tc_tree_aux => [DA SA].
+    case tB: tc_tree_aux => [DB SB]/=.
+    destruct DA, DB => //= + [?]; subst.
+    case eA: step => [A'|A'|A'|A']/=; 
+    rewrite !(is_ko_cutr,kB, andbT,andbF) => /tc_orP[tNA tNB tNs];
+    rewrite (sigma2ctx_cat1 _ tOA tNA)//;
+    case tB': tc_tree_aux => [DB' SB']/=;
+    case tA': tc_tree_aux => [DA' SA']/=;
+    have {HA}? := HA _ _ _ _ _ _ vA eA tOA tNA DR CS H tA tA'; subst;
+    cycle 1;
+      [|rewrite (step_keep_cut eA isT) cutA/= -fun_if => -[??]; subst;
+        have ? := compat_subst_sub tOs;
+        have ? := compat_subst_compat_sig tOs;
+        by apply: tc_tree_aux_cat1 (bbOr_valid bB) tB tB'; auto
+      ..].
+    by case kA' :is_ko => -[??]; subst => //.
+  - move=> A HA B0 HB0 B HB r s O N1 N2 d /= /and4P[vA++cK]<-{r} /tc_andP[tOA tOBO tOB] + DR CS SP.
+    case kA: is_ko.
+      rewrite is_ko_success//=is_ko_failed//=is_ko_step//=kA.
+      by move=> /eqP -> bB /tc_andP[tNA tNB _] [?][<-].
+    case: ifP => /=[sA vB bB0|sA /eqP->].
+      rewrite succes_is_solved//.
+      case:ifP => kB0.
+        rewrite !tc_tree_aux_catR get_tree_And; case: ifP.
+          have scA: success (cutl A) by rewrite success_cut.
+          move => + /tc_andP[tNA tNB0 +].
+          case eB: step => //=[B'] _ tB'.
+          rewrite/= success_is_ko//scA is_ko_cutr//=get_ctxS_cutl//=.
+          rewrite tc_tree_aux_catR (get_ctxS_tcE _ tOA tNA)//.
+          apply: HB eB _ _ _ _ _; auto.
+            admit.
+            admit.
+          by apply/sigP_success.
+        case eB: step => [B'|B'|B'|B']//= _ /tc_andP[tNA tNB0 tNB];
+        rewrite kA kB0 sA tc_tree_aux_catR (get_ctxS_tcE _ tOA tNA);
+        apply: HB eB _ _ _ _ _; auto; admit.
+        (* apply/sigP_success. *)
+      case tA: (tc_tree_aux _ A) => [DA SA].
+      case tB0: (tc_tree_aux _ B0) => [DB0 SB0].
+      case tB: (tc_tree_aux _ B) => [DB SB].
+      destruct DB, DB0 => //= + [?]; subst.
+      rewrite get_tree_And/= => /tc_andP[].
+      case:ifP.
+        have scA: success (cutl A) by rewrite success_cut.
+        rewrite success_is_ko//=scA is_ko_cutr.
+        case eB: step => //=[B'] _ tNA tNB0 tNB.
+        rewrite get_ctxS_cutl// tc_tree_aux_catR.
+        rewrite (get_ctxS_tcE _ tOA tNA).
+        apply: HB eB _ _ _ _ _ tB; auto.
+          admit.
+          admit.
+        by apply/sigP_success.
+      rewrite success_is_ko/=sA//= tc_tree_aux_catR kB0.
+      case tA': (tc_tree_aux _ A) => [DA' SA'].
+      case tB0': (tc_tree_aux _ B0) => [DB0' SB0'].
+      move=> + tNA tNB0.
+      rewrite (get_ctxS_tcE _ tOA tNA).
+      case tB': (tc_tree_aux) => [DB' SB'].
+      move=> + tNB.
+      have := HB _ _ _ _ _ _ vB erefl tOB tNB _ _ (sigP_success _ SP) tB tB'; subst.
+      move=> ++ [??]; subst.
+      (* this is a bug *)
+      admit.
+    case:ifP => [fA bB|fA bB].
+      rewrite failed_expand//= failed_success//=.
+      move=> /tc_andP[tNA tNB _].
+      case:ifP => kB; first by case:ifP; congruence.
+      case tA: (tc_tree_aux _ A) => [DA SA].
+      case tA': (tc_tree_aux _ A) => [DA' SA'].
+      case tB: (tc_tree_aux _ B) => [DB SB].
+      case tB': (tc_tree_aux _ B) => [DB' SB'].
+      move=> [??]; subst.
+      rewrite kA => -[??]; subst.
+      (* TODO: use a more generic version of tc_tree_aux_cat1 *)
+      admit.
+    rewrite base_and_is_ko//=.
+    case eA: step => [A'|A'|A'|A']/=; rewrite ?(base_and_is_ko bB); last first.
+    - by rewrite !(expand_solved_same _ eA) in sA.
+    - by rewrite !(expand_failed_same _ eA) in fA.
+    all: move=> /tc_andP[tNA tNB _].
+    all: case: ifP => kA'; first by congruence.
+    all: case tA: (tc_tree_aux _ A) => [DA SA];
+         case tA': (tc_tree_aux _ A') => [DA' SA'];
+         case tB: (tc_tree_aux _ B) => [DB SB];
+         case tB': (tc_tree_aux _ B) => [DB' SB'];
+         case tB2: (tc_tree_aux _ B) => [DB2 SB2].
+    all: move=> [??]; subst.
+      admit.
+    admit.
+    (* - destruct DA. *)
+        (* have ? := HA _ _ _ _ _ _ vA eA tOA tNA SP tA tA'; subst. *)
+Admitted.
+
+Lemma good_assignment_cat sP X tE s1 N:
+    closed_in tE N ->
+    good_assignment sP (X + tE) s1 N = good_assignment sP tE s1 N.
+Proof. by move=> cE; rewrite/good_assignment change_only_in_tm_ck_tm_. Qed.
+
+Lemma sigP_cat sP X tE s1 N:
+    sigP sP tE s1 N ->
+    sigP sP (X + tE) s1 N.
+Proof.
+  move=> H; apply/forallP => -[k kN]; rewrite valPE/=.
+  have:= forallP H (Sub k kN); rewrite valPE/=.
+  case: fndP => // ks1.
+  rewrite good_assignment_cat//.
+  have {H}:= forallP H (Sub k kN); rewrite valPE/= in_fnd.
+  rewrite /good_assignment/=.
+Admitted.
+
+Definition mutual_exclusion :=
+  forall pr S sP O u t s, (get_tm_hd_sig sP O (Callable2Tm t)) = Some S ->
+    get_sig_hd S = d Func ->
+     F u pr t s = [::] \/ (forall PREF LAST, F u pr t s = rcons PREF LAST ->
+        forall s1 x, (s1, x) \in PREF ->
+          seq.head ACut x.(premises) = ACut).
+
+Lemma tc_weak {sP N T} (g: tc sP N T) : all_weak N. 
+Proof. by move/and3P: g => []. Qed.
+
+
+Axiom saturate_sigP : forall sP O A u s r,
+  tc sP O A ->
+  step u s A = r ->
+  { X : sigV | let N := X + O in complete_sig X O && tc sP N (get_tree r) }.
+
+Lemma run_is_det {sP sV sV' s A tE}: 
+  check_program sP tE -> 
+  mutual_exclusion ->
+  tc sP tE A -> valid_tree A ->
+    domf sV `<=` domf tE ->
+    compat_sig sV tE ->
+    sigP sP tE s sV ->
+    tc_tree_aux sP A tE (Func, sV) = (Func, sV') ->
+     forall u s' B n,
+      runb u s A (Some s') B n ->
+        next_alt false B = None /\ sigP sP tE s' sV'.
+Proof.
+  move=> ckP ME ++++++ u s' B n H.
+  remember (Some s') as ss eqn:Hs'.
+  elim: H s' Hs' sV sV' tE ckP; clear - ME => //=.
+  - move=> s1 s2 A B sA <-{s2} <-{B} s' [<-]{s'} sV sV' tE ckP H1 vA DR CS SP H2.
+    (* have /=-> := success_det_tree_next_alt vA sA H2.
+    have ? := success_det_tree_same_ctx H1 sA H2; subst.
+    have /= := expand_sigP Func H1 SP (succes_is_solved _ _ sA).
+    rewrite H2 => ->//.
+    apply: Build_Unif; move=> *; apply: None. *)
+    admit.
+  - move=> s1 s2 r A B n eA R IH s' ? sV sV' O ckP tOA vA DR CS SP dtA; subst.
+    have [N /= /andP[CM tNB]] := saturate_sigP tOA eA.
+    case dtB: (tc_tree_aux sP B (N + O) (Func, sV)) => [X Y].
+    have ? := tc_tree_aux_step CM vA eA tOA tNB DR CS SP dtA dtB; subst.
+    have := IH _ erefl _ _ _ _ tNB (valid_tree_expand vA eA) _ _ (sigP_cat _ SP) dtB.
+    move=> [].
+      admit.
+      by apply/fsubsetP => x; rewrite domf_cat in_fsetU => /(fsubsetP DR)->; rewrite orbT.
+      apply/forallP => -[k kNO]; rewrite valPE [val _]/=.
+      case: fndP => // ksV.
+      rewrite fnd_in lookup_cat.
+      have kO:= fsubsetP DR k ksV.
+      rewrite kO (in_fnd kO)/=.
+      by have:= forallP CS (Sub k kO); rewrite valPE/= in_fnd//.
+    move=> -> H; split; auto.
+    Print sigP.
+    admit.
+  - move=> s1 s2 r A B n eA R IH s' ? sV sV' Rx cA vA SP dtA; subst.
+    (* have [Ry /= gtee] := saturate_sigP cA eA.
+    case TC: (tc_tree_aux sP B Ry (Func, sV)) => [X Y].
+    have ? := tc_tree_aux_step vA cA SP eA gtee dtA TC; subst.
+    have [-> H]:= IH _ erefl _ _ _ (andP gtee).1 (valid_tree_expand vA eA) SP TC.
+    split; auto.
+    apply: sigP_more_precise H. *)
+    admit.
+  - move=> s1 s2 A B r n fA nA _ IH s ? sV sV' C vA SP TC; subst.
+    (* have := failed_det_tree_next_alt vA C TC nA.
+    move => [[]// [N [? X MP]]]//.
+    have [] := IH _ erefl _ _ _ (valid_tree_next_alt vA nA) SP X; last first.
+      move=> H INV.
+      split; first by [].
+      by apply: sigP_more_precise MP INV.
+    by apply: closed_in_next_alt nA. *)
+    admit.
+Admitted.
+
+
+(*
+
+
+Section is_ko.
+  Lemma cutl_tc_tree_aux {sP R A d s}:
+    success A ->
+    tc_tree_aux sP (cutl A) R (d, sigma2ctx sP R s) = (d, R + sigma2ctx sP R (get_substS s A)).
+  Proof.
+    elim: A d s => //=.
+    - move=> A HA smid B HB d s; case: ifP => [dA sB|dA sA]/=.
+        rewrite is_dead_is_ko//success_is_ko?success_cut//=.
+        rewrite HB//=.
+        (* by rewrite HB//= is_dead_is_ko// maxD_refl//=success_is_ko//success_cut//. *)
+      by rewrite success_is_ko?success_cut//=is_ko_cutr HA//= maxD_refl//=.
+    - move=>A HA B0 HB0 B HB d s /andP[sA sB].
+      rewrite sA/= success_is_ko?success_cut//= HA//=is_ko_cutr sA.
+      rewrite get_ctx_sigma2_ctx ges_subst_cutl//.
+      by rewrite tc_tree_aux_catR HB.
+  Qed.
+End is_ko.
+
+Lemma assume_tm_flex_head {sP f d a N} V :
+  get_tm_hd (Callable2Tm f) = inr (inr V) ->
+    assume_call sP N (Callable_Comb f a) d = N.
+Proof.
+  rewrite/assume_call/=.
+  rewrite/flex_head => ->.
+  case: sigtm_rev => //= [[[]]]//.
+Qed.
+
+Section closed_in.
+  Open Scope fset_scope.
+
+  Definition all_vars_subset_strict (sV: sigV) (vars:{fset V}) :=
+    (vars == domf sV) && all_vars_subset sV vars.
+
+  Definition closed_inS (sV: sigV) t := all_vars_subset sV (vars_tm t).
+  Definition closed_inTS (sV: sigV) t := all_vars_subset sV (vars_tree t).
+
+  Lemma all_vars_comb f a: vars_tm (Tm_Comb f a) = vars_tm f `|` vars_tm a.
+  Proof. by []. Qed.
+
+  (* Lemma fsubset_assume sP O t s : domf O `<=` domf (assume_tm sP O t s).
+  Proof.
+    elim: t s O => //= [?|?|?|f IHf a IHa] [|[[]??]] O //=; [|case: ifP..] => //.
+      case: fndP => // H; case: ifP => //=; rewrite fsubsetUr//.
+    move=> _; by apply: fsubset_trans _ (IHa _ _).
+  Qed. *)
+
+  Lemma all_vars_subset_sub {K: choiceType} {V : Type} A B (ctx:{fmap K -> V}) : A `<=` B -> all_vars_subset ctx B -> all_vars_subset ctx A.
+    move=> H /forallP/= H1; apply/forallP => /=-[k kA]/=.
+    have /=kB := fsubsetP H k kA.
+    apply: H1 (Sub k kB).
+  Qed.
+
+  Lemma closed_inT_all_vars_sub A B ctx : vars_tree A `<=` vars_tree B -> closed_inT ctx B -> closed_inT ctx A.
+  Proof. by apply: all_vars_subset_sub. Qed.
+
+  Lemma closed_in_merge_sigL {t A B}: 
+    closed_in A t -> closed_in (merge_sig A B) t.
+  Proof. by apply: closed_in_sub; rewrite merge_sig_domf fsubsetUl. Qed.
+
+  Lemma closed_in_merge_sigR {t A B}: 
+    closed_in A t -> closed_in (merge_sig B A) t.
+  Proof. rewrite merge_comm. apply closed_in_merge_sigL. Qed.
+
+  Lemma closed_inT_sub A B t : domf A `<=` domf B -> closed_inT A t -> closed_inT B t.
+  Proof.
+    rewrite/closed_inT.
+    move=> dA /forallP/= H; apply/forallP => /= x; have {}H := H x.
+    by apply: fsubsetP H.
+  Qed.
+
+  Lemma closed_inT_merge_sigL {t A B}: 
+    closed_inT A t -> closed_inT (merge_sig A B) t.
+  Proof. by apply: closed_inT_sub; rewrite merge_sig_domf fsubsetUl. Qed.
+
+  Lemma closed_inT_merge_sigR {t A B}: 
+    closed_inT A t -> closed_inT (merge_sig B A) t.
+  Proof. rewrite merge_comm. apply closed_inT_merge_sigL. Qed.
+
+
+  (* Lemma all_varsT_dead A : vars_tree (dead A) = fset0.
+  Proof. elim: A => //=[_ -> _ _ ->|_ -> _ -> _ ->]; rewrite !fsetUid. Qed.
+  Lemma all_varsT_cutr A : vars_tree (cutr A) = fset0.
+  Proof. by elim: A => //=[_ -> _ _ ->|_ -> _ -> _ ->]; rewrite !fsetUid. Qed.
+
+  Lemma closed_in_dead {ctx A}: closed_inT ctx (dead A).
+  Proof. apply/forallP => /=; rewrite all_varsT_dead => -[]//. Qed. *)
+
+  (* Lemma closed_inT_cutr O A: closed_inT O (cutr A).
+  Proof. apply/forallP => /=; rewrite all_varsT_cutr => -[]//. Qed. *)
+
+  (* Lemma closed_inT_cutl O A: closed_inT O A -> closed_inT O (cutl A).
+  Proof.
+    elim: A => //=.
+    - move=> p c _; apply/forallP => -[]//.
+    - move=> L HL s R HR /closed_inT_orP[CL CR].
+      case: ifP => dL; apply/closed_inT_orP; split; auto.
+      by rewrite closed_inT_cutr.
+    move=> A HA B0 HB0 B HB /closed_inT_andP[cA cB0 cB].
+    by case: ifP => sA; apply/closed_inT_andP; repeat split; auto; rewrite closed_inT_cutr.
+  Qed. *)
+
+  Lemma all_vars_subset_fset0 {K : choiceType} {V : Type} A: @all_vars_subset K V A fset0.
+  Proof. apply/forallP => /=-[]//. Qed.
+
+  Lemma all_vars_subset_dom {K : choiceType} {V : Type} A B X:
+    domf A = domf B -> 
+    @all_vars_subset K V A X = @all_vars_subset K V B X.
+  Proof.
+    move=> H.
+    apply/forallP.
+    case: ifP => //=.
+      move=> H1 [k kP]/=.
+      have /={}H1 := forallP H1 (Sub k kP).
+      by move/fsetP: H => /(_ k) ->.
+    move=> /forallP/=.
+    apply: contra_not => H1 [k kP].
+    have /={}H1 := H1 (Sub k kP).
+    by move/fsetP: H => /(_ k) <-.
+  Qed.
+
+  Lemma close_in_dom A B t: domf A = domf B ->
+    closed_in A t = closed_in B t.
+  Proof. by apply: all_vars_subset_dom. Qed.
+  
+  Lemma close_inT_dom A B t: domf A = domf B ->
+    closed_inT A t = closed_inT B t.
+  Proof. by apply: all_vars_subset_dom. Qed.
+
+  Lemma all_varsT_dead_sub A:
+    vars_tree (dead A) `<=` vars_tree A.
+  Proof. elim: A => //= *; rewrite !fsetUSS//. Qed.
+
+  Lemma all_vars_next_alt b A B:
+    next_alt b A = Some B ->
+    vars_tree B `<=` vars_tree A.
+  Proof.
+    elim: A b B => //=.
+    - move=> []//[]//.
+    - move=> p c _ B [<-]//.
+    - move=> _ []//.
+    - move=> A HA s B HB b C.
+      case nA: next_alt => [A'|].
+        by move=> [<-]/=; rewrite !fsetSU//; apply: HA nA.
+      case nB: next_alt => [B'|]//[<-]{C}/=.
+      rewrite !fsetUSS//=; last by apply: HB nB.
+      case: ifP => //= _.
+      by rewrite all_varsT_dead_sub//.
+    move=> A HA B0 HB0 B HB b C.
+    case:ifP => fA.
+      case nA: next_alt => [A'|]//=.
+      case nB0: next_alt => [B0'|]//=[<-]/=.
+      apply: fsubsetU.
+      rewrite orbC predU1r// -fsetUA.
+      apply: fsetUSS (HA _ _ nA) _.
+      rewrite fsubUset fsubset_refl.
+      apply: HB0 nB0.
+    case: ifP => sA; last by move=> [<-].
+    case nB: next_alt => [B'|]; first by move=> [<-]/=; apply: fsetUS (HB _ _ nB).
+    case nA: next_alt => [A'|]//=.
+    case nB0: next_alt => [B0'|]//=[<-]/=.
+    apply: fsubsetU.
+    rewrite orbC predU1r// -fsetUA.
+    apply: fsetUSS (HA _ _ nA) _.
+    rewrite fsubUset fsubset_refl.
+    apply: HB0 nB0.
+  Qed.
+
+  Lemma all_vars_cutr_sub A : vars_tree (cutr A) `<=` vars_tree A.
+  Proof. by elim: A => //=; move=> *; rewrite !fsetUSS//. Qed.
+
+  Lemma all_vars_cutl_sub A : vars_tree (cutl A) `<=` vars_tree A.
+  Proof. by elim: A => //=>*; case: ifP => //= _; rewrite !fsetUSS//=all_vars_cutr_sub//. Qed.
+
+  Lemma all_vars_CB_sub u s A B:
+    step u s A = CutBrothers B ->
+    vars_tree B `<=` vars_tree A.
+  Proof.
+    elim: A s B => //[? []//||].
+      move=> A HA s B HB s1 B0/=; case: ifP; case: step => //.
+    move=> A HA B0 HB0 B HB s C/=.
+    case eA: step => //=[A'|A'].
+      move=> [<-]/=; do 2 apply: fsetUSS => //.
+      apply: HA eA.
+    have [? sA] := expand_solved_same _ eA; subst.
+    case eB: step => //[B'][<-]/=.
+    apply: fsetUSS (HB _ _ eB).
+    apply: fsetUSS; last by rewrite all_vars_cutr_sub.
+    apply: all_vars_cutl_sub.
+  Qed.
+
+  Lemma closed_in_next_alt {b A B ctx}:
+    closed_inT ctx A -> next_alt b A = Some B -> closed_inT ctx B.
+  Proof.
+    move=> H /all_vars_next_alt H1.
+    apply: closed_inT_all_vars_sub H1 H.
+  Qed.
+
+  Lemma closed_inT_step_CB {O u s A B}:
+    closed_inT O A -> step u s A = CutBrothers B -> closed_inT O B.
+  Proof.
+    move=> cA /all_vars_CB_sub H.
+    apply: closed_inT_all_vars_sub H cA.
+  Qed.
+
+End closed_in.
+
+Section change_only_in.
+  Open Scope fset_scope.
+
+
+
+  Definition change_only_in (N O: sigV) (V:{fset V}) :=
+    [&& (domf O == domf N), compat_sig N O &
+    [forall kN : domf N,
+          let valN := N.[valP kN] in
+          let valO := odflt valN O.[?val kN] in
+        if val kN \in V then incl valN valO
+        else valN == valO
+    ]].
+
+  Definition change_only_in_tm (N O: sigV) t :=
+    change_only_in N O (vars_tm t).
+
+  Definition change_only_in_tree (N O: sigV) t :=
+    change_only_in N O (vars_tree t).
+
+  Lemma change_only_in_vars_same_domain O N t:
+    change_only_in N O t -> domf O = domf N.
+  Proof. by move=> /and3P[]/eqP. Qed.
+
+  Lemma change_only_in_refl O t:
+    change_only_in O O t.
+  Proof.
+    rewrite /change_only_in eqxx compat_sig_refl.
+    apply/forallP => /=-[k /[dup] kP kP_]/=.
+    rewrite valPE (in_fnd kP_)/=; case: ifP => [_|_/[!eqxx]]//.
+  Qed.
+
+  (* Lemma change_only_in_trans A B C t0 t1:
+    change_only_in A B t0 -> change_only_in B C t1 -> change_only_in A C (t0 `|` t1).
+  Proof.
+    move=> /andP[/eqP dAB /forallP/=cAB].
+    move=> /andP[/eqP dBC /forallP/=cBC].
+    rewrite /change_only_in {1}dBC {1}dAB eqxx/=.
+    apply/forallP => /=-[k kA].
+    have kB : k \in domf B by rewrite dAB.
+    have kC : k \in domf C by rewrite dBC.
+    have {cAB}:= cAB (Sub k kA); have {cBC}:= cBC (Sub k kB).
+    rewrite !valPE/= !in_fnd//=.
+    case: ifP => kt1; case: ifP => kt2; rewrite in_fsetU kt1 kt2/=.
+    - by move=> /andP[C1 I1] /andP[C2 I2]; rewrite (compat_type_trans C1 C2) (incl_trans I2 I1).
+    - by move=> /andP[C1 I1]/eqP->; rewrite C1.
+    - by move=> /eqP->/andP[C1 I1]; rewrite C1.
+    by move=> /eqP->/eqP->.
+  Qed. *)
+
+  (* Lemma change_only_in_or1 N O A B:
+    change_only_in N O A ->
+      change_only_in N O (A `|` B).
+  Proof.
+    move=> /andP[/eqP H]/forallP/=H1.
+    rewrite/change_only_in {1}H eqxx/=.
+    apply/forallP => /=-[k kN]/=.
+    have kO: k \in domf O by rewrite H.
+    have:= H1 (Sub k kN).
+    rewrite valPE in_fsetU in_fnd//=.
+    case:ifP => //= kA/eqP<-; rewrite compat_type_refl.
+    case:ifP => //=.
+  Qed. *)
+
+  Lemma change_only_in_or N O f a:
+    change_only_in N O (f `|` a) =
+      [&& (domf O == domf N), compat_sig N O &
+        [forall kN : domf N,
+              let valN := N.[valP kN] in
+              let valO := odflt valN O.[?val kN] in
+            if (val kN \in f) || (val kN \in a) then incl valN valO
+            else valN == valO
+        ]].
+  Proof.
+    rewrite /change_only_in_tm/change_only_in; do 2 f_equal.
+    apply/forallP => /=.
+    case:ifP => /=.
+      move=> /forallP/= H [k kP]; rewrite valPE/=.
+      have {H}/= := H (Sub k kP).
+      rewrite in_fsetU valPE//.
+    move=> /negP.
+    apply:contra_not => H.
+    apply/forallP => -[k kP]/=; rewrite valPE.
+    have:= H (Sub k kP) => /=.
+    rewrite in_fsetU valPE//.
+  Qed.
+
+  Hint Resolve change_only_in_refl : core.
+  Hint Resolve compat_sig_refl : core.
+
+  Lemma compat_sig_set v O R (vO : v \in domf O):
+    compat_type O.[vO] R -> compat_sig O.[v <- R] O.
+  Proof.
+    move=> H; apply/forallP => -[k kO]; rewrite valPE [val _]/=.
+    case: fndP => //kE; rewrite ffunE/= in_fnd/=.
+    case: eqP => //?; subst.
+    by rewrite (bool_irrelevance kO vO).
+  Qed.
+
+  Lemma compat_sig_set2 v O N R1 R2:
+    compat_sig O N -> compat_type R1 R2 -> compat_sig O.[v <- R1] N.[v <- R2].
+  Proof.
+    move=> cON cR.
+    apply/forallP => -[k K]; rewrite valPE ffunE /=.
+    case: ifP => /eqP E; subst.
+      rewrite in_fnd//= ?fsetU11//=.
+      by move=> kU; rewrite ffunE/= eqxx compat_type_comm.
+    have kN : k \in domf N by move/fset1UP: K => []//.
+    rewrite in_fnd/=.
+    case: fndP => //=kvO; rewrite ffunE/=.
+    have kO : k \in domf O by move/fset1UP: kvO => []//.
+    rewrite in_fnd/=.
+    case: eqP => //.
+    by have := forallP cON (Sub k kN); rewrite valPE/= in_fnd/=.
+  Qed.
+
+  Lemma assume_tm_dom sP O A M: domf (assume_tm sP O A M) = domf O.
+  Proof.
+    elim: A O M => /=[_ O []//|_ O []//|v O [|[[] S _]]//|].
+      by case: fndP => // kO; case: ifP => //; rewrite domf_set_in//.
+    by move=> f Hf a Ha O [//|[[] S l]]; case: ifP => //=fH; rewrite Ha.
+  Qed.
+
+  Lemma compat_sig_trans {A B C}: 
+    domf C `<=` domf B -> domf B `<=` domf A ->
+      compat_sig A B -> compat_sig B C -> compat_sig A C.
+  Proof.
+    move=> dCB dBA cAB cBC.
+    apply/forallP => -[k kC]; rewrite valPE [val _]/=.
+    case: fndP => //=kA.
+    have kB := fsubsetP dCB k kC.
+    have/=:= forallP cAB (Sub k kB); rewrite valPE.
+    have/=:= forallP cBC (Sub k kC); rewrite valPE.
+    rewrite !in_fnd/=.
+    apply: compat_type_trans.
+  Qed.
+
+  Lemma incl_sig_trans {A B C}: 
+    domf C `<=` domf B -> domf B `<=` domf A ->
+      incl_sig A B -> incl_sig B C -> incl_sig A C.
+  Proof.
+    move=> dCB dBA cAB cBC.
+    apply/forallP => -[k kC]; rewrite valPE [val _]/=.
+    case: fndP => //=kA.
+    have kB := fsubsetP dCB k kC.
+    have/=:= forallP cBC (Sub k kC); rewrite valPE.
+    have/=:= forallP cAB (Sub k kB); rewrite valPE.
+    rewrite !in_fnd/=.
+    apply: incl_trans.
+  Qed.
+
+  Lemma compat_sig_assume_tm sP O A M: compat_sig (assume_tm sP O A M) O.
+  Proof.
+    elim: A O M => /=[_ O []//|_ O []//|v O [|[[] S _]]//|].
+      case: fndP => // kO; case: ifP => // H; rewrite compat_sig_set// min_comm.
+      by apply: compat_type_minR.
+    move=> f Hf a Ha O [//|[[] S l]]; case: ifP => //=fH.
+    by apply: compat_sig_trans (Ha _ _) (Hf _ _); rewrite !assume_tm_dom.
+  Qed.
+
+  Lemma assume_tm_in_vars sP O A M (kO : domf O):
+    if val kO \in vars_tm A then incl (odflt O.[valP kO] (assume_tm sP O A M).[?val kO]) O.[valP kO]
+    else (odflt O.[valP kO] (assume_tm sP O A M).[?val kO]) == O.[valP kO].
+  Proof.
+    case: kO => k kO; rewrite valPE [val _]/=.
+    have kOa: k \in domf (assume_tm sP O A M) by rewrite assume_tm_dom.
+    rewrite in_fnd/=.
+    elim: A O M k kO kOa => /=; only 1, 2: by move=> _ O [|x xs] ? k1 kO; rewrite (bool_irrelevance k1 kO).
+      move=> v O [|[[] S _]] v1 k1 k2; try by rewrite (bool_irrelevance k1 k2) incl_refl eqxx if_same.
+      move: k2.
+      rewrite in_fset1; case: eqP => H; subst.
+        rewrite in_fnd; case: ifP => /= C k2; last by rewrite (bool_irrelevance k1 k2).
+        by rewrite ffunE/=eqxx /incl -min_assoc min_refl.
+      case: fndP; last by move=> _ k2; rewrite (bool_irrelevance k1 k2).
+      move=> vO; case: ifP => C k2; last by rewrite (bool_irrelevance k1 k2).
+      rewrite ffunE/=; case: (v1 =P _) => // _.
+      by rewrite in_fnd/=.
+    move=> f Hf a Ha O [|[M S] xs] k k1 k2; first by rewrite (bool_irrelevance k1 k2) incl_refl eqxx if_same.
+    move: k2; case: ifP => fh k2; first by rewrite (bool_irrelevance k1 k2) incl_refl eqxx if_same.
+    rewrite in_fsetU.
+    move: k2; case: M => //=k2; last first.
+      have:= Hf O xs _ k1 k2.
+      by case: ifP => //=kf /eqP->; case:ifP.
+    have k3: k \in domf (assume_tm sP O f xs) by rewrite assume_tm_dom.
+    have:= Ha _ _ _ k3 k2.
+    case: ifP => kA; rewrite (orbF,orbT); last by move=> /eqP->; auto.
+    move=> H; apply: incl_trans H _.
+    have:= Hf _ _ _ k1 k3.
+    by case: ifP => // _ /eqP ->. 
+  Qed.
+
+  Lemma change_only_in_tm_assume_tm sP O M A:
+    change_only_in_tm (assume_tm sP O A M) O A.
+  Proof.
+    rewrite/change_only_in_tm/change_only_in.
+    rewrite {1}assume_tm_dom eqxx {1}compat_sig_assume_tm.
+    apply/forallP => /= -[k kO]; rewrite valPE [val _]/=.
+    have kO' : k \in O by rewrite assume_tm_dom in kO.
+    have/=:= assume_tm_in_vars sP A M (Sub k kO').
+    by rewrite valPE !in_fnd/=.
+  Qed.
+
+  Lemma change_only_in_tm_ck_callable {O N T sP d0 dA}:
+    check_callable sP O T d0 = (dA, N) -> change_only_in_tm N O (Callable2Tm T).
+  Proof.
+    rewrite/check_callable/change_only_in_tm.
+    case CT: check_tm => [[[| d]| m f a] b]; cycle 1; [|by move=> [_ <-]..].
+    case: b CT; last by move=> _ [_ <-].
+    case GC: get_callable_hd_sig => [v|] H1 [_ <-]//.
+    by apply: change_only_in_tm_assume_tm.
+  Qed.
+
+  (* Lemma change_only_in_mergeL SA SB O V:
+    change_only_in SA O V ->
+      change_only_in SB O V ->
+        change_only_in (merge_sig SA SB) O V.
+  Proof.
+    move=> /andP[/eqP dAO /forallP/=cAO] /andP[/eqP dBO /forallP/=cBO].
+    rewrite /change_only_in {1}merge_sig_domf -dAO -dBO fsetUid eqxx.
+    apply/forallP => -[k kP].
+    rewrite valPE [val _]/=.
+    have kO: k \in domf O by move: kP; rewrite merge_sig_domf -dAO -dBO fsetUid.
+    have kA: k \in domf SA by rewrite -dAO.
+    have kB: k \in domf SB by rewrite -dBO.
+    rewrite/= !ffunE.
+    case: fsetUP => //=[kA' _ kB' _|??/negP//|/negP//].
+    rewrite in_fnd//= (bool_irrelevance kA' kA) (bool_irrelevance kB' kB) {kA' kB'}.
+    have:= cAO (Sub k kA); rewrite valPE in_fnd//=.
+    have:= cBO (Sub k kB); rewrite valPE in_fnd//=.
+    case:ifP => kV.
+      move=>/andP[C1 I1] /andP[C2 I2].
+      rewrite inclL_max//= (compat_type_trans C2)//.
+      apply: compat_type_maxR.
+      by apply: compat_type_trans (compat_type_comm1 _) C1.
+    by move=>/eqP<-/eqP<-; rewrite max_refl.
+  Qed. *)
+
+  (* Definition good_continuation (k: D * sigV -> D * sigV) :=
+    forall (d:D) O T, change_only_in (k (d, O)).2 O (vars_tree T). *)
+
+  (*Lemma change_only_in_tree_tc_tree_aux {sP T d0 dN O N k}:
+    tc_tree_aux sP T k (d0, O) = (dN, N) ->
+    good_continuation k-> change_only_in_tree N O T.
+  Proof.
+    rewrite/change_only_in_tree.
+    elim: T d0 dN O N k => //; only 1, 3: by move=> d0 dN O N k [_ <-]//.
+    - move=> d0 dN O N k/= + /(_ d0 O OK) => ->//.
+    - move=> p c d0 dN O N k/=.
+      case C: check_callable => [D S].
+      move=> + /(_ (maxD d0 D) S ((CallS p c))) => ->/=.
+      have /= := change_only_in_tm_ck_callable C.
+      rewrite/change_only_in_tm.
+      move=> H1 H2.
+      have:= change_only_in_trans H2 H1.
+      by rewrite fsetUid.
+    - move=> d0 dN O N k/= + /(_ Func O CutS)/= => ->//.
+    - move=> A HA s B HB d0 dN O N k/=.
+      case kA: is_ko; case kB: is_ko => //=.
+      - by move=> [??]; subst.
+      - move=> H1 H2.
+        rewrite fsetUC. 
+        apply: change_only_in_or1.
+        apply: HB .
+          apply: H1.
+      case
+      move=> /change_only_in_or_subst<-.
+      rewrite change_only_in_refl//.
+      (* case dtB: tc_tree_aux => [DB SB].
+      case dtA: tc_tree_aux => [DA SA].
+      have {}HA := HA _ _ _ _ dtA.
+      have {}HB := HB _ _ _ _ dtB.
+      case kA: is_ko; case kB: is_ko => //=; cycle -1; [|move=> [_<-]//..].
+      move=> [??]; subst.
+      by rewrite change_only_in_refl. *)
+      (* - case:ifP => CA [_<-]; apply: change_only_in_mergeL; try (by apply: change_only_in_or1);
+        by rewrite fsetUC; apply: change_only_in_or1.
+      - by rewrite fsetUC; apply: change_only_in_or1.
+      - by apply: change_only_in_or1. *)
+    - move=> A HA B0 HB0 B HB O N d0 d1/=.
+      case dtA: tc_tree_aux => [DA SA].
+      case dtB0: tc_tree_aux => [DB0 SB0].
+      case dtB: tc_tree_aux => [DB SB].
+      have {}HA := HA _ _ _ _ dtA.
+      have {}HB := HB _ _ _ _ dtB.
+      have {}HB0 := HB0 _ _ _ _ dtB0.
+      case: ifP => kA; first by move=> [_ <-].
+      case: ifP => kB [_<-].
+        rewrite fsetUAC fsetUC.
+        apply: change_only_in_trans HB0 _.
+        by apply: change_only_in_or1.
+      apply: change_only_in_mergeL.
+        rewrite fsetUC.
+        apply: change_only_in_trans HB _.
+        by apply: change_only_in_or1.
+      apply: change_only_in_or1.
+      rewrite fsetUC.
+      apply: change_only_in_trans HB0 HA.
+  Qed. *)
+  (* Print Assumptions change_only_in_tree_tc_tree_aux. *)
+End change_only_in.
+
+Section cat.
+
+  Open Scope fset_scope.
+
+  Definition change_only_in_k (k: D * sigV -> D * sigV) V :=
+    forall d0 s0 d1 s1, k (d0, s0) = (d1, s1) ->
+      change_only_in s1 s0 V.
+
+  Definition k_cat (k: D * sigV -> D * sigV) :=
+    forall d0 s s0 d1 s1, k (d0, s0) = (d1, s1) ->
+      k (d0, s + s0) = (d1, s + s1).
+
+  Lemma xxxx sP A R O1 d s:
+    (* need that O1 and R are compatible, and all are weak *)
+    tc_tree_aux sP A (R + O1) (d, R + s) =
+    tc_tree_aux sP A (R + O1) (d, s).
+  Proof.
+    elim: A d R s O1 => /=.
+    - move=> d R s O1.
+  Admitted.
+
+  Opaque compat_sig_subst.
+
+  (* good type environment *)
+  Definition gte sP (N : sigV) T := [&& all_weak N, closed_inT N T & compat_sig_subst sP N T].
+
+  (* good type environment extension *)
+
+  Lemma tc_tree_aux_cat sP T R K d0 s0 d1 d2 N1 N2:
+    gte sP R T -> gtee sP K R T ->
+    valid_tree T ->
+    tc_tree_aux sP T R (d0,s0) = (d1, N1) ->
+    tc_tree_aux sP T K (d0,s0) = (d2, N2) ->
+    ((d1 = d2) * (N2 = K + N1)).
+  Proof.
+    (* elim: T R K d0 d1 d2 N1 N2 s0 => /=;
+    only 1, 2, 3, 5: by move=> ??? > _ _ _ [<-<-][<-<-]; rewrite catfA.
+    - move=> /= p c O1 O2 d0 d1 d2 N1 N2 s0 G1 G2 _.
+      case C1: check_callable => [dX sX].
+      case C2: check_callable => [dY sY].
+      move=> [??][??]; subst.
+      rewrite -catfA in C2.
+      have H3 := closed_in_cat _ C.
+      by have [<-<-]:= check_callable_cat (H3 _) C1 C2.
+    - move=> A HA s B HB O1 O2 d0 d1 d2 N1 N2 s0. 
+      move=> /closed_inT_orP[cA cB] /=.
+      case: ifP => [dA vB|dA/andP[vA bB]].
+        rewrite is_dead_is_ko//=.
+        case: ifP => kB; first by move=> [??][??]; subst; rewrite catfA.
+        by apply: HB.
+      case kA: is_ko => /=.
+        case: ifP => kB; first by move=> [??][??]; subst; rewrite catfA.
+        by apply/HB/bbOr_valid.
+      case: ifP => kB; first by apply: HA.
+      case tA: (tc_tree_aux _ A) => [DA SA].
+      case tA': (tc_tree_aux _ A) => [DA' SA'].
+      case tB: (tc_tree_aux _ B) => [DB SB].
+      case tB': (tc_tree_aux _ B) => [DB' SB'].
+      have {HA}[??] := HA _ _ _ _ _ _ _ _ cA vA tA tA'; subst.
+      have {HB}[??] := HB _ _ _ _ _ _ _ _ cB (bbOr_valid bB) tB tB'; subst.
+      case: ifP => CA /=[??][??]; subst; split; auto.
+        admit.
+      admit.
+    move=> A HA B0 HB0 B HB O1 O2 d0 d1 d2 N1 N2 s0 /closed_inT_andP[cA cB0 cB] /=.
+    move=>/and4P[vA++cK].
+    case kA: is_ko.
+      rewrite is_ko_success//=is_ko_failed//= => /eqP? bB[??][??]; subst.
+      by rewrite catfA.
+    rewrite !tc_tree_aux_catR.
+    case: ifP => /=[sA vB bB0|sA/eqP?]; subst.
+      move/orP: bB0 => []bB; last first.
+        rewrite base_and_ko_is_ko// => tB tB'.
+        apply: HB cB vB tB tB'.
+      rewrite base_and_is_ko//.
+      case tA: (tc_tree_aux _ A) => [DA SA].
+      case tA': (tc_tree_aux _ A) => [DA' SA'].
+      case tB: (tc_tree_aux _ B) => [DB SB].
+      case tB': (tc_tree_aux _ B) => [DB' SB'].
+      case tB0: (tc_tree_aux _ B0) => [DB0 SB0].
+      case tB0': (tc_tree_aux _ B0) => [DB0' SB0'].
+      move=> [??][??]; subst.
+      have {HA}[??] := HA _ _ _ _ _ _ _ _ cA vA tA tA'; subst.
+      have {HB}[??] := HB _ _ _ _ _ _ _ _ cB vB tB tB'; subst.
+      rewrite xxxx in tB0'.
+      have {HB0}[??] := HB0 _ _ _ _ _ _ _ _ cB0 (base_and_valid bB) tB0 tB0'; subst.
+      admit.
+    case kB: is_ko; rewrite/bbAnd.
+      case bB: base_and; first by rewrite base_and_is_ko in kB.
+      by case: ifP => //=fA {}bB [??][??]; subst; rewrite catfA.
+    rewrite (contraFF base_and_ko_is_ko)// orbF if_same => bB.
+    case tA: (tc_tree_aux _ A) => [DA SA].
+    case tA': (tc_tree_aux _ A) => [DA' SA'].
+    case tB: (tc_tree_aux _ B) => [DB SB].
+    case tB': (tc_tree_aux _ B) => [DB' SB'].
+    move=> [??][??]; subst.
+    have {HA}[??] := HA _ _ _ _ _ _ _ _ cA vA tA tA'; subst.
+    rewrite xxxx in tB'.
+    by have := HB _ _ _ _ _ _ _ _ cB (base_and_valid bB) tB tB'; subst. *)
+  Admitted.
+End cat.
+
+Section extends.
+  Open Scope fset_scope.
+
+  Definition extends (O N : sigV) :=
+    (domf O `<=` domf N) &&
+    [forall x : domf N,
+        if val x \in domf O then Some N.[valP x] == O.[? val x]
+        else N.[valP x] == weak N.[valP x]].
+
+  Lemma extends_refl N : extends N N.
+  Proof.
+    rewrite /extends fsubset_refl; apply/forallP=> -[x xP]/=.
+    by rewrite valPE/= xP in_fnd eqxx.
+  Qed.
+    
+  Lemma extends_trans : transitive extends.
+  Proof.
+    rewrite /extends => M N O => /andP[sNM /forallP H1] /andP[sMO /forallP H2].
+    rewrite (fsubset_trans sNM sMO); apply/forallP=> -[x xO]/=.
+    have /= {H2} := H2 (Sub x xO).
+    case: ifP => [xM | /negbT nxM ].
+      rewrite valPE/= in_fnd.
+      have [xN | nxN] := fndP.
+        have /= /[!xN]/eqP := H1 (Sub x xM).
+        by rewrite in_fnd valPE/= => <-.
+      have /= /[!(negPf nxN)] := H1 (Sub x xM).
+      rewrite valPE/= => /eqP E.
+      by rewrite E => /eqP[->]; rewrite weak2.
+    have nxN : x \notin domf N.
+      by apply: contra nxM; apply: fsubsetP.
+    by rewrite valPE/= (negPf nxN).
+  Qed.
+
+  Lemma extend_sub A B : extends A B -> domf A `<=`domf  B. by case/andP. Qed.
+
+
+  Lemma extendsP {O N} : 
+    reflect (exists X, N = X + O /\ all_weak X.[\ domf O]) (extends O N).
+  Proof.
+    case E: extends; constructor.
+      move: E=> /andP[ON /forallP/= H].
+      exists [fmap x : domf N => odflt (weak N.[valP x]) O.[? val x] ].
+      split.
+        apply/fmapP => k.
+        have [kO|nkO]:= (boolP (k \in domf O)).
+          have kN:= fsubsetP ON k kO.
+          have kS: k \in domf ([fmap x => odflt (weak N.[valP x]) O.[? \val x]] + O) by rewrite mem_catf kO orbT.
+          rewrite !in_fnd; f_equal.
+          have:= H (Sub k kN).
+          rewrite valPE [val _]/= kO !in_fnd => /eqP[->].
+          by rewrite getf_catr.
+        case: fndP => [kN|nkN].
+          have SD: domf [fmap x => odflt (weak N.[valP x]) O.[? \val x]] = domf N by apply/fsetP => x/=.
+          have kS: k \in domf ([fmap x => odflt (weak N.[valP x]) O.[? \val x]] + O) by rewrite domf_cat SD in_fsetU kN.
+          rewrite in_fnd getf_catl//= ffunE valPE/= not_fnd//=.
+          have:= H (Sub k kN).
+          rewrite /= (negPf nkO) valPE => /eqP<-//.
+        have H1 : domf N = domf [fmap x => odflt (weak N.[valP x]) O.[? fsval x]] by apply/fsetP.
+        have H2: k \notin domf [fmap x => odflt (weak N.[valP x]) O.[? fsval x]] by rewrite -H1.
+        rewrite not_fnd//=.
+        by rewrite mem_catf (negPf nkO) orbF//.
+      apply/forallP => -[x xN]; rewrite valPE ffunE/=.
+      rewrite ffunE/=.
+      have:= xN.
+      rewrite domf_rem in_fsetD => /andP[xO] xN'.
+      by rewrite not_fnd//= weak2.
+    move /negP: E; apply contra_not.
+    move=> [X[? W]]; subst.
+    rewrite/extends {1}domf_cat fsubsetUr.
+    apply/forallP => -[x xN].
+    rewrite valPE [val _]/=.
+    have:= xN.
+    rewrite {1}domf_cat in_fsetU.
+    case:ifP => [xO _|nxO /[!orbF] xX].
+      rewrite in_fnd.
+      rewrite (fnd_in xN) lookup_cat xO/= in_fnd//.
+    rewrite (fnd_in xN) lookup_cat nxO in_fnd//=.
+    have xK: x \in (domf X.[\ domf O]) by rewrite domf_rem in_fsetD (negbT nxO)//.
+    have:= forallP W (Sub x xK).
+    rewrite valPE (fnd_in xK).
+    by rewrite fnd_rem nxO in_fnd/=.
+  Qed.
+
+  (* Lemma tc_tree_auxW sP A d d' d'' O O' N N' :
+    closed_inT O A ->
+    tc_tree_aux sP O A d = (d', N) ->
+    extends O O' ->
+    tc_tree_aux sP O' A d = (d'', N') -> d' = d'' /\ extends N N'.
+  Proof.
+    (* IDEA: we only change the variables that are in A *)
+    (* the other variables stay the same *)
+    (* the variables we change, change in the same way tkx to tc_tree_aux__ *)
+    move=> CA tO E tO'.
+    have [/=X[? H]] := extendsP E; subst.
+    have [??] := tc_tree_aux_cat CA tO tO'; subst.
+    split; auto.
+    have H1 := change_only_in_vars_same_domain (change_only_in_tree_tc_tree_aux tO).
+    rewrite H1 in H.
+    by apply/extendsP; repeat eexists.
+  Qed. *)
+
+End extends.
+
+Section more_precise.
+  Open Scope fset_scope.
+
+  (* Lemma more_preciseP N O:
+    reflect ( 
+      (domf O `<=` domf N) /\
+      forall x : domf N,
+          let oldv := odflt N.[valP x] O.[? val x] in
+          let newv := N.[valP x] in
+          compat_type oldv newv /\ incl newv oldv) (more_precise N O).
+  Proof.
+    case X: more_precise; constructor.
+    - move: X => /andP[-> /forallP/=] H; split; auto; by move=> H1; apply/andP/H.
+    - move/negP: X; apply:contra_not; rewrite/more_precise.
+      by move=> [->]//= H; apply/forallP => /= x; apply/andP/H.
+  Qed. *)
+
+  Lemma change_only_in_vars_mp O N t: change_only_in N O t -> more_precise N O.
+  Proof.
+    rewrite/more_precise/change_only_in.
+    move=> /and3P[/eqP H CS H1].
+    rewrite {1}H fsubset_refl CS.
+    apply/forallP => -[k kO]; rewrite valPE/=.
+    case: fndP => //= kN.
+    have:= forallP H1 (Sub k kN); rewrite valPE/= in_fnd/=.
+    by case: ifP => // _ /eqP->.
+  Qed.
+
+  Lemma more_precise_refl A : more_precise A A.
+  Proof.
+    apply: change_only_in_vars_mp.
+    apply: change_only_in_refl fset0.
+  Qed.
+
+  Lemma more_precise_trans : transitive more_precise.
+  Proof.
+    rewrite /more_precise => B A C.
+    move=> /and3P[dBA cAB iAB] /and3P[dCB cBC iBC].
+    rewrite (fsubset_trans dCB dBA) (compat_sig_trans dCB dBA cAB cBC).
+    by apply: incl_sig_trans iAB iBC.
+  Qed.
+
+  Lemma more_precise_sub A B : more_precise A B -> domf B `<=` domf A.
+  Proof. by case/andP. Qed.
+
+  Lemma closed_inT_mp {t A B}: 
+    closed_inT B t -> more_precise A B ->  closed_inT A t.
+  Proof.
+    move=> + MP.
+    have:= more_precise_sub MP.
+    apply: closed_inT_sub.
+  Qed.
+
+  Lemma more_precise_same_type {B A : sigV} x:
+    more_precise B A -> forall kA : x \in A, forall kB : x \in B, compat_type A.[kA] B.[kB].
+  Proof.
+    move=> /and3P[dAb cBA iBA] kA kB.
+    have:= forallP cBA (Sub x kA); rewrite valPE/=.
+    by rewrite in_fnd.
+  Qed.
+
+  Lemma in_more_precise {k} {B A : sigV}:
+    more_precise B A -> forall kA : k \in domf A,
+        exists kB : k \in domf B, incl B.[kB] A.[kA].
+  Proof.
+    move=> /and3P[dAB cBA iBA] kA.
+    have kB := (fsubsetP dAB k kA).
+    exists kB; have:= forallP iBA (Sub k kA).
+    by rewrite in_fnd//= valPE.
+  Qed.
+
+  Lemma in_more_compat_type {k} {B A : sigV}:
+    more_precise B A -> forall kA : k \in domf A,
+      exists kB : k \in domf B, compat_type A.[kA] B.[kB].
+  Proof.
+    move=> /and3P[dAB cBA iBA] kA.
+    have kB := (fsubsetP dAB k kA).
+    exists kB; have:= forallP cBA (Sub k kA).
+    by rewrite in_fnd//= valPE.
+  Qed.
+
+  Lemma in_more_compat_type_more_precise {k} {B A : sigV}:
+    more_precise B A -> forall kA : k \in domf A,
+        exists kB : k \in domf B, compat_type A.[kA] B.[kB] /\ incl B.[kB] A.[kA].
+  Proof.
+    move=> MP kA.
+    have [kB CP] := in_more_compat_type MP kA.
+    have [kB' +] := in_more_precise MP kA.
+    rewrite (bool_irrelevance kB' kB) => I.
+    by exists kB; split.
+  Qed.
+
+  Lemma in2_more_compat_type_more_precise {k} {B A : sigV}:
+    more_precise B A -> forall kA : k \in domf A,
+        forall kB : k \in domf B, (compat_type A.[kA] B.[kB] /\ incl B.[kB] A.[kA])%type2.
+  Proof.
+    move=> /in_more_compat_type_more_precise H kA kB.
+    have [kB' []] := H _ kA.
+    by rewrite (bool_irrelevance kB' kB); split.
+  Qed.
+
+  Lemma in2_more_precise {k} {B A : sigV}:
+    more_precise B A -> forall kA : k \in domf A,
+        forall kB : k \in domf B, incl B.[kB] A.[kA].
+  Proof. by move=> MP kA kB; rewrite (in2_more_compat_type_more_precise MP kA kB). Qed.
+
+  Lemma in2_more_compat_type {k} {B A : sigV}:
+    more_precise B A -> forall kA : k \in domf A,
+        forall kB : k \in domf B, compat_type A.[kA] B.[kB].
+  Proof. by move=> MP kA kB; rewrite (in2_more_compat_type_more_precise MP kA kB). Qed.
+
+  Lemma more_precise_merge N O:
+    domf N = domf O -> more_precise N O -> merge_sig O N = O.
+  Proof.
+    move=> SD MP.
+    apply/fmapP => k.
+    have SD' : domf (merge_sig O N) = domf O by rewrite merge_sig_domf SD fsetUid.
+    case: fndP => /[dup] kON kON_; last first.
+      have kO : k \notin domf O by rewrite -SD'.
+      by rewrite not_fnd.
+    rewrite merge_sig_domf in kON.
+    have kO : k \in domf O by rewrite -SD'.
+    rewrite in_fnd fnd_in.
+    have kN : k \in domf N by rewrite SD.
+    rewrite merge_sigLR/=.
+    move/and3P: MP => [_ _ /forallP].
+    move=> /(_ (Sub k kO)); rewrite valPE/= in_fnd/= => /eqP<-.
+    by rewrite min_comm max_assorb.
+  Qed.
+  
+  Lemma set2_more_precise old new S1 S2 v:
+    more_precise new old ->
+      incl S1 S2 -> compat_type S1 S2 ->
+        more_precise new.[v <- S1] old.[v <- S2].
+  Proof.
+    move=> /and3P[dON cNO iNO i12] c12.
+    rewrite/more_precise !{1}dom_setf fsetUS //.
+    rewrite compat_sig_set2//=.
+    apply/forallP => -[k kvO]; rewrite [val _]/= valPE.
+    have /fset1UP[] := kvO => kO; subst.
+      have kvN: v \in domf (new.[v <- S1]) by apply/fset1UP;auto.
+      by rewrite in_fnd//= !ffunE/= eqxx.
+    have kN := fsubsetP dON k kO.
+    have kvN: k \in domf (new.[v <- S1]) by apply/fset1UP; auto.
+    rewrite in_fnd/= !ffunE/= !in_fnd/=; case: ifP => //= _.
+    have /= := forallP iNO (Sub k kO).
+    by rewrite in_fnd/= valPE.
+  Qed.
+
+  Lemma setL_more_precise old new sNew k (kO : k \in domf old):
+    more_precise new old ->
+      incl sNew old.[kO] -> compat_type old.[kO] sNew ->
+        more_precise new.[k <- sNew] old.
+  Proof.
+    move=> /and3P[dON cNO iNO] isO cON.
+    rewrite/more_precise/=; apply/and3P; split.
+      by apply/fsubsetP => x H; rewrite fset1Ur// (fsubsetP dON x H).
+      apply/forallP => /=-[x xO]; case: fndP => //= xdn.
+      rewrite valPE ffunE/=.
+      have xN:= fsubsetP dON _ xO.
+      rewrite in_fnd/=; case: eqP => ?; subst.
+        by rewrite (bool_irrelevance xO kO).
+      have/=:= forallP cNO (Sub x xO).
+      by rewrite valPE in_fnd.
+    apply/forallP => -[x xO]; rewrite valPE [val _]/=.
+    have xN:= fsubsetP dON _ xO.
+    have xkN : x \in (new.[k <- sNew]) by apply/fset1UP; auto.
+    rewrite in_fnd/= ffunE/= in_fnd//=; case: eqP => ?; subst.
+      by rewrite (bool_irrelevance xO kO).
+    have/=:= forallP iNO (Sub x xO).
+    by rewrite valPE in_fnd.
+  Qed.
+
+  Lemma setL_more_precise_abs old new sNew k:
+    more_precise new old ->
+      k \notin domf old -> 
+        more_precise new.[k <- sNew] old.
+  Proof.
+    move=> /and3P[dON cNO iNO] kO.
+    apply/andP; split.
+      apply/fsubsetP => x H.
+      by rewrite fset1Ur// (fsubsetP dON x H).
+    apply/andP; split.
+      apply/forallP => -[k1 kvN]; rewrite valPE [val _]/=.
+      case: fndP => //= k1N; rewrite ffunE/=; case: eqP => H; subst.
+        by rewrite kvN in kO.
+      have/fset1UP[]:=k1N=>// kN; rewrite in_fnd//=.
+      have /= := forallP cNO (Sub k1 kvN).
+      by rewrite valPE in_fnd.
+    apply/forallP => -[k1 kvN]; rewrite valPE [val _]/=.
+    case: fndP => //= k1N; rewrite ffunE/=; case: eqP => H; subst.
+      by rewrite kvN in kO.
+    have/fset1UP[]:=k1N=>// kN; rewrite in_fnd//=.
+    have /= := forallP iNO (Sub k1 kvN).
+    by rewrite valPE in_fnd.
+  Qed.
+
+  Hint Resolve more_precise_refl : core.
+
+  Lemma more_precise_assume_tm {new old sP tm d}:
+    more_precise new old ->
+    more_precise (assume_tm sP new tm d) (assume_tm sP old tm d).
+  Proof.
+    elim: tm new old d.
+    - move=> _ new old []//.
+    - move=> _ new old []//.
+    - move=> v new old [|[[] s] _] //= H.
+      case: (fndP old) => [/[dup] ko ko_|].
+        have [kn[CP IN]] := in_more_compat_type_more_precise H ko.
+        rewrite (in_fnd kn).
+        rewrite (bool_irrelevance ko_ ko).
+        do 2 case:ifP => //=.
+        - move=> H1 H2; apply: set2_more_precise H _ (compat_type_min _ (compat_type_comm1 _) _) => //.
+          rewrite -(eqP IN)/incl min_assoc (@min_comm _ s) min_assoc min_refl.
+          by rewrite -!min_assoc min_refl//.
+          by rewrite compat_type_comm.
+        - move=> H1 H2; apply: setL_more_precise => //; rewrite (bool_irrelevance ko_ ko).
+          by apply: incl_trans IN; rewrite/incl -min_assoc min_refl.
+          apply: compat_type_trans CP _.
+          by rewrite min_comm compat_type_minR.
+        - by move=> /compat_type_comm1 /compat_type_trans -/(_ _ CP) /compat_type_comm1 ->.
+      move=> vo.
+      case: fndP => //=[kf]; case:ifP => //.
+      move=> H1.
+      by apply: setL_more_precise_abs.
+    - by move=> /= f Hf a Ha N O [//|[[] s] xs] MP; case:ifP => //=fl; [apply: Ha|]; apply: Hf.
+  Qed.
+
+  Lemma assume_tm_more_precise sP old tm S:
+    more_precise (assume_tm sP old tm S) old.
+  Proof.
+    apply: change_only_in_vars_mp.
+    apply: change_only_in_tm_assume_tm.
+  Qed.
+
+  Lemma more_precise_mergeL {A B C}:
+    more_precise A C -> more_precise B C ->
+      more_precise (merge_sig A B) C.
+  Proof.
+    move=> /and3P[dCA cAC iAC] /and3P[dCB cBC iBC].
+    rewrite/more_precise; apply/andP; split; first rewrite merge_sig_domf.
+      by apply: fsubsetU; rewrite dCA.
+    apply/andP; split; apply/forallP => -[k kC]; rewrite valPE [val _]/=;
+    have kA := fsubsetP dCA _ kC;
+    have kB := fsubsetP dCB _ kC;
+    rewrite merge_sigLR/=.
+      have /=:= forallP cAC (Sub k kC).
+      have /=:= forallP cBC (Sub k kC).
+      rewrite valPE !in_fnd/=.
+      move=> H1 H2.
+      rewrite -{1}(@max_refl C.[kC]).
+      apply: compat_type_max => //=.
+      by rewrite compat_type_comm.
+    have /=:= forallP iBC (Sub k kC).
+    have /=:= forallP iAC (Sub k kC).
+    rewrite valPE !in_fnd/=.
+    apply: inclL_max.
+  Qed.
+
+  (* Lemma extends_mp {A B}:
+    extends A B -> more_precise B A.
+  Proof.
+    move=>/extendsP /=[X [H1 AW]]; subst.
+    rewrite /more_precise {1}domf_cat fsubsetUr.
+    apply/forallP => -[k kV]; rewrite !valPE [val _]/=.
+    have:= kV; rewrite {1}domf_cat in_fsetU.
+    case:fndP => [kA _|nkA kX].
+      by rewrite (fnd_in kV) lookup_cat kA (in_fnd kA)/= compat_type_refl incl_refl.
+    rewrite orbF in kX.
+    by rewrite (fnd_in kV) lookup_cat nkA (in_fnd kX)/= compat_type_refl incl_refl.
+  Qed. *)
+
+  Lemma closed_in_mp {t A B}: 
+    closed_in B t -> more_precise A B ->  closed_in A t.
+  Proof.
+    move=> + MP.
+    have:= more_precise_sub MP.
+    apply: closed_in_sub.
+  Qed.
+
+  Lemma more_precise_check_callable1 sP O N T d0 dA:
+    check_callable sP O T d0 = (dA, N) -> 
+      more_precise N O.
+  Proof. by move=> /change_only_in_tm_ck_callable/change_only_in_vars_mp. Qed.
+
+  Definition more_precise_opt '(smore, bmore) '(sless, bless) :=
+    (bmore || ~~bless) && incl smore sless.
+
+  Lemma more_precise_compat_check_tm sP new old c:
+    closed_in old c ->
+      more_precise new old ->
+      compat_type
+        (check_tm sP new c).1
+        (check_tm sP old c).1.
+  Proof.
+    move=> +mp.
+    elim: c => //=.
+    - move=> v /[!closed_in_var]vO /[!(in_fnd vO)]/=.
+      have [kN] := in_more_compat_type mp vO.
+      by rewrite in_fnd//= compat_type_comm.
+    - move=> f + a + /[!closed_in_comb]/andP[vf vA] => /(_ vf) + /(_ vA).
+      case: check_tm => [sa []];
+      case: check_tm => [sa' []];
+      case: check_tm => [sf' []] => //; case: sa => [[]|[]s t]; case: sa' => [[]|[]s' t']//= /andP[??]//=;
+      case: check_tm => [sf []] => //=; case E: incl => //=; case F: incl => //= ?; rewrite !compat_type_weak //.
+  Qed.
+
+  Lemma more_precise_check_tm sP new old c:
+      closed_in old c ->
+      more_precise new old ->
+        more_precise_opt (check_tm sP new c) (check_tm sP old c).
+  Proof.
+    elim: c new old => //=.
+    - by move=> k N O MP; case: fndP => *; exact: incl_refl.
+    - move=> v N O /[!closed_in_var] vO MP /[!in_fnd vO].
+      by have [vN ?]:= in_more_precise MP vO; rewrite in_fnd.
+    - move=> f + a + N O /[!closed_in_comb]/andP[vf va] MP => /(_ _ _ vf MP) + /(_ _ _ va MP).
+      have := more_precise_compat_check_tm sP va MP.
+      have := more_precise_compat_check_tm sP vf MP.
+      case: check_tm => [[//[|d1]|//[] s1 t1]// b1];
+      case: check_tm => [[//[|d2]|//[] s2 t2]// b2]//=; rewrite !incl_arr/=;
+      move=> /andP[++] + /andP[++]; last by move=> +++ ->/= /andP[+->]//.
+      case: check_tm => [sx bx];
+      case: check_tm => [sw bw]/=; rewrite ?andbF/=?andbT//;
+      destruct bx, bw; rewrite//=?andbF?andbT/=; try (by move=> +/comp_weak->); last first.
+        by case:ifP => /= _ _ /comp_weak <-//; rewrite weak_incl.
+      destruct b1, b2; rewrite ?andbF?andbT//=; last first.
+        by move=> + /comp_weak->.
+        by case:ifP => //=; move=> ++/comp_weak<-; rewrite //weak_incl.
+      repeat case: ifP => //=; try by move=> +++/comp_weak<-; rewrite //weak_incl.
+        by move=> _ _ _ _ _ _ /andP[].
+      move=> I1 I2 C1 C2 C3 _ /andP[I3 I4] I5.
+      by rewrite  (incl_trans I5 (incl_trans I1 I3)) in I2.
+  Qed.
+
+  Lemma closed_in_MP_get_callable_hd_sig sP N O t: 
+    closed_in O t ->
+      more_precise N O -> 
+        if get_tm_hd_sig sP N t is Some vN then
+          exists vO, get_tm_hd_sig sP O t = Some vO /\ incl vN vO
+        else get_tm_hd_sig sP O t = None.
+  Proof.
+    rewrite/get_tm_hd_sig/=.
+    elim: t => //=.
+    - by move=> k _ MP; case: fndP => //=; repeat eexists.
+    - by move=> k _ MP; repeat eexists.
+    - move=> v /[!closed_in_var]vO MP.
+      have [vN I] := in_more_precise MP vO.
+      by rewrite (in_fnd vN)/= (in_fnd vO);repeat eexists.
+    - move=> f Hf a Ha /[!closed_in_comb]/andP[CA CO] MP; by apply: Hf.
+  Qed.
+
+  Lemma more_precise_check_callable sP N O t dO dN dN' dO' O' N':
+    closed_in O (Callable2Tm t) ->
+    check_callable sP O t dO = (dO', O') -> 
+    check_callable sP N t dN = (dN', N') ->
+    more_precise N O ->
+    more_precise N' O' /\ (((minD dO dN = dN) -> minD dO' dN' = dN')).
+  Proof.
+    rewrite/check_callable/=.
+    move=> CO ++ MP.
+    have:= more_precise_check_tm sP CO MP.
+    have:= more_precise_compat_check_tm sP CO MP.
+    case Cn: check_tm => [sn bn]; case Co: check_tm => [so bo]/=.
+    rewrite/get_callable_hd_sig/=.
+    move=> + /andP[HB].
+    case: sn Cn => [[|dn]|mn fn an] Cn; case: so Co => [[|doo]|mo fo ao] Co//=; try (by destruct mn); cycle 2.
+    - by move=> _ _[<-<-][<-<-]; auto.
+    - by move=> _ _ [??][??]; subst; auto.
+    - move=> _.
+      case: bo HB Co; [case: bn Cn => //Cn|] => // _ Co I; last first.
+        move=> [<-<-].
+        destruct bn; last move=> [<-<-]; auto.
+        case sN: get_tm_hd_sig => [v|][<-<-]; last by auto.
+        split; last by [].
+        apply: more_precise_trans (MP).
+        apply: assume_tm_more_precise.
+      have:= closed_in_MP_get_callable_hd_sig sP CO MP.
+      rewrite/get_tm_hd_sig.
+      case X: get_tm_hd => [D|[P|V]].
+        have:= get_tm_hd_callable t.
+        by rewrite X => -[].
+      - case: fndP => [kf [_ [[<-]]] _ [<-<-]| nkf _ [<-<-]][<-<-]; last by [].
+        split; first by apply: more_precise_assume_tm.
+        move=> <-; destruct dn, doo, dO => //=.
+      case: (fndP O); last first.
+        move=> vO + [??]; subst => /=.
+        case: fndP => [kf [S []]|]// _ _ [_<-]//.
+      have CN := closed_in_mp CO MP.
+      move=> VO.
+      have [VN I1] := in_more_precise MP VO.
+      rewrite (in_fnd VN).
+      move=> [vO[[?]] H [<-<-]][<-<-]; subst.
+      split => //=.
+        destruct t => //=.
+        simpl in X.
+        rewrite !(assume_tm_flex_head X)//=.
+      move=> <-; destruct doo, dn, dO => //=.
+  Qed.
+
+  Definition good_continuation1 (k: (D * sigV) -> (D*sigV)) :=
+    forall dO dN dO' dN' O O' N N',
+      more_precise  N O ->
+        k (dO, O) = (dO', O') ->
+        k (dN, N) = (dN', N') -> 
+        more_precise N' O' /\ (minD dO dN = dN -> minD dO' dN' = dN').
+
+  Print get_ctxS.
+
+  (* Lemma good_continuation1P sP B0 k R:
+    base_and B0 ->
+    closed_inT R B0 ->
+    good_continuation1 k ->
+      good_continuation1 (tc_tree_aux sP B0 R k) .
+  Proof.
+    elim: B0 k => //=.
+    move=> A HA B0 HB0 B HB k H.
+    have {H} : (is_call A || (A == CutS)) /\ [/\ (B0 = B),  base_and B, success A = false, valid_tree A & is_ko A = false].
+      by move: H; destruct A => //= /andP[/eqP->->]; auto.
+    move=> [H1] [? bB SA vA kA]; subst; clear HB0 HA.
+    move=> /closed_inT_andP[cA cB0 cB] GCk dO dN dO' dN' O O' N N' MP.
+    rewrite kA SA base_and_is_ko//=.
+    case tA: tc_tree_aux => [dA sA]/=.
+    case tA': tc_tree_aux => [dA' sA'].
+    move=> [??][??]; subst.
+    have {}HB := HB _ bB cB GCk.
+    move: tA tA' => /=.
+    destruct A => //=; last first.
+      move=> tB tB'.
+      have [] := HB _ _ _ _ _ _ _ _ MP tB tB'; auto.
+    case C1: check_callable => [dA sA].
+    case C2: check_callable => [dA' sA'].
+    move=> tB tB'.
+    have [] := more_precise_check_callable (closed_in_cat _ cA) C1 C2.
+      admit. (*more_precise merge 2*)
+    move=> MPa H.
+    have [->] := HB _ _ _ _ _ _ _ _ MPa tB tB'.
+    by destruct dO, dA, dN, dA'; auto.
+  Admitted. *)
+
+  (* Lemma more_precise_gtee A B K R T:
+    (* TODO: all_weak K and compat with B *)
+    compat_sig R B ->
+    gtee K R T -> more_precise A B -> more_precise (K + A) (R + B).
+  Proof.
+    move=> cRB /andP[/andP[wK _] /andP[cKR dRK]].
+    move=> /andP[dBA/forallP/= MP].
+    rewrite /more_precise 2!{1}domf_cat fsetUSS//.
+    apply/forallP => -[k kKA]; rewrite valPE [val _]/=.
+    (* have: (k \in domf K) || (k \in domf A) by move: kKA; rewrite domf_cat in_fsetU. *)
+    rewrite (fnd_in kKA).
+    rewrite 2!lookup_cat.
+    case : (fndP B k) => kB.
+      have kA: k \in domf A := fsubsetP dBA k kB.
+      have := H (Sub k kA).
+      rewrite kA (in_fnd kA)/=.
+      by rewrite in_fnd//=valPE.
+    case : (fndP A k) => kA.
+      have := H (Sub k kA).
+      rewrite valPE/= not_fnd//=; case: fndP => //=kK.
+      admit.
+    have kK : k \in domf K by move: kKA; rewrite domf_cat in_fsetU (negPf kA) => /orP[].
+    by rewrite in_fnd/= compat_type_refl incl_refl.
+  Admitted. *)
+
+  Lemma compat_sig_cat R K A B:
+    domf B `<=` domf A ->
+    domf K `<=` domf R ->
+    compat_sig R K -> compat_sig A R -> compat_sig A B ->
+    compat_sig (R + A) (K + B).
+  Proof.
+    move=> dBA dKR c1 c2 c3.
+    apply/forallP => -[k kKB]; rewrite valPE [val _]/=.
+    rewrite fnd_in !lookup_cat.
+    case: (fndP B k) => kB.
+      have kA := fsubsetP dBA _ kB.
+      have:= forallP c3 (Sub k kB); rewrite valPE/=.
+      by rewrite in_fnd kA/=.
+    case: fndP => kK.
+      have kR := fsubsetP dKR _ kK.
+      rewrite (in_fnd kR)/=.
+      have:= forallP c1 (Sub k kK).
+      rewrite valPE/= in_fnd//=.
+      move=> cKR.
+      case: (fndP A k) => //=kA.
+      have:= forallP c2 (Sub k kR).
+      rewrite valPE/= in_fnd//=.
+      by apply: compat_type_trans.
+    have:= kKB.
+    by rewrite {1}domf_cat in_fsetU (negPf kB) (negPf kK).
+  Qed.
+
+  Lemma incl_sig_cat R K A B:
+    domf B `<=` domf A ->
+    domf K `<=` domf R ->
+    all_weak K -> all_weak R ->
+    compat_sig R K ->
+    compat_sig A R ->
+    compat_sig A B ->
+    incl_sig A B ->
+    incl_sig (R + A) (K + B).
+  Proof.
+    move=> dBA dKR wK wR c1 c2 c3 iAB.
+    apply/forallP => -[k kKB]; rewrite valPE [val _]/=.
+    rewrite fnd_in !lookup_cat.
+    case: (fndP B k) => kB.
+      have kA := fsubsetP dBA _ kB.
+      have:= forallP iAB (Sub k kB); rewrite valPE/=.
+      by rewrite in_fnd kA/=.
+    case: fndP => kK.
+      have kR := fsubsetP dKR _ kK.
+      have:= forallP wK (Sub k kK); rewrite valPE => /eqP {}wK.
+      have:= forallP wR (Sub k kR); rewrite valPE => /eqP {}wR.
+      rewrite (in_fnd kR)/=.
+      have:= forallP c1 (Sub k kK).
+      rewrite valPE/= in_fnd//=.
+      move=> cKR.
+      rewrite wK wR.
+      case: (fndP A k) => //=kA.
+        have:= forallP c2 (Sub k kR).
+        rewrite valPE/= in_fnd//=.
+        move=> cRA.
+        apply: compat_type_incl_weak.
+        have cKA:= compat_type_trans cKR cRA.
+        by rewrite compat_type_comm.
+      by rewrite (compat_type_weak_eq cKR).
+    by exfalso; have:= kKB; rewrite domf_cat in_fsetU (negPf kB) (negPf kK).
+  Qed.
+
+  Lemma more_precise_catL sP T A B K R:
+    gte sP K T -> gtee sP R K T ->
+    compat_sig A R ->
+    more_precise A B -> more_precise (R + A) (K + B).
+  Proof.
+    move=> /andP [wK _] /and3P[/andP[wR _ cRK]] dKR cAR.
+    move=> /and3P[dBA cAB iAB].
+    apply/and3P; split.
+      by rewrite !domf_cat; apply: fsetUSS.
+      by apply: compat_sig_cat.
+    by apply: incl_sig_cat.
+  Qed.
+
+  (* Lemma 
+    all_vars_subset K (vars_sigma s) ->
+      compat_sig (sigma2ctx sP s) K. *)
+
+  Lemma compat_subst_compat_sig sP K s:
+    compat_subst sP K s -> compat_sig (sigma2ctx sP K s) K.
+  Proof.
+    move=> /andP[CL H].
+    apply/forallP => -[k kK].
+    rewrite valPE [val _]/=.
+    case: fndP => //= ks; rewrite ffunE.
+    have:= forallP H (Sub k ks).
+    rewrite valPE in_fnd.
+    by case: check_tm => //=S [] H1; rewrite compat_type_comm//compat_type_weakL.
+  Qed.
+
+  (* Lemma compat_subst_closed_in sP R (s: Sigma) k (kP: k \in domf s):
+    compat_subst sP R s -> closed_in R s.[kP].
+  Proof.
+    move=> /forallP => /(_ (Sub k kP))/=.
+    case: fndP => //=kR; rewrite valPE. *)
+
+
+  Lemma more_precise_sigma2ctx sP s R K A:
+    all_weak R ->
+    gtee sP K R A -> compat_subst sP R s ->
+    more_precise (sigma2ctx sP K s) (sigma2ctx sP R s).
+  Proof. by move=> *; erewrite sigma2ctx_cat1; eauto. Qed.
+
+  Lemma more_precise_get_ctxS sP K R N O A:
+    gte sP R A ->
+    gtee sP K R A ->
+    more_precise N O ->
+    more_precise (get_ctxS sP K N A) (get_ctxS sP R O A).
+  Proof.
+    elim: A N O => //=.
+      move=> A HA s B HB N O /gte_orP[GA GB Gs] /gtee_orP[GA' GB' Gs'] MP.
+      case: ifP => dA; auto.
+      apply: HB => //.
+      apply: more_precise_sigma2ctx; eauto.
+      by move/and3P: GA => [].
+    move=> A HA B0 HB0 B HB N O /gte_andP[GA GB0 GB] /gtee_andP[GA' GB0' GB'] MP.
+    by case:ifP => sA; auto.
+  Qed.
+
+  (* Lemma get_ctxS_dom k s sP K N B:
+    k \in K ->
+    k \in domf (get_substS s B) ->
+    k \in domf (get_ctxS sP K N B).
+  Proof.
+    elim: B => //=. *)
+
+  Lemma compat_sig_get_ctxS sP K N A:
+    (* gte sP K A -> compat_sig N K -> *)
+    compat_sig (get_ctxS sP K N A) K.
+  Proof.
+    (*move=> H H1; apply/forallP=> -[k kK].
+    have {H1} := forallP H1 (Sub k kK).
+    rewrite !valPE/= => H2.
+    elim: A H => //=.
+      move=> A HA s B HB /gte_orP [gA gB /andP[H cS]].
+      case:ifP => dA; last by auto.
+      rewrite get_ctx_sigma2_ctx.
+      case: fndP => //= kB; rewrite ffunE valPE.
+      suffices: compat_type K.[kK] (check_tm sP K (get_substS s B).[kB]).1.
+        case: check_tm => [S []]//=.
+        by move=> /comp_weak<-; rewrite compat_type_weak//.
+      case C: check_tm => [/=S b].
+      have {HB HA} := HB gB.
+      have:= forallP cS (Sub ).
+      have:= cS.
+      rewrite/compat_subst.
+      case X: check_tm => //=.
+      case: fndP => //=. *)
+    Admitted.
+
+  Lemma more_precise_tc_tree_aux A R K sP O N dO dO' O' dN dN' N':
+    gte sP R A ->
+    gtee sP K R A ->
+    valid_tree A ->
+    more_precise N O ->
+    compat_sig N K ->
+      tc_tree_aux sP A R (dO, O) = (dO', O') ->
+      tc_tree_aux sP A K (dN, N) = (dN', N') -> 
+     (* good_continuation1 k -> *)
+        more_precise N' O' /\ (minD dO dN = dN -> minD dO' dN' = dN').
+  Proof.
+    elim: A O N dO dO' O' dN dN' N' R K => //=;
+    only 1, 2, 4: by move=> /= > G G' _ MP CS [<-<-][<-<-]; split; auto;
+    by apply: more_precise_catL; eauto.
+    - move=> p c O N dO dO' O' dN dN' N' R K G G' _ CO MP.
+      case CkO: check_callable => [dOx Ox].
+      case CkN: check_callable => [dNx Nx] [??][??]; subst.
+      have [_ CR _] := (and3P G).
+      have  := more_precise_check_callable (closed_in_cat _ CR) CkO CkN (more_precise_catL G G' MP CO).
+      by move=> []; destruct dO, dN; auto.
+    - move=> A HA s B HB O N dO dO' O' dN dN' N' R K.
+      move=> /gte_orP[GA GB Rs] /gtee_orP[GA' GB' Ks] + MP CS.
+      case dtA: (tc_tree_aux _ A) => //=[dAO OA].
+      case dtB: (tc_tree_aux _ B) => //=[dBO OB].
+      case dtAN: (tc_tree_aux _ A) => //=[dAN NA].
+      case dtBN: (tc_tree_aux _ B) => //=[dBN NB].
+      case:ifP => [dA vB|dA /andP[vA bB]].
+        rewrite is_dead_is_ko//=.
+        case:ifP => kB[??][??]; subst.
+          split; auto.
+          by apply: more_precise_catL; eauto.
+        apply: HB dtB dtBN; auto.
+          by apply: more_precise_sigma2ctx (gte_w GA) GA' _.
+        by apply: compat_subst_compat_sig.
+      have [MPa {}HA] := HA _ _ _ _ _ _ _ _ _ _ GA GA' vA MP CS dtA dtAN.
+      have [MPb {}HB]:= HB _ _ _ _ _ _ _ _ _ _ GB GB' (bbOr_valid bB) (more_precise_sigma2ctx (gte_w GA) GA' Rs) (compat_subst_compat_sig Ks) dtB dtBN.
+      case kA:is_ko => /=.
+        move: dtA dtAN; rewrite !is_ko_tc_tree_aux//= =>-[??][??]; subst.
+        case: ifP => kB [??][??]; subst; last by [].
+        by move: dtB dtBN; rewrite is_ko_tc_tree_aux//=.
+      case: ifP => kB [??][??]; subst.
+        move: dtB dtBN; rewrite !is_ko_tc_tree_aux//= => -[??][??]; subst.
+      split.
+        admit. (*more_precise merge PB*)
+      case:ifP => //= CA.
+      destruct dO, dAO, dBO => //= ?; subst => /=.
+      destruct dAN; last by auto.
+      destruct dBN; auto.
+    - move=> A HA B0 HB0 B HB O N dO dO' O' dN dN' N' R K /gte_andP[cA cB0 cB] /gtee_andP[cA' cB0' cB'].
+      move=> /and4P[vA++cK] MP cNK.
+      case:(boolP (is_ko _)) => kA.
+        rewrite is_ko_success//= is_ko_failed// => /eqP->{B0 cK HB0 cB0 cB0'} bB.
+        move=> [<-<-][<-<-]; split; auto.
+        by apply: more_precise_catL cA cA' _ _.
+      case:ifP => /=[sA vB bB | sA /eqP->{B0 HB0 cB0 cB0' cK} +].
+        move: bB => /orP[]bB; last first.
+          rewrite base_and_ko_is_ko//= => H1 H2.
+          apply: HB H1 H2; auto.
+          apply: more_precise_catL (cA) (cA') _ (more_precise_get_ctxS cA cA' MP).
+            apply: compat_sig_get_ctxS.
+          apply: compat_sig_catL_id.
+          apply: compat_sig_get_ctxS.
+        rewrite base_and_is_ko//.
+        case dtA: (tc_tree_aux _ A) => [dAO svAO].
+        case dtAN: (tc_tree_aux _ A) => [dAN svAN].
+        case dtB: (tc_tree_aux _ B) => [dBO sVBO].
+        case dtBN: (tc_tree_aux _ B) => [dBN sVBN].
+        case dtB0: (tc_tree_aux _ B0) => [dB0 sVB0].
+        case dtB0N: (tc_tree_aux _ B0) => [dB0N sVB0N].
+        move=> [??][??]; subst.
+        have [MPa {}HA] := HA _ _ _ _ _ _ _ _ _ _ cA cA' vA MP cNK dtA dtAN.
+        have TODO: compat_sig (get_ctxS sP K N A) K  by apply: compat_sig_get_ctxS.
+        have [MPb {}HB] := HB _ _ _ _ _ _ _ _ _ _ cB cB' vB (more_precise_get_ctxS cA cA' MP) TODO dtB dtBN.
+        have TODO1: compat_sig svAN K by admit.
+        have [MPb0 {}HB0] := HB0 _ _ _ _ _ _ _ _ _ _ cB0 cB0' (base_and_valid bB) MPa TODO1 dtB0 dtB0N.
+        split.
+          admit. (*more_precise merge PB*)
+        destruct dBO, dB0 => //=.
+        by move=> /[dup]/HB/=<-/HA/HB0/=<-.
+      case dtA: (tc_tree_aux _ A) => [dAO svAO].
+      case dtAN: (tc_tree_aux _ A) => [dAN svAN].
+      case dtB: (tc_tree_aux _ B) => [dBO sVBO].
+      case dtBN: (tc_tree_aux _ B) => [dBN sVBN].
+      case kB: is_ko => + [??][??]; subst; rewrite/bbAnd.
+        case bB: base_and; first by rewrite base_and_is_ko in kB.
+        by rewrite (@more_precise_catL sP A)//.
+      rewrite (contraFF base_and_ko_is_ko)// orbF if_same => bB.
+      have [MPa {}HA] := HA _ _ _ _ _ _ _ _ _ _ cA cA' vA MP cNK dtA dtAN.
+      have TODO: compat_sig svAN K by admit.
+      have [] := HB _ _ _ _ _ _ _ _ _ _ cB cB' (base_and_valid bB) MPa TODO dtB dtBN.
+      by auto.
+  Admitted.
+
+
+End more_precise.
+Hint Resolve more_precise_refl : core.
+
+Section next_alt.
+
+  (* Lemma success_det_tree_same_ctx {sP A sV1 sV2 d0 d1}:
+    closed_inT sV1 A -> success A -> (tc_tree_aux sP sV1 A d0) = (d1, sV2) ->
+      (sV2 = sV1)%type2.
+  Proof.
+    elim: A sV1 sV2 d0 d1 => //=; try by move=>*; congruence.
+    (* - move=> A HA s B HB sV1 sV2 d0 d1 /closed_inT_orP[cA cB].
+      case TCB: tc_tree_aux => [D2 S2].
+      case TCA: tc_tree_aux => [D1 S1].
+      have {}HA := HA _ _ _ _ cA _ TCA.
+      have {}HB := HB _ _ _ _ cB _ TCB.
+      case: ifP => [dA sB|ndA sA]; first by rewrite is_dead_is_ko =>//=; case: ifP => kB [??]; subst; auto.
+      rewrite success_is_ko//.
+      case:ifP => kB [??]; subst; first by auto.
+      rewrite HA//.
+      have MP := more_precise_tc_tree_aux1 TCB.
+      apply: more_precise_merge MP.
+      have /andP[/eqP H _]:= change_only_in_tree_tc_tree_aux TCB.
+      by rewrite H. *)
+    - move=> A HA B0 HB0 B HB sV1 sV2 d0 d1 /closed_inT_andP[cA cB0 cB] /andP[sA sB].
+      rewrite !success_is_ko//=.
+      case dtA: tc_tree_aux => [DA SA].
+      case dtB: tc_tree_aux => [DB SB].
+      case dtB0: tc_tree_aux => [DB0 SB0].
+      have ? := HA _ _ _ _ cA sA dtA; subst.
+      have ? := HB _ _ _ _ cB sB dtB; subst.
+      have MP := more_precise_tc_tree_aux1 dtB0.
+      move=> [??]; subst.
+      apply: more_precise_merge MP.
+      have /andP[/eqP H _]:= change_only_in_tree_tc_tree_aux dtB0.
+      by rewrite H.
+  Qed. *)
+
+  Lemma check_callable_func2 {sP sV A s1 s2 d0 d1 d2 d3}:
+    check_callable sP sV A d0 = (d1, s1) ->
+      check_callable sP sV A d2 = (d3, s2) ->
+        s1 = s2 /\ minD d1 d3 = if minD d0 d2 == d0 then d1 else d3.
+  Proof.
+    rewrite/check_callable.
+    case: check_tm => //=[sA bA].
+    case: sA => //; last by move=> _ _ _ [<-<-][<-<-]; rewrite if_same.
+    move=> []; first by move=> [<-<-][<-<-]; rewrite if_same.
+    move=> d.
+    case: bA; last by move=> [<-<-][<-<-]; rewrite if_same.
+    case: get_callable_hd_sig; last by move=> [<-<-][<-<-]; rewrite if_same.
+    move=> X [<-<-][<-].
+    by destruct d0, d, d2.
+  Qed.
+
+  Lemma success_det_tree_next_alt sP A R d0 s0 N:
+    valid_tree A -> success A -> tc_tree_aux sP A R (d0,s0) = (Func, N) ->
+      (next_alt false (build_na A (next_alt true A)) = None)%type2.
+  Proof.
+    elim: A d0 s0 N => //=.
+    - move=> A HA s B HB d0 s0 N.
+      case kA: is_ko => /=.
+        rewrite (is_ko_next_alt _ kA)//= (is_ko_success kA).
+        case: ifP => [dA vB sB|//].
+        rewrite success_is_ko// => H.
+        have:= HB _ _ _ vB sB H.
+        case nB: (next_alt _ B) => //=[B'|] nB'; rewrite is_dead_next_alt//= if_same;
+        last by rewrite is_dead_next_alt.
+        by rewrite nB'.
+      rewrite (contraFF is_dead_is_ko kA).
+      move=> /andP[vA bB] sA.
+      move /orP: bB => []bB; last first.
+        have kB := base_or_aux_ko_is_ko bB.
+        rewrite kB (is_ko_next_alt _ kB).
+        move=> /(HA _ _ _ vA sA).
+        case nA: (next_alt _ A) => [A'|]/= nA'; last rewrite !is_dead_next_alt//=.
+        rewrite nA' is_ko_next_alt//.
+      have kB := base_or_aux_is_ko bB.
+      by rewrite kB success_has_cut//=.
+    - move=> A HA B0 HB0 B HB d0 s0 N /and4P[vA ++ Ck] /andP[sA sB].
+      rewrite sA success_is_ko//= success_failed//= => vB /orP[]bB; last first.
+        have kB := base_and_ko_is_ko bB.
+        rewrite kB !(is_ko_next_alt _ kB)// => tB.
+        have:= HB _ _ _ vB sB tB.
+        case nB: (next_alt _ B) => [B'|]//=; last first.
+          move=> _.
+          by case nA: (next_alt _ A) => [A'|]/=; rewrite is_dead_failed//is_dead_next_alt//.
+        rewrite success_failed//sA => nB'.
+        by rewrite nB' (is_ko_next_alt _ kB)//; case: next_alt.
+      have kB := base_and_is_ko bB.
+      rewrite kB.
+      case tA: (tc_tree_aux _ A) => //=[dA SA];
+      case tB: (tc_tree_aux _ B) => //=[[] SB]//=;
+      case tB0: (tc_tree_aux _ B0) => //=[[] SB0]//= [?]; subst.
+      rewrite (next_alt_aux_base_and bB).
+      have {HB} := HB _ _ _ vB sB tB.
+      destruct dA.
+        have {HA} := HA _ _ _ vA sA tA.
+        case nA: (next_alt _ A) => [A'|]//=; case nB: (next_alt _ B) => [B'|]//= nA' nB'.
+        - rewrite success_failed sA//nA nB' next_alt_aux_base_and//.
+          admit.
+        - rewrite (next_alt_failed nA) next_alt_aux_base_and//= if_same.
+          admit.
+        - by rewrite success_failed sA//nB' nA.
+        - by rewrite is_dead_failed// is_dead_next_alt//.
+      admit.
+  Admitted.
+
+  (* Lemma failed_det_tree_next_alt {sP A O O' d ign B} b:
+    valid_tree A ->
+    closed_inT O A ->
+    tc_tree_aux sP O A ign = (d, O') ->
+      next_alt b A = Some B ->
+        exists d' N, [/\ minD d d' = d',
+          (tc_tree_aux sP O B ign) = (d', N) & more_precise N O'].
+  Proof.
+    elim: A B O O' d ign b => //=.
+    - move=> B s1 s2 d ign [] _ _ //[<-<-][<-]; repeat eexists; rewrite ?minD_refl//.
+    - move=> p c B s1 s2 d1 d2 _ _ cl. 
+      case C: check_callable => [D S] [<-<-][<-]/=; rewrite C; repeat eexists.
+        by rewrite minD_refl.
+      by rewrite more_precise_refl.
+    - by move=> B s1 s2 d1 d2 _ _ _ [??][?]; subst; (repeat eexists); rewrite ?more_precise_refl//=.
+    - move=> A HA s B HB s1 s2 C d1 d2 b + /closed_inT_orP[cA cB].
+      case dtA: (tc_tree_aux _ _ A) => /=[DA sVA]//=.
+      case dtB: (tc_tree_aux _ _ B) => /=[DB sVB]//=.
+      have {}HA := HA _ _ _ _ _ _ _ cA dtA.
+      have {}HB := HB _ _ _ _ _ _ _ cB dtB.
+      case:ifP => [dA /andP[dAB vB]|ndA /and3P[dAB vA bB]].
+        rewrite is_dead_is_ko//=.
+        case:ifP => kB[??]; subst.
+          rewrite is_dead_next_alt//=.
+          rewrite is_ko_next_alt//.
+        rewrite is_dead_next_alt//=.
+        case nB: next_alt => //=[B'][<-]{s1}/=.
+        rewrite is_dead_is_ko//.
+        case dtB': (tc_tree_aux _ _ B') => /=[DB' sVB']//=.
+        have [d' [N [H1 H2 H3]]] := HB _ _ vB nB.
+        have [? H] := tc_tree_aux_func2 dtB' H2; subst.
+        rewrite (next_alt_is_ko nB).
+        repeat eexists; last by [].
+        by destruct d2, DB, DB', d'.
+      case kA: is_ko; case kB: is_ko => //=-[??]; subst.
+      - by rewrite !is_ko_next_alt => //=.
+      - rewrite is_ko_next_alt//=.
+        case nB: next_alt => [v|]//=[<-]/=; subst.
+        rewrite (is_dead_is_ko is_dead_dead).
+        have [d' [N [H1 H2 H3]]]:= HB _ _ (bbOr_valid bB) nB.
+        move: dtA; rewrite is_ko_tc_tree_aux => //= -[??]; subst.
+        rewrite (next_alt_is_ko nB)//= H2.
+        repeat eexists; last by [].
+        by destruct d2 => //=.
+      - rewrite (is_ko_next_alt _ kB).
+        case nA: next_alt => [v|]//= [<-]/=.
+        rewrite (next_alt_is_ko nA)/=kB.
+        have [d' [N [H1 H2 H3]]]:= HA _ _ vA nA.
+        rewrite H2; repeat eexists; last by [].
+        by destruct d2 => //.
+      case nA: next_alt => [A'|]//=.
+        move=> [<-]/=.
+        rewrite (next_alt_is_ko nA)/=kB; rewrite dtB.
+        have:= HA _ _ vA nA.
+        move=>[d'[S [m tcA' L]]]/=.
+        rewrite tcA'/=.
+        have MP1 :=(more_precise_tc_tree_aux1 dtA).
+        have MP2 := (more_precise_tc_tree_aux1 dtB). 
+        have C1 := closed_in_mp _ MP1.
+        have C2 := closed_in_mp _ MP2.
+        case:ifP => cA'; repeat eexists; [|by apply: more_precise_refl..].
+        destruct d2, DA, DB, d' => //=.
+        by rewrite (next_alt_keep_cut vA nA) cA'.
+      case nB: next_alt => [B'|]//= [<-]/=.
+      have {HB}:= HB _ _ (bbOr_valid bB) nB.
+      move => -[d'[S [m dtB' L]]].
+      rewrite (is_dead_is_ko is_dead_dead)//=.
+      rewrite dtB' (next_alt_is_ko nB).
+      repeat eexists; last first.
+        have MP:= more_precise_tc_tree_aux1 dtA.
+        have MP1:= more_precise_tc_tree_aux1 dtB.
+        have cA1 := closed_in_mp _ MP1.
+        apply:more_precise_refl.
+        (* by apply: more_precise_mergeR. *)
+        (* move=> //. *)
+      case:ifP => //=.
+      by destruct d2, DA, DB => //=.
+    move=> A HA B0 HB0 B HB C O O' d1 d2 b /and4P[vA +++] /closed_inT_andP[cA cB0 cB].
+    case dtA: (tc_tree_aux _ _ A) => /=[DA SA]//=.
+    case dtB: (tc_tree_aux _ _ B) => /=[DB SB]//=.
+    have MPOA := more_precise_tc_tree_aux1 dtA.
+    have cB': closed_inT SA B by apply: closed_inT_mp cB _.
+    have {}HA := HA _ _ _ _ _ _ vA cA dtA.
+    have {}HB := HB _ _ _ _ _ _ _ cB' dtB.
+    case: (ifP (is_ko A)) => kA; first by rewrite is_ko_success// is_ko_failed//=is_ko_next_alt//.
+    case:ifP => /=[sA vB bB0 CC| sA/eqP -> {B0 HB0 cB0}].
+      case dtB0: (tc_tree_aux _ _ B0) => /=[DB0 SB0]//=.
+      rewrite success_failed//=.
+      case:ifP => kB [??]; subst.
+        rewrite is_ko_next_alt//.
+        case nA: next_alt => //=[A'].
+        move/orP: bB0 => [bB|bB]; last by rewrite next_alt_aux_base_and_ko.
+        rewrite next_alt_aux_base_and//=.
+        move=> [<-]/=.
+        rewrite (next_alt_is_ko nA).
+        have [d3[N2 [mA2 tcA' MP3]]] := HA _ _ nA.
+        rewrite tcA'.
+        case dtB0': (tc_tree_aux _ _ B0) => /=[DB0' SB0'].
+        have cB0': closed_inT SA B0 by apply: closed_inT_mp cB0 _.
+        have [MP4 mx] := more_precise_tc_tree_aux (base_and_valid bB) cB0' dtB0 dtB0' MP3.
+        rewrite failed_is_ko ?base_and_failed//.
+        repeat eexists; first by destruct DB, d3, DB0'; auto.
+        by rewrite merge_refl.
+      case nB: next_alt => [B'|].
+        move=> [<-]/=.
+        have [d1[N1 [M2 TC MP2]]] := HB _ _ vB nB.
+        rewrite success_is_ko//=.
+        rewrite dtA/= dtB0 TC.
+        rewrite (next_alt_is_ko nB).
+        repeat eexists; first by destruct DB0, DB => //.
+        (* by apply: more_precise_merge2. *)
+        admit.
+      case nA: next_alt => //=[A'].
+      move/orP: bB0 => [bB|bB]; last by rewrite next_alt_aux_base_and_ko.
+      rewrite next_alt_aux_base_and//=.
+      move=> [<-]/=.
+      rewrite (next_alt_is_ko nA).
+      have [d3[N2 [mA2 tcA' MP3]]] := HA _ _ nA.
+      rewrite tcA'.
+      case dtB0': (tc_tree_aux _ _ B0) => /=[DB0' SB0'].
+      have cB0': closed_inT SA B0 by apply: closed_inT_mp cB0 _.
+      have [MP4 mx] := more_precise_tc_tree_aux (base_and_valid bB) cB0' dtB0 dtB0' MP3.
+      rewrite failed_is_ko ?base_and_failed//.
+      repeat eexists; first by destruct DB0, DB, d3, DB0'; auto.
+      rewrite merge_refl.
+      (* by apply: more_precise_mergeR. *)
+      admit.
+    move=> + _; rewrite dtB.
+    case kB: is_ko.
+      have bF: base_and B = false.
+        case bB: base_and => //.
+        rewrite failed_is_ko ?base_and_failed// in kB.
+      rewrite/bbAnd bF; case: ifP => //= fA bB [??]; subst.
+      case nA: next_alt => [A'|]; last by [].
+      rewrite is_ko_next_alt//.
+    case: ifP => /=[fA bB|fA bB] [??]; subst; last first.
+      by move=> [<-]/=; rewrite kA dtA dtB merge_refl maxD_refl kB; repeat eexists.
+    case nA: next_alt => [A'|]; last by [].
+    move/orP:bB => []bB; last by rewrite next_alt_aux_base_and_ko.
+    rewrite next_alt_aux_base_and//.
+    have {HA} [d'[S [m tcA' K]]] := HA _ _ nA.
+    move=> [<-]/=.
+    rewrite (next_alt_is_ko nA)/= tcA'.
+    case tcB': tc_tree_aux => [DB' SB'].
+    have [MP1 M] := more_precise_tc_tree_aux (base_and_valid bB) cB' dtB tcB' K.
+    rewrite !maxD_refl !merge_refl kB.
+    by repeat eexists; auto.
+  Qed. *)
+End next_alt.
+
+Lemma check_rules_select {sP sV u l rc m s rules}:
+  check_rules sP sV rules ->
+    select u rc m rules s = l ->
+      check_rules sP sV (map snd l).
+Proof.
+  move=> +<-{l}.
+  elim: rules => //= -[hd pm]/= rs IH.
+  case cr: check_rule => // /IH {}IH.
+  case X: H => //=[s']; rewrite IH andbT.
+  rewrite cr//.
+Qed.
+
+(* Lemma sigP_catL sP s K O:
+  all_weak K ->
+  sigP sP s O -> sigP sP s (K + O).
+Proof.
+  move=> H1 H2.
+  apply/forallP => -[k kKO]; rewrite valPE [val _]/=.
+  rewrite fnd_in lookup_cat.
+  case: (fndP O k) => kO.
+    move=> /=.
+    have /= := forallP H2 (Sub k kO).
+    by rewrite valPE.
+  case: fndP => [kK|nkK].
+    have /= := forallP H1 (Sub k kK).
+    rewrite valPE => /eqP /[dup] H <-.
+    case: fndP => //ks.
+    rewrite/good_assignment.
+      case C: check_tm => [S []].
+    apply/andP.
+    apply/forallP.
+    move=> /=.
+    move=> /=.
+  case: fndP => //.
+  move=> /=. *)
+
+Lemma sigP_success1 sP tE s O K:
+  (* all_weak K -> *)
+  (* gte K A -> *)
+  sigP sP tE s O ->
+  sigP sP tE s (K + O).
+Proof.
+  move=> H.
+  apply/forallP => -[k kKO]; rewrite valPE [val _]/=.
+  have:= kKO; rewrite {1}domf_cat in_fsetU.
+  rewrite fnd_in lookup_cat.
+  case: (fndP O k) => kO.
+    move=> /= _.
+    have:= forallP H (Sub k kO).
+    by rewrite valPE//=.
+  rewrite orbF => kK.
+  rewrite in_fnd/=.
+Abort.
+
+Lemma tc_tree_aux_step u sP R K A r s1 O N1 N2 d:
+  valid_tree A ->
+
+  gte sP R A ->
+  sigP sP R s1 O ->
+
+  step u s1 A = r ->
+
+  gtee sP K R (get_tree r) ->
+
+  tc_tree_aux sP A R (Func, O) = (Func, N1) ->
+  tc_tree_aux sP (get_tree r) K (Func, O) = (d, N2) ->
+  d = Func.
+Proof.
+  elim: A r s1 O N1 N2 d; 
+  only 1, 2, 3, 5: by move=> r s1 k O N1 N2 d _ _ <- /=; congruence.
+  - move=> p c r s1 O N1 N2 d _ GR sigP <-/={r} GK.
+    case C: check_callable => [D S][??] H; subst.
+    admit.
+  - move=> A HA s B HB r s1 O N1 N2 d/= + /gte_orP [GA GB Cs] SP <-{r}.
+    case: (boolP (is_dead _)) => [dA vB|dA /andP[vA bB]].
+      rewrite get_tree_Or/= is_dead_is_ko//= => /gtee_orP[GA' + Cs'].
+      case: ifP => kB; first by rewrite is_ko_step//=; case: ifP; congruence.
+      case eB: step => [B'|B'|B'|B'] /= GB';
+      (case: ifP => kB'; first by move=> +[??]; subst);
+      rewrite (sigma2ctx_cat1 (gte_w GA) GA')//=;
+      by apply: HB eB _; auto; apply/sigP_id.
+    case kA: is_ko; first (rewrite is_ko_step//=kA/=; case: ifP; first congruence).
+      move=> kB /gtee_orP[GA' GB' Cs'].
+      rewrite (sigma2ctx_cat1 (gte_w GA) GA')//=;
+      move=> H1 H2; by have [] := tc_tree_aux_cat GB GB' (bbOr_valid bB) H1 H2.
+    case: ifP => kB.
+      case eA: step => [A'|A'|A'|A']/=; rewrite !(is_ko_cutr,kB, andbT);
+      (case kA': is_ko; [by congruence | ]) => /gtee_orP[GA' GB' Cs'];
+      by apply: HA eA GA'.
+    case: ifP => cutA; last by [].
+    case eA: step => [A'|A'|A'|A']/=; rewrite !(is_ko_cutr,kB, andbT,andbF);
+    case tA: tc_tree_aux => [DA SA];
+    case tB: tc_tree_aux => [DB SB];
+    case tB': tc_tree_aux => [DB' SB']/=;
+    case tA': tc_tree_aux => [DA' SA']/=;
+    move=> /gtee_orP[GA' GB' Gs']; destruct DA, DB => //-[?]; subst;
+    cycle 1; [|
+      rewrite (step_keep_cut eA isT) cutA;
+      rewrite (sigma2ctx_cat1 (gte_w GB) GB')//= in tB';
+      have ? := HA _ _ _ _ _ _ vA GA SP eA GA' tA tA'; subst;
+      (by case: ifP => kA' [??]; subst; have [] := tc_tree_aux_cat GB GB' (bbOr_valid bB) tB tB')..].
+    move: tB'; rewrite cutr_tc_tree_aux => -[??]; subst.
+    case kA': is_ko => -[??]; subst; first by auto.
+    by apply: HA eA _ tA tA'.
+  - move=> A HA B0 HB0 B HB r s O N1 N2 d /= /and4P[vA+++] /gte_andP[GA GB0 GB] SP.
+    case kA: is_ko.
+      rewrite is_ko_success//=is_ko_failed//=is_ko_step//=.
+      move=> /eqP->{B0 HB0 GB0} bB _ <-{r} /gtee_andP[cA' cB' _][?]/=; rewrite kA; congruence.
+    case sA: success => /=.
+      rewrite succes_is_solved// => vB bB ckB <-{r}.
+      case:ifP => kB0.
+        case eB: step => [B'|B'|B'|B']//=; 
+        rewrite success_is_ko?success_cut//sA(kB0, is_ko_cutr)?get_ctxS_cutl//;
+        move=> /gtee_andP[GA' GB0' GB'];
+        move=> H1 H2; admit.
+      case eB: step => [B'|B'|B'|B']//=; rewrite success_is_ko?success_cut//sA(kB0, is_ko_cutr)?get_ctxS_cutl//;
+      move=> /gtee_andP[GA' GB0' GB'];
+      case tA: (tc_tree_aux _ A) => [DA SA];
+      case tA': (tc_tree_aux _ A) => [DA' SA'];
+      case tB0: (tc_tree_aux _ B0) => [DB0 SB0]/=;
+      case tB0': (tc_tree_aux _ B0) => [DB0' SB0']/=;
+      case tB: (tc_tree_aux _ B) => [DB SB]/=;
+      case tB': (tc_tree_aux _ B') => [DB' SB']/=;
+      destruct DB, DB0 => //= -[?][??]; subst;
+      try rewrite (HB _ _ _ _ _ _ vB GB (sigP_success _ SP) eB GB' tB tB')/=;
+      admit.
+      (* - 
+         destruct DB0' => //.
+        have TODO: compat_sig O K by admit.
+        have TODO1: compat_sig SA' K by admit.
+        have [MP H] := more_precise_tc_tree_aux GA GA' vA (more_precise_refl _) TODO tA tA'.
+        have:= more_precise_tc_tree_aux GB0 GB0' (bbAnd_valid bB) MP TODO1 tB0 tB0'.
+        move=> [_ /(_ (H erefl))].
+      - rewrite tc_tree_aux_catR in tB'.
+        by apply: HB vB GB (sigP_success _ _) eB GB' tB tB'.
+      - destruct DB0' => //.
+        have TODO: compat_sig O K by admit.
+        have [MP H] := more_precise_tc_tree_aux GA GA' vA (more_precise_refl _) TODO tA tA'.
+        have TODO1: compat_sig SA' K by admit.
+        have:= more_precise_tc_tree_aux GB0 GB0' (bbAnd_valid bB) MP TODO1 tB0 tB0'.
+        by move=> [_ /(_ (H erefl))].
+      - destruct DB0' => //.
+        have TODO: compat_sig O K by admit.
+        have [MP H] := more_precise_tc_tree_aux GA GA' vA (more_precise_refl _) TODO tA tA'.
+        have TODO1: compat_sig SA' K by admit.
+        have:= more_precise_tc_tree_aux GB0 GB0' (bbAnd_valid bB) MP TODO1 tB0 tB0'.
+        by move=> [_ /(_ (H erefl))]. *)
+    move=> /eqP->{B0 HB0 GB0}.
+    case:ifP => [fA bB|fA bB] _ <-.
+      rewrite failed_expand//= failed_success//=.
+      move=> /gtee_andP[GA' GB' _].
+      case:ifP => kB; first by case:ifP; congruence.
+      case tA: (tc_tree_aux _ A) => [DA SA].
+      case tA': (tc_tree_aux _ A) => [DA' SA'].
+      case tB: (tc_tree_aux _ B) => [DB SB].
+      case tB': (tc_tree_aux _ B) => [DB' SB'].
+      move=> [??]; subst.
+      rewrite kA => -[??]; subst.
+      have TODO: compat_sig O K by admit.
+      have [M1 H] := more_precise_tc_tree_aux GA GA' vA (more_precise_refl _) TODO tA tA'.
+      have TODO1: compat_sig SA' K by admit.
+      have := more_precise_tc_tree_aux GB GB' (bbAnd_valid bB) M1 TODO1 tB tB'.
+      by move=> [_ /(_ (H erefl))].
+    rewrite base_and_is_ko//=.
+    case eA: step => [A'|A'|A'|A']/=; rewrite ?(base_and_is_ko bB); last first.
+    - by rewrite !(expand_solved_same _ eA) in sA.
+    - by rewrite !(expand_failed_same _ eA) in fA.
+    all: move=> /gtee_andP[cA' cB' _].
+    all: case: ifP => kA'; first by congruence.
+    all: case tA: (tc_tree_aux _ A) => [DA SA];
+         case tA': (tc_tree_aux _ A') => [DA' SA'];
+         case tB: (tc_tree_aux _ B) => [DB SB];
+         case tB': (tc_tree_aux _ B) => [DB' SB'];
+         case tB2: (tc_tree_aux _ B) => [DB2 SB2].
+    all: move=> [??]; subst.
+    have:= more_precise_tc_tree_aux GB cB' (base_and_valid bB) _ _ tB tB'.
+    all: admit.
+Admitted.
+
+Lemma sigP_more_precise sP tE s N O:
+  more_precise N O -> sigP sP tE s N -> sigP sP tE s O.
+Proof.
+  move=> MP /forallP H; apply/forallP=> -[k kO].
+  have kN := fsubsetP (more_precise_sub MP) k kO.
+  have /={H} := H (Sub k kN).
+  have [kS|bkS] := fndP.
+    rewrite !valPE/=; apply: incl_good_assignment (in2_more_precise MP _ _) _.
+    by rewrite compat_type_comm more_precise_same_type.
+  rewrite ?valPE/= => /eqP def_N; have ino := in2_more_precise MP kO kN.
+  have /comp_weak wON := more_precise_same_type MP kO kN.
+  by rewrite -eq_incl weak_incl wON -def_N ino.
+Qed.
+
+
+*)
